\documentclass{article}


\usepackage{amssymb}

\begin{document}


\[
\{ D^{j}T^{k}\psi\;:\: j,k\in\mathbb{Z}\}\]

\[
\Phi(K)=\cup_{i=1}^{n}\varphi_{i}(K).\]

\[
\tilde{\varphi_{i}}(x,w)=(\varphi_{i}(x),\sigma_{i}(w))\]

\[
G=\{(x,n,y)\in X\times\mathbb{Z}\times X\;:\; T^{k}(x)=T^{l}(y),n=k-l\}.\]

\[
Z(U,V,k,l):=\{(x,k-l,y)\in G:x\in U,y\in V\},\]

\begin{eqnarray*}
f\ast g(x,k-l,y) & = & \sum f(x,m-n,z)\cdot g(z,(n+k)-(m+l),y),\end{eqnarray*}

\[
f^{*}(x,k-l,y)=\overline{f(y,l-k,x)}.\]

\[
\Vert f\Vert:=\sup\Vert\pi(f)\Vert\]

\begin{equation}
\alpha(f)(x,0,y)=\frac{1}{\sqrt{\vert T^{-1}(Tx))\vert\vert
T^{-1}(Ty))\vert}}f(Tx,0,Ty),\label{eq:alphainfty}\end{equation}

\begin{equation}
S(x,m-n,y)=\begin{cases}
\frac{1}{\sqrt{\vert T^{-1}(Tx)\vert}}, & \mbox{if }m=1,n=0,Tx=y,\\
0 & \mbox{otherwise,}\end{cases}\label{eq:isometry}\end{equation}

\begin{equation}
\alpha(f)=SfS^{\ast},\label{eq:Stacey1}\end{equation}

\begin{equation}
SS^{*}(x,k-l,y)=\frac{1}{\vert
T^{-1}(Tx)\vert}1_{R_{1,1}}(x,k-l,y).\label{eq:Stacey2}\end{equation}

\begin{equation}
\mathcal{L}(f)(x,0,y)=\frac{1}{\sqrt{\vert T^{-1}(x)\vert\vert
T^{-1}(y)\vert}}\sum_{\stackrel{Tu=x}{Tv=y}}f(u,0,v).\label{eq:transferinfty}
\end{equation}

\[
\langle\xi,\eta\rangle(x)=\frac{1}{\vert
T^{-1}(x)\vert}\sum_{Ty=x}\overline{\xi(y)}\eta(y),\]

\[
\iota(\varphi)(x,k-l,y)=\varphi(x)1_{R_{0,0}}(x,k-l,y),\]

\begin{eqnarray}
\iota(a)\iota(b)S & = &
\psi(\phi(a)\phi(b)\xi_{0})=\lim\psi(\sum_{i}\phi(a_{i})\xi_{0}\otimes\xi_{0}^{*
}\phi(b_{i})(\phi(b)\xi_{0}))\label{eq:defining}\\
 & = & \lim\sum_{i}\iota(a_{i})SS^{*}\iota(b_{i})\iota(b)S\nonumber \\
 & = & \lim\sum_{i}\iota(a_{i})S\iota(\mathcal{L}(b_{i}b))\nonumber \\
 & = & \lim\sum_{i}\iota(a_{i})\iota(\alpha\circ\mathcal{L}(b_{i}b))S\nonumber
\\
 & = &
\lim\sum_{i}(\psi,\iota)^{(1)}(\phi(a_{i})\xi_{0}\otimes\xi_{0}^{*}\phi(b_{i}
))(\iota(b)S)\nonumber \\
 & = & (\psi,\iota)^{(1)}(\phi(a))(\iota(b)S).\nonumber \end{eqnarray}

\begin{equation}
\psi(\xi\otimes\eta^{*}(\phi(b)\xi_{0}))=(\psi,\iota)^{(1)}(\xi\otimes\eta^{*}
)(\iota(b)S),\label{eq:definingbis}\end{equation}

\[
\iota(\beta(a))S_{i}=S_{i}\iota(a).\]

\begin{equation}
\iota(\beta(a))=\sum_{i=1}^{n}S_{i}\iota(a)S_{i}^{*}.\label{eq:inner}
\end{equation}

\[
\pi(f)\xi(u)=\int_{G^{u}}f(\gamma)(U(\gamma)\xi(s(\gamma)))\Delta^{\frac{1}{2}}
(\gamma)\, d\lambda^{u}(\gamma),\]

\[
\Delta(x,m-n,y)=\frac{D(x)D(Tx)\cdots D(T^{m-1}x)}{D(y)D(Ty)\cdots
D(T^{n-1}y)}.\]

\begin{equation}
\mathcal{L}_{D}^{*}(\mu)(f):=\int_{X}\sum_{Ty=x}D(y)f(y)\,
d\mu(x).\label{eq:Transfer}\end{equation}

\[
U(\gamma)(s(\gamma),c)=(r(\gamma),c),\]

\begin{eqnarray*}
\pi(\iota(\alpha(f))) & = & \pi(S_{1})\pi(\iota(f))\pi(S_{1})^{*}\\
 & + & \pi(S_{2})\pi(\iota(f))\pi(S_{2})^{*},\end{eqnarray*}

\[
m_{2}(z):=z\overline{m_{1}(-z)}.\]

\[
H_{n}\stackrel{S_{m,n}}{\longrightarrow}H_{m}\]

\[
US_{\infty,n+1}=S_{\infty,n+1}\pi(S_{1})=S_{\infty,n},\]

\begin{eqnarray*}
{(S}_{m,n}\xi)(z) & = & 2^{(m-n)/2}m_{1}(z)m_{1}(z^{2})\\
 & \cdots & m_{1}(z^{2^{(m-n)-1}})\xi(z^{2^{(m-n)}}).\end{eqnarray*}

\[
\mathcal{L}_{m_{1}}(f)(z)=\frac{1}{\vert T^{-1}(x)\vert}\sum_{w^{2}=z}\vert
m_{1}(w)\vert^{2}f(w).\]

\[
\rho(f)\xi(z_{1},z_{2},\ldots)=f(z_{1})\xi(z_{1},z_{2},\ldots),\]

$$U\xi(z_{1},z_{2},\ldots)=\xi(z_{1}^{2},z_{1},z_{2},\ldots)J^{\frac{1}{2}}(z_{1}
,z_{2},\ldots),$$

\[
\rho(f\circ T_{\infty})=U\rho(f)U^{-1},\]

\begin{multline*}
D(R_{\infty}(S_{\infty,n+1}\xi))(x)=D(R_{n+1}\xi)(x)=2^{1/2}(R_{n+1}\xi)(2x)\\
=2^{1/2}2^{\frac{-(n+1)}{2}}\xi(e^{2\pi
i(2^{-(n+1)}2x)})\phi(2^{-(n+1)}2x)=(R_{n}\xi)(x)\\
=(R_{\infty}S_{\infty,n}\xi)(x)=(R_{\infty}US_{\infty,n+1}\xi)(x).
\end{multline*}

\[
\bigoplus_{n\in\mathbb{Z}}\mathcal{W}_{n}=L^{2}(\mathbb{R}).\]

\begin{eqnarray}
\mathcal{W}_{0} & = &
\mathcal{V}_{1}\ominus\mathcal{V}_{0}=R_{1}L^{2}(\mathbb{T})\ominus
R_{0}L^{2}(\mathbb{T})\label{eq:Wzero}\\
 & = & R_{1}L^{2}(\mathbb{T})\ominus R_{1}\pi(S_{1})L^{2}(\mathbb{T})\nonumber
\\
 & = & R_{1}(L^{2}(\mathbb{T})\ominus\pi(S_{1})L^{2}(\mathbb{T}))\nonumber \\
 & = & R_{1}\pi(S_{2})L^{2}(\mathbb{T}),\nonumber \end{eqnarray}

\begin{eqnarray*}
\zeta_{k}(x)= & 2^{-1/2}(2^{1/2}m_{2}(e^{(2\pi i2^{-1}x)})e^{-2\pi
ikx})\phi(2^{-1}x)\\
= & e^{-2\pi ikx}\zeta(x)\end{eqnarray*}

\[
\zeta(x):=m_{2}(e^{\pi ix})\phi(2^{-1}x).\]

\begin{eqnarray*}
\zeta_{j,k}(x) & = & D^{j}\zeta_{k}(x)\\
 & = & 2^{j/2}e^{(-2\pi ik2^{j}x)}\zeta(2^{j}x).\end{eqnarray*}

\[
m_{2}(e^{\pi ix})\phi(2^{-1}x)\]

\[
G_{\infty}=\{(\underline{x},n-m,\underline{y})\,:\, T^{n}x_{1}=T^{m}y_{1}\}.\]

\end{document}