\documentclass[12pt]{article}


\usepackage{amssymb,verbatim}

\begin{document}


$$ E_{p}(\phi) = \tfrac{1}{p} \int_{M} |d\phi|^p \, v_{g} .$$

$$ \tau_{p}(\phi) = |d\phi|^{p-4} [|d\phi|^{2}\tau(\phi) + \tfrac{p-2}{2} d\phi(\operatorname{grad} |d\phi|^2)] =0  ,$$

$$ \tau(\phi) =  \operatorname{trace}{ \nabla d \phi } $$

$$ E^{2}(\phi) = \tfrac{1}{2} \int_{M} | \tau(\phi) |^{2} \, v_{g} .$$

$$ \tau^{2}(\phi) = - \Delta^{\phi} \tau(\phi) - \operatorname{trace}_{g}{R^{N}}(
d\phi, \tau(\phi) ) d\phi ,$$

$$ h( d\phi_{x}(X), d\phi_{x}(Y)) = \lambda^{2}(x) g(X,Y), $$

$$ R(X,Y) = [ \nabla_{X} , \nabla_{Y} ] - \nabla_{[X,Y]} ,$$

\begin{align}\label{longeq}
& |\tau(\phi)|^{4} - 2\Delta \lambda^{2} |\tau(\phi)|^{2} + 4 \Delta \lambda^{2}
\operatorname{div}{\langle d\phi , \tau(\phi)\rangle} + n (\Delta \lambda^{2})^{2} \\
& + 2 \langle d\phi , \tau(\phi) \rangle (\nabla |\tau(\phi)|^{2}) + |S|^{2} = 0 ,\notag
\end{align}

\begin{align}
 &h(d\phi(X),d\phi(Y)) = \lambda^{2} g(X,Y) ,\quad \forall X,Y \in {\mathcal{H}}
\label{eqa} ; \\
& - \Delta^{\phi}\tau(\phi) - \operatorname{trace}{{\mathrm R}^{N}(d\phi,
\tau(\phi))d\phi} = 0 \label{eqb};\\
&  \lambda^{2} \tau(\phi) + d\phi \operatorname{grad}{\lambda^{2}} = 0 \label{eqc}; \\
& |\tau(\phi)|^{4} - 2\Delta \lambda^{2} |\tau(\phi)|^{2} + 4 \Delta \lambda^{2}
\operatorname{div}{\langle d\phi , \tau(\phi)\rangle} + n (\Delta \lambda^{2})^{2} \label{eqd}\\
&+ 2 \langle d\phi
, \tau(\phi) \rangle (\nabla |\tau(\phi)|^{2}) + |S|^{2} = 0  .\notag
\end{align}

\begin{align}
& \Delta^{2} (f{\circ}\phi)  = \frac{\partial^{4} f}{\partial y^{\alpha}\partial
y^{\beta}\partial y^{\gamma}\partial y^{\delta}} \left[ g^{ij}g^{kl} \frac{\partial
\phi^{\alpha}}{\partial x^{i}} \frac{\partial \phi^{\beta}}{\partial x^{j}}
\frac{\partial \phi^{\gamma}}{\partial x^{k}} \frac{\partial
\phi^{\delta}}{\partial x^{l}} \right] + \label{eqe}\\
& \frac{\partial^{3} f}{\partial y^{\alpha}\partial y^{\beta}\partial y^{\gamma}}
\left[ \left( \frac{\partial^{2} \phi^{\gamma}}{\partial x^{i}\partial x^{j}}
\frac{\partial \phi^{\beta}}{\partial x^{k}}\frac{\partial \phi^{\alpha}}{\partial
x^{l}} + \frac{\partial^{2} \phi^{\beta}}{\partial x^{i}\partial x^{k}}
\frac{\partial \phi^{\gamma}}{\partial x^{j}}\frac{\partial \phi^{\alpha}}{\partial
x^{l}} + \frac{\partial^{2} \phi^{\alpha}}{\partial x^{i}\partial x^{l}}
\frac{\partial \phi^{\gamma}}{\partial x^{j}}\frac{\partial
\phi^{\beta}}{\partial x^{k}} + \right. \right. \notag\\
& \left. \frac{\partial^{2} \phi^{\beta}}{\partial x^{k}\partial x^{j}}
\frac{\partial \phi^{\gamma}}{\partial x^{i}}\frac{\partial \phi^{\alpha}}{\partial
x^{l}} + \frac{\partial^{2} \phi^{\alpha}}{\partial x^{l}\partial x^{j}}
\frac{\partial \phi^{\gamma}}{\partial x^{i}}\frac{\partial \phi^{\beta}}{\partial
x^{k}} + \frac{\partial^{2} \phi^{\alpha}}{\partial x^{l}\partial x^{k}}
\frac{\partial \phi^{\gamma}}{\partial x^{i}}\frac{\partial
\phi^{\beta}}{\partial x^{j}} \right) g^{ij}g^{kl} +  \notag\\
& \left. 2 g^{ij} \frac{\partial g^{kl}}{\partial x^{i}} \left( \frac{\partial
\phi^{\gamma}}{\partial x^{j}} \frac{\partial \phi^{\beta}}{\partial x^{k}}
\frac{\partial \phi^{\alpha}}{\partial x^{l}} \right) \right]  + \notag\\
& \frac{\partial^{2} f}{\partial y^{\alpha} \partial y^{\beta}} \left[ \left(
\frac{\partial^{3} \phi^{\beta}}{\partial x^{i}\partial x^{j}\partial x^{k}}
\frac{\partial \phi^{\alpha}}{\partial x^{l}} + \frac{\partial^{2}
\phi^{\beta}}{\partial x^{j}\partial x^{k}} \frac{\partial^{2}
\phi^{\alpha}}{\partial x^{l}\partial x^{i}} + \frac{\partial^{2}
\phi^{\beta}}{\partial x^{i}\partial x^{k}} \frac{\partial^{2}
\phi^{\alpha}}{\partial x^{l}\partial x^{j}} +
\right. \right. \notag\\
& \left. \frac{\partial^{3} \phi^{\alpha}}{\partial x^{i}\partial x^{j}\partial
x^{l}} \frac{\partial \phi^{\beta}}{\partial x^{k}} + \frac{\partial^{2}
\phi^{\beta}}{\partial x^{i}\partial x^{j}} \frac{\partial^{2}
\phi^{\alpha}}{\partial x^{l}\partial x^{k}} + \frac{\partial^{3}
\phi^{\alpha}}{\partial x^{i}\partial x^{k}\partial x^{l}} \frac{\partial
\phi^{\beta}}{\partial x^{j}} + \frac{\partial^{3} \phi^{\alpha}}{\partial
x^{j}\partial x^{k}\partial x^{l}}
\frac{\partial \phi^{\beta}}{\partial x^{i}} \right) g^{ij}g^{kl} + \notag\\
&\left. \left( \frac{\partial^{2} \phi^{\alpha}}{\partial x^{k}\partial x^{l}}
\frac{\partial \phi^{\beta}}{\partial x^{j}} + \frac{\partial^{2}
\phi^{\alpha}}{\partial x^{j}\partial x^{l}} \frac{\partial \phi^{\beta}}{\partial
x^{k}} + \frac{\partial^{2} \phi^{\beta}}{\partial x^{j}\partial x^{k}}
\frac{\partial \phi^{\alpha}}{\partial x^{l}} \right) 2 g^{ij} \frac{\partial
g^{kl}}{\partial x^{i}} + g^{ij} \frac{\partial^{2} g^{kl}}{\partial x^{i} \partial
x^{j}} \frac{\partial \phi^{\alpha}}{\partial x^{l}}
\frac{\partial \phi^{\beta}}{\partial x^{k}} \right] + \notag\\
&\frac{\partial f}{\partial y^{\alpha}} \left[ \frac{\partial^{2}
\phi^{\alpha}}{\partial x^{k}\partial x^{l}} g^{ij} \frac{\partial^{2}
g^{kl}}{\partial x^{i} \partial x^{j}} + \frac{\partial^{3} \phi^{\alpha}}{\partial
x^{j}\partial x^{k}\partial x^{l}} 2 g^{ij} \frac{\partial g^{kl}}{\partial x^{i}} +
\frac{\partial^{4} \phi^{\alpha}}{\partial x^{i}\partial x^{j}\partial x^{k}\partial
x^{l}}g^{ij}g^{kl} \right] . \notag
\end{align}

\begin{align}
& g^{ij} \frac{\partial \phi^{\alpha}}{\partial x^{i}}\frac{\partial
\phi^{\beta}}{\partial x^{j}} = \lambda^{2} h^{\alpha\beta} \label{s1};\\
&d\phi^{\gamma} \operatorname{grad}{\left(\lambda^{2}\right)} + \lambda^{2}
\tau^{\gamma}(\phi)  = 0 \label{s2};\\
&h^{\alpha\beta}\Delta(\lambda^{2}) + 
\operatorname{div}{ (\tau^{\beta}(\phi)d\phi^{\alpha})} +
\operatorname{div}{ (\tau^{\alpha}(\phi)d\phi^{\beta}}) -
\tau^{\alpha}(\phi)\tau^{\beta}(\phi) =\lambda^{2} dh^{\alpha\beta}(\tau(\phi)) \label{s3};\\
&g^{ij} \frac{\partial^{2} }{\partial x^{i} \partial x^{j}} \tau^{\alpha}(\phi) = 0,
\label{s4}
\end{align}

$$A^{\alpha\beta} = h^{\alpha\beta}\Delta(\lambda^{2}) +
g^{ij}\frac{\partial \phi^{\alpha}}{\partial x^{i}} \frac{\partial
\tau^{\beta}(\phi)}{\partial x^{j}} + g^{ij}\frac{\partial \phi^{\beta}}{\partial
x^{i}} \frac{\partial \tau^{\alpha}(\phi)}{\partial x^{j}}
+\tau^{\alpha}(\phi)\tau^{\beta}(\phi) - \lambda^{2} \frac{\partial
h^{\alpha\beta}}{\partial y^{p}} \tau^{p}(\phi),$$

\begin{align*}
|A|^{2} &=  n (\Delta \lambda^{2})^{2} + |\tau(\phi)|^{4} -
2(\Delta\lambda^{2})|\tau(\phi)|^{2} + 4 (\Delta\lambda^{2})
\operatorname{div}{\langle d\phi , \tau(\phi)\rangle} \label{eq10}\\
& + 4 g^{ij} \frac{\partial \phi^{\alpha}}{\partial x^{i}} \frac{\partial
\tau^{\beta}(\phi)}{\partial x^{j}} h_{\alpha\delta}h_{\beta\mu}
\tau^{\delta}(\phi)\tau^{\mu}(\phi)
  + 2 \lambda^{2} \tau^{\alpha}(\phi)\tau^{\beta}(\phi)
\frac{\partial h_{\alpha\beta}}{\partial y^{p}} \tau^{p}(\phi) \notag\\
& + 2 g^{ij} \frac{\partial \phi^{\alpha}}{\partial x^{i}} \frac{\partial
\tau^{\beta}(\phi)}{\partial x^{j}} h_{\alpha\delta}h_{\beta\mu} g^{kl}
\frac{\partial \phi^{\delta}}{\partial x^{k}} \frac{\partial
\tau^{\mu}(\phi)}{\partial x^{l}} +  2 g^{ij} \frac{\partial \phi^{\alpha}}{\partial
x^{i}} \frac{\partial \tau^{\beta}(\phi)}{\partial x^{j}}
h_{\alpha\delta}h_{\beta\mu} g^{kl} \frac{\partial \phi^{\mu}}{\partial x^{k}}
\frac{\partial
\tau^{\delta}(\phi)}{\partial x^{l}} \notag\\
& + 4 \lambda^{2} g^{ij} \frac{\partial \phi^{\alpha}}{\partial x^{i}} \frac{\partial
\tau^{\beta}(\phi)}{\partial x^{j}} \frac{\partial h_{\alpha\beta}}{\partial y^{p}}
\tau^{p}(\phi) + \lambda^{4} \frac{\partial h^{\alpha\beta}}{\partial y^{p}}
h_{\alpha\delta}h_{\beta\mu} \frac{\partial h^{\delta\mu}}{\partial y^{q}}
\tau^{p}(\phi) \tau^{q}(\phi) , \notag
\end{align*}

\begin{align*}
\langle d\phi, \tau(\phi) \rangle (\nabla |\tau(\phi)|^{2}) = 2 g^{ij} \frac{\partial
\phi^{\alpha}}{\partial x^{i}} \frac{\partial \tau^{\beta}(\phi)}{\partial x^{j}}
h_{\alpha\delta}h_{\beta\mu} \tau^{\delta}(\phi)\tau^{\mu}(\phi)
  +  \lambda^{2} \tau^{\alpha}(\phi)\tau^{\beta}(\phi)
\frac{\partial h_{\alpha\beta}}{\partial y^{p}} \tau^{p}(\phi)
\end{align*}

$$ S^{\alpha\beta} =  g^{ij} \frac{\partial \phi^{\alpha}}{\partial x^{i}}
\frac{\partial \tau^{\beta}(\phi)}{\partial x^{j}} + \lambda^{2} h^{\alpha\delta}
\Gamma^{\beta}_{\gamma\delta} \tau^{\gamma}(\phi)
  + g^{ij} \frac{\partial \phi^{\beta}}{\partial x^{i}}
\frac{\partial \tau^{\alpha}(\phi)}{\partial x^{j}} + \lambda^{2} h^{\beta\delta}
\Gamma^{\alpha}_{\gamma\delta} \tau^{\gamma}(\phi) .
$$

\begin{align*}
|S|^{2} &= 2 g^{ij} \frac{\partial \phi^{\alpha}}{\partial x^{i}} \frac{\partial
\tau^{\beta}(\phi)}{\partial x^{j}} h_{\alpha\delta}h_{\beta\mu} g^{kl}
\frac{\partial \phi^{\delta}}{\partial x^{k}} \frac{\partial
\tau^{\mu}(\phi)}{\partial x^{l}} +  2 g^{ij} \frac{\partial \phi^{\alpha}}{\partial
x^{i}} \frac{\partial \tau^{\beta}(\phi)}{\partial x^{j}}
h_{\alpha\delta}h_{\beta\mu} g^{kl} \frac{\partial \phi^{\mu}}{\partial x^{k}}
\frac{\partial
\tau^{\delta}(\phi)}{\partial x^{l}} \\
& + 4 \lambda^{2} g^{ij} \frac{\partial \phi^{\alpha}}{\partial x^{i}} \frac{\partial
\tau^{\beta}(\phi)}{\partial x^{j}} \frac{\partial h_{\alpha\beta}}{\partial y^{p}}
\tau^{p}(\phi) + \lambda^{4} \frac{\partial h^{\alpha\beta}}{\partial y^{p}}
h_{\alpha\delta}h_{\beta\mu} \frac{\partial h^{\delta\mu}}{\partial y^{q}}
\tau^{p}(\phi) \tau^{q}(\phi).
\end{align*}

\begin{align*}
&- (\Delta^{\phi}  \tau(\phi) )^{\alpha}= g^{ij} \left[ \frac{\partial^{2}
\tau^{\alpha}(\phi)}{\partial x^{i}\partial x^{j}}  + \frac{\partial
\tau^{\gamma}(\phi)}{\partial x^{j}} \frac{\partial \phi^{\beta}}{\partial x^{i}}
\Gamma^{\alpha}_{\beta\gamma} + \frac{\partial \tau^{\gamma}(\phi)}{\partial x^{i}}
\frac{\partial \phi^{\beta}}{\partial x^{j}} \Gamma^{\alpha}_{\beta\gamma} +
\tau^{\gamma}(\phi) \frac{\partial^{2} \phi^{\beta}}{\partial
x^{i}\partial x^{j}} \Gamma^{\alpha}_{\beta\gamma} \right.\\
  &+ \left.
\tau^{\gamma}(\phi) \frac{\partial \phi^{\beta}}{\partial x^{j}} \frac{\partial
\Gamma^{\alpha}_{\beta\gamma}}{\partial y^{\mu}} \frac{\partial \phi^{\mu}}{\partial
x^{i}} + \tau^{\mu}(\phi) \frac{\partial \phi^{\beta}}{\partial x^{j}}
\Gamma^{\gamma}_{\mu\beta} \frac{\partial \phi^{\delta}}{\partial x^{i}}
\Gamma^{\alpha}_{\gamma\delta} - \Gamma^{k}_{ij} \frac{\partial
\tau^{\alpha}(\phi)}{\partial x^{k}}
  - \Gamma^{k}_{ij} \tau^{\gamma}(\phi)
\frac{\partial \phi^{\beta}}{\partial x^{k}}
\Gamma^{\alpha}_{\beta\gamma} \right] \\
& = 2 g^{ij} \frac{\partial \tau^{\gamma}(\phi)}{\partial x^{i}} \frac{\partial
\phi^{\beta}}{\partial x^{j}} \Gamma^{\alpha}_{\beta\gamma} + \tau^{\gamma}(\phi)
\tau^{\beta}(\phi) \Gamma^{\alpha}_{\beta\gamma} + \lambda^{2} \tau^{\gamma}(\phi)
h^{\beta\mu} \frac{\partial \Gamma^{\alpha}_{\beta\gamma}}{\partial y^{\mu}} +
\lambda^{2} h^{\beta\delta}\tau^{\mu}(\phi) \Gamma^{\gamma}_{\mu\beta}
\Gamma^{\alpha}_{\gamma\delta} ,
\end{align*}

\begin{align*}
- \lambda^{2} {\mathrm {Ric}}^{N} \tau(\phi) &=  \lambda^{2} \left[ - \frac{\partial
h^{\alpha\beta}}{\partial y^{\gamma}} \Gamma^{\delta}_{\alpha\beta} - h^{\alpha\beta}
\frac{\partial \Gamma^{\delta}_{\alpha\gamma}}{\partial y^{\beta}} - \sum_{\mu
=1}^{n} h^{\alpha\beta} \Gamma^{\mu}_{\alpha\gamma} \Gamma^{\delta}_{\mu\beta}
\right] \tau^{\gamma}(\phi) .
\end{align*}

\begin{align*}
\tau^{2}(\phi)  &= \left[ 2 g^{ij} \frac{\partial \tau^{\gamma}(\phi)}{\partial
x^{i}} \frac{\partial \phi^{\beta}}{\partial x^{j}} \Gamma^{\alpha}_{\beta\gamma} +
\tau^{\gamma}(\phi) \tau^{\beta}(\phi) \Gamma^{\alpha}_{\beta\gamma} - \lambda^{2}
\frac{\partial h^{\delta\beta}}{\partial y^{\gamma}} \Gamma^{\alpha}_{\delta\beta}
\tau^{\gamma}(\phi)\right]  \frac{\partial }{\partial y^{\alpha}}= 0.
\end{align*}

\begin{equation*}
\tau^{2} (\psi\circ\phi) = \lambda^{4} \tau^{2}(\psi) \circ \phi ,
\end{equation*}

\begin{equation}\label{trace}
n \Delta(\lambda^{2}) + 2 \operatorname{div}{\langle d\phi , \tau(\phi)\rangle} = |\tau(\phi)|^{2} ,
\end{equation}

\begin{align*}
\phi : {{\mathbb R}}^{n}\setminus\{0\} &\to {{\mathbb R}}^n \\
x &\mapsto \frac{x}{|x|^2}
\end{align*}

\begin{align*}
\phi : {{\mathbb R}}^{4}\setminus\{0\} &\to {{\mathbb R}}^4 \\
x &\mapsto \frac{x}{|x|^2}
\end{align*}

\begin{align*}
|\tau(\phi)|^2 &= \frac{16}{|x|^6} ; \quad \Delta \lambda^2 = \frac{8}{|x|^6} ; \quad
\langle d\phi,\tau(\phi)\rangle = 4\frac{x}{|x|^6} ; \quad \operatorname{div} \langle
d\phi,\tau(\phi)\rangle = -\frac{8}{|x|^6}.
\end{align*}

\begin{align*}
S^{\alpha\alpha} &= -\tfrac{8}{|x|^8} \left( |x|^2 + 2 (x^{\alpha})^2 \right) ; \quad
S^{\alpha\beta} = -\tfrac{16}{|x|^8}  x^{\alpha}x^{\beta} ,
\end{align*}

$$ A_{E}F = (\nabla_{E^{\mathcal{H}}} F^{\mathcal{H}})^{\mathcal{V}} \quad B_{E}F = (\nabla_{E^{\mathcal{V}}}F^{\mathcal{V}})^{\mathcal{H}}, \quad E,F \in \Gamma(TM).$$

\begin{align*}
& d\phi(-\Delta X) + \Delta^{\mathcal{H}} (\ln\lambda) d\phi(X) + (n-2) \nu(\ln\lambda)d\phi(X)
  + 2 d\phi(\nabla_{\operatorname{grad}^{\mathcal{H}} \ln\lambda} X) \\
  &+ 2d\phi(\operatorname{grad} X(\ln\lambda))-d\phi(\nabla_{X} (\operatorname{grad}^{\mathcal{H}}\ln\lambda)) -2 (\operatorname{div}^{\mathcal{H}} X) d\phi(\operatorname{grad} \ln\lambda)\\
& + X(\ln \lambda)d\phi(X) 
 - d\phi (\nabla_{X} \operatorname{grad} \ln\lambda) + \lambda^2 \operatorname{Ricci}^{N}(d\phi(X))
 + (n-1) d\phi(\nabla_{X} \nu)  \\
 &- (m-n)[ \mu(\ln\lambda) d\phi(X) - \langle X, \mu \rangle d\phi(\operatorname{grad}\ln\lambda)]
-(m-n)d\phi (\nabla_{X} \mu)+ n d\phi(A^{*}_{X}\nu) \\
&+ \operatorname{trace} d\phi( (\nabla A)^{*}_{X} - (\nabla A)X + 3A^{*}_{\nabla X} + (\nabla_{X}
B^{*})^{*} - B_{\nabla X} + 2 B_{\nabla_{X}} -2 A^{*}_{\nabla_{X}} ) = 0,
\end{align*}

\begin{align*}
\nabla^{\phi}_{e_{i}} d\phi(X)
&= e_{i}(\ln \lambda) d\phi(X) + X(\ln \lambda) d\phi(e_{i}) - \langle X,e_{i}\rangle
d\phi(\operatorname{grad} \ln \lambda) + d\phi(\nabla_{e_{i}}X) ,
\end{align*}

\begin{align*}
&\nabla^{\phi}_{e_{i}} \nabla^{\phi}_{e_{i}} d\phi(X) 
= e_{i}(e_{i}(\ln \lambda)) d\phi(X) + (e_{i}(\ln \lambda))^2 d\phi(X) + e_{i}(\ln \lambda)X(\ln \lambda)d\phi(e_{i}) \\
&-e_{i}(\ln \lambda)\langle X,e_{i} \rangle d\phi(\operatorname{grad}\ln \lambda)
+ e_{i}(\ln \lambda)d\phi(\nabla_{e_{i}}X) + e_{i}(X(\ln\lambda))d\phi(e_{i}) \\
&+ X(\ln\lambda) \nabla^{\phi}_{e_{i}} d\phi(e_{i}) - e_{i}\langle X,e_{i} \rangle
d\phi(\operatorname{grad}\ln \lambda)
- \langle X,e_{i} \rangle e_{i}(\ln \lambda) d\phi(\operatorname{grad}\ln \lambda) \\
&- \langle X,e_{i} \rangle (\operatorname{grad}^{\mathcal{H}}\ln \lambda) (\ln \lambda) d\phi(e_{i})
+ \langle X,e_{i} \rangle \langle \operatorname{grad}\ln\lambda ,e_{i} \rangle d\phi(\operatorname{grad}\ln \lambda) \\
&- \langle X,e_{i} \rangle d\phi(\nabla_{e_{i}} \operatorname{grad}^{\mathcal{H}}\ln\lambda) + e_{i}(\ln \lambda)d\phi(\nabla_{e_{i}}X) \\
&+ (\nabla_{e_{i}}X)^{\mathcal{H}}(\ln\lambda)d\phi(e_{i}) - \langle e_{i},\nabla_{e_{i}}X
\rangle d\phi(\operatorname{grad}\ln\lambda) + d\phi(\nabla_{e_{i}}(\nabla_{e_{i}}X)^{\mathcal{H}}) .
\end{align*}

\begin{align*}
&\big( \nabla^{\phi}_{e_{i}} \nabla^{\phi}_{e_{i}} -
\nabla^{\phi}_{\nabla_{e_{i}}e_{i}}\big) d\phi(X) =
e_{i}(e_{i}(\ln \lambda)) d\phi(X) + 2 d\phi(\nabla_{\operatorname{grad}^{\mathcal{H}} \ln\lambda} X) \\
&+ d\phi(\operatorname{grad} (X(\ln\lambda))) 
+ X(\ln\lambda)(\nabla d\phi)(e_{i},e_{i}) -d\phi(\nabla_{X} (\operatorname{grad}^{\mathcal{H}}\ln\lambda)) \\
&+ (\nabla_{e_{i}}X)^{\mathcal{H}} (\ln\lambda)d\phi(e_{i}) 
- 2\langle e_{i},\nabla_{e_{i}}X \rangle d\phi(\operatorname{grad}\ln\lambda)
 + d\phi(\nabla_{e_{i}}(\nabla_{e_{i}}X)^{\mathcal{H}})\\
&- (\nabla_{e_{i}}e_{i})^{\mathcal{H}} (\ln \lambda) d\phi(X) +
d\phi(\nabla_{X}(\nabla_{e_{i}}e_{i})^{\mathcal{V}} ) - d\phi(\nabla_{\nabla_{e_{i}}e_{i}}X).
\end{align*}

\begin{align*}
- \nabla^{\phi}_{\nabla_{e_{s}}e_{s}} d\phi(X) &= - (\nabla_{e_{s}}e_{s} )^{\mathcal{H}} (\ln
\lambda) d\phi(X)- X(\ln \lambda) d\phi(\nabla_{e_{s}}e_{s})\\
&+ \langle X, \nabla_{e_{s}}e_{s} \rangle d\phi(\operatorname{grad}\ln\lambda)  
- d\phi ( \nabla_{(\nabla_{e_{s}}e_{s})^{\mathcal{H}}} X ) - d\phi
([(\nabla_{e_{s}}e_{s})^{\mathcal{V}},X]),
\end{align*}

\begin{align*}
&(\nabla^{\phi}_{e_{s}} \nabla^{\phi}_{e_{s}} - \nabla^{\phi}_{\nabla_{e_{s}}e_{s}})
d\phi(X) = d\phi(\nabla_{e_{s}}\nabla_{e_{s}} X) - d\phi(\nabla_{e_{s}}\nabla_{X}
e_{s})  - d\phi(\nabla_{\nabla_{e_{s}}X}e_{s})\\
&+ d\phi(\nabla_{\nabla_{X}e_{s}}e_{s}) 
- (\nabla_{e_{s}}e_{s} )^{\mathcal{H}} (\ln \lambda) d\phi(X) - X(\ln \lambda)
d\phi(\nabla_{e_{s}}e_{s})\\
& + \langle X, \nabla_{e_{s}}e_{s} \rangle
d\phi(\operatorname{grad}\ln\lambda)- d\phi (\nabla_{\nabla_{e_{s}}e_{s}}X) 
+ d\phi (\nabla_{X}(\nabla_{e_{s}}e_{s})^{\mathcal{V}}).
\end{align*}

\begin{align*}
&-\Delta (\tau(\phi))
= d\phi(-\Delta X) - d\phi(\nabla_{e_{i}}(\nabla_{e_{i}}X)^{\mathcal{V}}) + \Delta^{\mathcal{H}} (\ln\lambda) d\phi(X) + n\nu(\ln\lambda) d\phi(X) \\
& + 2 d\phi(\nabla_{\operatorname{grad}^{\mathcal{H}} \ln\lambda} X) + d\phi(\operatorname{grad} X(\ln\lambda)) -d\phi(\nabla_{X} (\operatorname{grad}^{\mathcal{H}}\ln\lambda)) -2 (\operatorname{div}^{\mathcal{H}} X) d\phi(\operatorname{grad} \ln\lambda) \\
& + X(\ln \lambda)(\tau(\phi) + (m-n) d\phi(\mu) )
+ (\nabla_{e_{i}}X)^{\mathcal{H}} (\ln\lambda)d\phi(e_{i})  + n d\phi(\nabla_{X} \nu) \\
& - (m-n)[ \mu(\ln\lambda) d\phi(X) + X(\ln\lambda) d\phi(\mu) - \langle X, \mu \rangle d\phi(\operatorname{grad}\ln\lambda)] \\
& - d\phi(\nabla_{e_{s}}\nabla_{X} e_{s}) - d\phi(\nabla_{\nabla_{e_{s}}X}e_{s}) +
d\phi(\nabla_{\nabla_{X}e_{s}}e_{s})+ d\phi (\nabla_{X}(\nabla_{e_{s}}e_{s})^{\mathcal{V}} ).
\end{align*}

\begin{align*}
&(\nabla_{e_{i}}X)^{\mathcal{H}} (\ln\lambda)d\phi(e_{i}) 
= d\phi( \operatorname{grad}  X (\ln\lambda ) ) - d\phi(\nabla_{X} \operatorname{grad} \ln\lambda)\\
& - \langle (\nabla_{e_{i}}X)^{\mathcal{V}} ,  \operatorname{grad}^{\mathcal{V}} \ln\lambda \rangle d\phi(e_{i}).
\end{align*}

\begin{align*}
- \langle (\nabla_{e_{i}}X)^{\mathcal{V}} ,  \operatorname{grad}^{\mathcal{V}} \ln\lambda \rangle d\phi(e_{i}) &=
 - \langle \tfrac{1}{2} (\nabla_{e_{i}}X)^{\mathcal{V}} ,  \operatorname{grad}^{\mathcal{V}} \ln\lambda \rangle d\phi(e_{i}) \\
&+ \langle \tfrac{1}{2} (\nabla_{X}e_{i})^{\mathcal{V}} ,  \operatorname{grad}^{\mathcal{V}} \ln\lambda \rangle d\phi(e_{i})
- |\operatorname{grad}^{\mathcal{V}} \ln\lambda|^2 d\phi(X)
\end{align*}

\begin{align*}
&- \langle (\nabla_{e_{i}}X)^{\mathcal{V}} ,  \operatorname{grad}^{\mathcal{V}} \ln\lambda \rangle d\phi(e_{i}) = - d\phi(\nabla_{X}\operatorname{grad}^{\mathcal{V}} \ln\lambda) - 2|\operatorname{grad}^{\mathcal{V}} \ln\lambda|^2 d\phi(X).
\end{align*}

\begin{align*}
(\nabla_{e_{i}}X)^{\mathcal{H}} (\ln\lambda)d\phi(e_{i}) &=  d\phi( \operatorname{grad}  X (\ln\lambda ) ) - d\phi(\nabla_{X} \operatorname{grad} \ln\lambda)- d\phi(\nabla_{X}\nu) \\
&- 2|\nu|^2 d\phi(X)
\end{align*}

\begin{align*}
&-\Delta (\tau(\phi)) =  d\phi(-\Delta X) - d\phi(\nabla_{e_{i}}(\nabla_{e_{i}}X)^{\mathcal{V}})
+ \Delta^{\mathcal{H}} (\ln\lambda) d\phi(X) \\
&+ (n-2) \nu(\ln\lambda)d\phi(X) 
 + 2 d\phi(\nabla_{\operatorname{grad}^{\mathcal{H}} \ln\lambda} X) + 2d\phi(\operatorname{grad} X(\ln\lambda)) \\
&-d\phi(\nabla_{X} (\operatorname{grad}^{\mathcal{H}}\ln\lambda)) -2 (\operatorname{div}^{\mathcal{H}} X) d\phi(\operatorname{grad} \ln\lambda)
+ X(\ln \lambda)\tau(\phi) - d\phi (\nabla_{X} \operatorname{grad} \ln\lambda) \\
& + (n-1) d\phi(\nabla_{X} \nu)  - (m-n)[ \mu(\ln\lambda) d\phi(X) - \langle X, \mu \rangle d\phi(\operatorname{grad}\ln\lambda)] \\
& - d\phi(\nabla_{e_{s}}\nabla_{X} e_{s}) - d\phi(\nabla_{\nabla_{e_{s}}X}e_{s}) +
d\phi(\nabla_{\nabla_{X}e_{s}}e_{s})+ d\phi (\nabla_{X}(\nabla_{e_{s}}e_{s})^{\mathcal{V}} ).
\end{align*}

\begin{align*}
&d\phi(\operatorname{trace}_{h} \nabla (\nabla X)^{\mathcal{V}}) = d\phi(\operatorname{trace} (\nabla A)X) ;\\
&d\phi(-\nabla_{e_{s}}\nabla_{X} e_{s} - \nabla_{\nabla_{e_{s}}X}e_{s}
+ \nabla_{\nabla_{X}e_{s}}e_{s} + \nabla_{X}(\nabla_{e_{s}}e_{s})^{\mathcal{V}}) = -(m-n)d\phi(\nabla_{X}\mu) \\
&+ \operatorname{trace} d\phi( (\nabla A)^{*}_{X} + 3 A^{*}_{\nabla X} + (\nabla_{X} B^{*})^{*} -
B_{\nabla X} -2A^{*}_{\nabla_{X}}  + 2 B_{\nabla_{X}}) + n d\phi(A^{*}_{X}\nu).
\end{align*}

$$ d\phi((\nabla_{e_{i}}A )_{e_{i}} X) =  d\phi(\nabla_{e_{i}} (\nabla_{e_{i}} X)^{\mathcal{V}} ),$$

\begin{align*}
&\langle -\nabla_{e_{s}}\nabla_{X} e_{s} - \nabla_{\nabla_{e_{s}}X}e_{s}
+ \nabla_{\nabla_{X}e_{s}}e_{s} + \nabla_{X}\nabla_{e_{s}}e_{s}, e_{j}\rangle  \\
&= \langle (\nabla_{e_{s}}A)_{X} e_{j}, e_{s}\rangle  + \langle A_{\nabla_{e_{s}} X}
e_{j}, e_{s}\rangle + \langle (\nabla_{X}B^{*})_{e_{s}} e_{j}, e_{s}\rangle + \langle
B^{*}_{\nabla_{e_{s}}X} e_{j}, e_{s}\rangle \\
&+ 2 \langle \nabla_{[e_{s},X]} e_{j} ,e_{s} \rangle
\end{align*}

\begin{align*}
\langle \nabla_{[e_{s},X]} e_{j} , e_{s} \rangle &= \langle e_{j} , A^{*}_{\nabla_{e_{s}}X} e_{s} -A^{*}_{\nabla_{X}e_{s}} e_{s} -
B_{\nabla_{e_{s}}X} e_{s} + B_{\nabla_{X}e_{s}} e_{s} \rangle .
\end{align*}

\begin{align*}
 \langle (\nabla_{e_{i}}A)^{*}_{X} e_{i}, e_{j}\rangle &= - n\langle  e_{j} , A^{*}_{X}\nu \rangle ;\\
 A^{*}_{\nabla_{e_{i}} X} e_{i} &=  A^{*}_{\nabla_{X}e_{i}} e_{i} = 0 ;\\
\langle (\nabla_{X}B^{*})^{*}_{e_{i}} e_{i}, e_{j}\rangle &= 
 B_{\nabla_{e_{i}}X}e_{i} = B_{\nabla_{X} e_{i}}  e_{i}  = 0.
\end{align*}

$$-\lambda^2 \operatorname{Ricci}^{N}(d\phi(X)).$$

\begin{align}
&- d\phi( \Delta (\operatorname{grad} \ln\lambda)) -\Delta(\ln \lambda) d\phi(\operatorname{grad} \ln \lambda) +  2 d\phi(\operatorname{grad} |\operatorname{grad} \ln \lambda|^2 )  \notag\\
& \quad + (2-n) |\operatorname{grad} \ln \lambda|^2 d\phi(\operatorname{grad} \ln \lambda)  + \lambda^2
\operatorname{Ricci}^{N}(d\phi(\operatorname{grad}\ln\lambda)) =0. \label{eqf}
\end{align}

\begin{align*}
&d\phi(-\Delta \mu)+ \Delta^{\mathcal{H}} (\ln\lambda) d\phi(\mu) + 2 d\phi(\nabla_{\operatorname{grad}^{\mathcal{H}} \ln\lambda} \mu) + 2d\phi(\operatorname{grad} \mu(\ln\lambda)) \\
& -d\phi(\nabla_{\mu} (\operatorname{grad}^{\mathcal{H}}\ln\lambda)) -2 (\operatorname{div}^{\mathcal{H}} \mu) d\phi(\operatorname{grad} \ln\lambda)  \\
&   +(m-2) |\mu |^2 d\phi(\operatorname{grad} \ln\lambda)  - d\phi (\nabla_{\mu} \operatorname{grad} \ln\lambda) + \lambda^2\operatorname{Ricci}^{N}(d\phi(\mu)) \\
&   + d\phi(\nabla_{\mu} \nu) + (2-m) d\phi(\nabla_{\mu}\mu)  -2(m-2)\mu(\ln\lambda) d\phi(\mu)\\
&+  \operatorname{trace} d\phi( (\nabla A)^{*}_{\mu} - (\nabla A)\mu + 3A^{*}_{\nabla \mu} +
(\nabla_{\mu} B^{*})^{*} + 2 B_{\nabla_{\mu}}- B_{\nabla \mu} -2
A^{*}_{\nabla_{\mu}}) \\
&+ 2 d\phi(A^{*}_{\mu}\nu) = 0.
\end{align*}

\begin{align*}
&d\phi(\Delta \mu) - \lambda^2 \operatorname{Ricci}^{N}(d\phi(\mu)) + (m-n) d\phi(\nabla_{\mu}\mu) \\
&- (\operatorname{trace} d\phi( (\nabla A)^{*}_{\mu} - (\nabla A)\mu + 3A^{*}_{\nabla \mu}
 + (\nabla_{\mu} B^{*})^{*} + 2 B_{\nabla_{\mu}}- B_{\nabla \mu} - 2 A^{*}_{\nabla_{\mu}} )) = 0.
\end{align*}

\begin{align*}
0 &= \operatorname{trace}_{g} \nabla^2 \operatorname{grad}\rho + (-2\Delta \rho + (2-m)|\operatorname{grad}\rho|^2) \operatorname{grad}\rho \\
&+ \tfrac{6-m}{2} \operatorname{grad} (|\operatorname{grad}\rho|^2 ) + \operatorname{Ricci}^{g}(\operatorname{grad}\rho) .
\end{align*}

\begin{align*}
\operatorname{grad} \ln\lambda &= -\tfrac{2\epsilon}{1+ \epsilon |x|^2} x ; \quad |\operatorname{grad} \ln\lambda|^2 = \tfrac{4|x|^2}{(1+ \epsilon |x|^2)^2}; \\
\operatorname{grad}|\operatorname{grad} \ln\lambda|^2 &= \tfrac{8(1- \epsilon |x|^2)}{(1+ \epsilon |x|^2)^3} x ; \quad
\Delta \ln\lambda = -\tfrac{2\epsilon}{(1+ \epsilon |x|^2)^2}(n + (n-2)\epsilon |x|^2) ;\\
(\operatorname{trace}\nabla^2) (\operatorname{grad}\ln\lambda)  &= \tfrac{4}{(1+ \epsilon |x|^2)^3}(n+2 +
(n-2)\epsilon|x|^2)x,
\end{align*}

$$-8(n-4)\tfrac{(1- \epsilon|x|^2)}{(1+ \epsilon |x|^2)^3} x =0 ,$$

\begin{align*}
\tau(\phi) &= \tfrac{4\epsilon}{1+ \epsilon |x|^2} x ; \quad |\tau(\phi)|^2 = \tfrac{4.16}{(1+ \epsilon |x|^2)^4} |x|^2 ;\\
\Delta \lambda^2 &= \tfrac{-16\epsilon}{(1+ \epsilon |x|^2)^4} (4-2\epsilon|x|^2) ; \quad
\operatorname{div} \langle d\phi ,\tau(\phi)\rangle  = \tfrac{16\epsilon}{(1+ \epsilon |x|^2)^4} (4-2\epsilon|x|^2) ;\\
\nabla |\tau(\phi)|^2 &= \tfrac{8.16(1-3\epsilon|x|^2)}{(1+\epsilon|x|^2)^5} x ;
\quad \langle d\phi ,\tau(\phi)\rangle (\nabla |\tau(\phi)|^2) = \tfrac{8.16^2
(1-3\epsilon|x|^2)}{(1+\epsilon|x|^2)^8} |x|^2 ,
\end{align*}

\begin{align*}
&|\tau(\phi)|^{4} - 2\Delta \lambda^{2} |\tau(\phi)|^{2} + 4 \Delta \lambda^{2}
\operatorname{div}{\langle d\phi , \tau(\phi)\rangle} + 4 (\Delta \lambda^{2})^{2} +
2 \langle d\phi , \tau(\phi) \rangle (\nabla |\tau(\phi)|^{2}) \\
&= \tfrac{16^3}{(1+\epsilon|x|^2)^8} |x|^2 (1+2 \epsilon -3\epsilon |x|^2),
\end{align*}

\begin{align*}
\nabla \rho &= \tfrac{2}{1 - |x|^2}x ; \quad
|\nabla \rho|^2 = \tfrac{4|x|^2}{(1 - |x|^2)^2} ;\\
\nabla|\nabla \rho|^2 &= 8\tfrac{1 + |x|^2}{(1 - |x|^2)^3}x ; \quad
\Delta \rho = \tfrac{2}{(1 - |x|^2)^2}( n(1 - |x|^2) +2 |x|^2) ;\\
\operatorname{trace}_{g} \nabla^{2} \nabla \rho &= \tfrac{4x}{(1 - |x|^2)^3} (n+2 - (n-2) |x|^2) .
\end{align*}

$$ \tfrac{8x}{(1 - |x|^2)^3} (4-n)(1+ |x|^2) =0 $$

$$ \Delta \lambda^2 = \tfrac{16}{(1 - |x|^2)^4} (4 + 2  |x|^2)$$

$$\tau(\phi) = -2 \operatorname{grad} \rho = \tfrac{-4}{1 - |x|^2} x \, \mbox{ and } \quad
|\tau(\phi)|^2 = \tfrac{64|x|^2}{(1 - |x|^2)^4}  .$$

$$ \langle d\phi , \tau(\phi) \rangle = \tfrac{-16}{(1 - |x|^2)^3} x \, \mbox{ and } \quad
\operatorname{div} \langle d\phi , \tau(\phi) \rangle = \tfrac{-16}{(1 - |x|^2)^4} (4 + 2 |x|^2) .$$

$$ 4 \Delta \lambda^2 + 2 \operatorname{div} \langle d\phi , \tau(\phi) \rangle =
\tfrac{32}{(1 - |x|^2)^4} (4 + 2 |x|^2) \neq |\tau(\phi)|^2,$$

\begin{align*}
\operatorname{grad} \rho &= -\tfrac{1}{x^{n}}\tfrac{\partial}{\partial x^{n}} ; \quad  |\operatorname{grad} \rho|^2 = \tfrac{1}{(x^{n})^2} ;\\
\operatorname{grad} |\operatorname{grad} \rho|^2 &= -\tfrac{2}{(x^{n})^3}\tfrac{\partial}{\partial x^{n}} ; \quad \Delta
\rho = \tfrac{1}{(x^{n})^2},
\end{align*}

$$\tfrac{2}{(x^{n})^3}(n-4) \tfrac{\partial}{\partial x^{n}}=0.$$

\begin{align*}
|\tau(\phi)|^2 &= \tfrac{4}{(x^{4})^4} ; \quad \Delta \lambda^2 = \tfrac{6}{(x^{4})^4} ;\\
\langle d\phi , \tau(\phi) \rangle &= \tfrac{2}{(x^{4})^3}\tfrac{\partial}{\partial
x^{4}} ; \quad \operatorname{div} \langle d\phi , \tau(\phi) \rangle = -\tfrac{6}{(x^{4})^4},
\end{align*}

$$ 4\Delta \lambda^2 + 2 \operatorname{div} \langle d\phi , \tau(\phi) \rangle = \tfrac{12}{(x^{4})^4} \neq |\tau(\phi)|^2$$

\begin{align*}
\operatorname{grad}^g \rho &= e_4 ; \quad |\operatorname{grad}^g \rho|_{g}^2 = 1 ; \quad \operatorname{grad}^g|\operatorname{grad}^g \rho|^2 = 0 ;\\
\Delta^g \rho & = -3 ; \quad \operatorname{trace}_{g} \nabla^2 \operatorname{grad} \rho = -3 e_{4}; \quad \operatorname{Ricci}(\operatorname{grad}^g \rho)  = -3 e_4,
\end{align*}

\begin{align*}
&\nabla^{g}_{e_{1}} e_{4} = - e_{1} ; \quad \nabla^{g}_{e_{2}} e_{4} = - e_{2} ;\quad
\nabla^{g}_{e_{3}} e_{4} = - e_{3} ; \quad \nabla^{g}_{e_{4}} e_{4} = 0 ; \\
&\nabla^{g}_{e_{1}} e_{1} =  \nabla^{g}_{e_{2}} e_{2} = \nabla^{g}_{e_{3}} e_{3} =
e_{4}.
\end{align*}

\begin{align*}
\tau(\phi) &= -2e_{4} ; \quad  \lambda^2 = (x^4)^2 ; \quad \Delta \lambda^2 = -2 (x^4)^2 ; \\
\langle d\phi , \tau(\phi) \rangle &= -2 e_{4} ; \quad \operatorname{div} \langle d\phi , \tau(\phi)
\rangle = 6 ,
\end{align*}

\begin{align*}
\nabla^{g}_{e_{i}}e_{j} &= \nabla^{ds^2}_{e_{i}}e_{j} + e_{i}(\rho)e_{j} + e_{j}(\rho)e_{i} - \langle
e_{i},e_{j} \rangle \operatorname{grad} \rho  = - \epsilon x^j e_{i} + \delta_{ij} \epsilon X
\end{align*}

\begin{align*}
&\operatorname{grad}^{g} \ln\lambda = \tfrac{(1+\epsilon |x|^2)^2}{4}\tfrac{\partial}{\partial x^i}
(\ln\lambda) \tfrac{\partial}{\partial x^i} =  \epsilon X ;\\
&|\operatorname{grad}^g \ln\lambda|_{g}^{2} = \tfrac{4}{(1+\epsilon |x|^2)^2} \tfrac{(1+\epsilon |x|^2)^2}{4} |x|^2 = |x|^2 ;\\
&\operatorname{grad}^g |\operatorname{grad}^g \ln\lambda|_{g}^{2} =\tfrac{(1+\epsilon |x|^2)^2}{4}
\tfrac{\partial}{\partial x^i} (|x|^2) \tfrac{\partial}{\partial x^i}
=(1+\epsilon |x|^2) X .
\end{align*}

\begin{align*}
& \sum_{i=1}^{n} \nabla^{g}_{e_{i}}e_{i} = (n-1) \epsilon X ; \quad  X(\ln \lambda) =
\epsilon |x|^2 ; \quad
\sum_{i=1}^{n} (\nabla^{g}_{e_{i}}e_{i}) (\ln \lambda) = (n-1) |x|^2 ;\\
&e_{i} (\ln\lambda) = \epsilon x^i ;\quad  e_{i}(e_{i} (\ln\lambda)) = \epsilon
\tfrac{1+\epsilon |x|^2}{2} ,
\end{align*}

$$\Delta \operatorname{grad}^g \ln\lambda = - \sum_{i=1}^{n} \nabla^{g}_{e_{i}}\nabla^{g}_{e_{i}} (\operatorname{grad}^g \ln\lambda)
 - \nabla^{g}_{\nabla^{g}_{e_{i}}e_{i}} (\operatorname{grad}^g \ln\lambda) , $$

\begin{align*}
& - \sum_{i=1}^{n} \nabla^{g}_{\nabla^{g}_{e_{i}}e_{i}} (\operatorname{grad}^g \ln\lambda) = -
\nabla^{g}_{(n-1) \epsilon X} (\epsilon X)
= - (n-1) \tfrac{1+\epsilon |x|^2}{2} X ;\\
&\nabla^{g}_{e_{i}} (\operatorname{grad}^g \ln\lambda)  = \epsilon (\tfrac{1-\epsilon |x|^2}{2} e_i + \epsilon x^i X) ;\\
&\nabla^{g}_{e_{i}}\nabla^{g}_{e_{i}} (\operatorname{grad}^g \ln\lambda) = - \tfrac{1 + \epsilon |x|^2}{2} x^i e_i + (1+ \epsilon (x^i)^2)X ;\\
&\sum_{i=1}^{n} \nabla^{g}_{e_{i}}\nabla^{g}_{e_{i}} (\operatorname{grad}^g \ln\lambda) = \tfrac{2n-1
+ \epsilon |x|^2}{2} X,
\end{align*}

$$- \Delta \operatorname{grad}^g \ln\lambda = \tfrac{n + (2-n)\epsilon |x|^2}{2} X.$$

$$ (2 + (4-n)\epsilon|x|^2) X =0,$$

\begin{align*}
\phi  : ( {{\mathbb R}} \times M^2 , g= \beta^2 dt^2 + \lambda^{-2} h) &\to (M^2 ,h) \\
(t,x) &\mapsto x
\end{align*}

\begin{align}\label{2D}
0 &= -\lambda^4 \operatorname{grad}_{h} (\Delta_{h} \ln\beta)  - 2\lambda^4 G_{h} \operatorname{grad}_{h} \ln\beta +
\tfrac{3}{2} V(\lambda^2|\operatorname{grad}_{h}\ln \beta|^2) V\\\notag &- \lambda^4|\operatorname{grad}_{h}\ln
\beta|^2 \operatorname{grad}_{h}\ln \beta - \nabla_{V}\nabla_{V} [\lambda^2 \operatorname{grad}_{h}\ln \beta] -
\tfrac{\lambda^{4}}{2} \operatorname{grad}_{h} |\operatorname{grad}_{h} \ln\beta|_{h}^{2} \\\notag & - \lambda^2
V(V(\ln\lambda)\operatorname{grad}_h \ln\beta - 2V(\ln\lambda)[\nabla_{V} (\lambda^2 \operatorname{grad}_{h}\ln \beta)
- \lambda^2 |\operatorname{grad}_h \ln\beta |_{h}^2 V].
\end{align}

$$f(x) = \frac{-c_1 (1+e^{c_1 x})}{1-e^{c_1 x}}$$

\begin{align*}
\phi : ({{\mathbb R}}^2 \times {{\mathbb R}} , dx^2 + dy^2 + \beta^2(x) dz^2) &\to ({{\mathbb R}}^2 , dx^2 + dy^2)\\
\phi(x,y,z) &= (x,y)
\end{align*}

$$A_{E}F = g(E^{\mathcal{H}},F^{\mathcal{H}}) V(\ln \lambda) V.$$

$$ B_{V} W = - \lambda^{2} \operatorname{grad}_{h} (\ln\beta) \langle W,V\rangle .$$

\begin{align*}
&[ \operatorname{trace}  ( (\nabla A)^{*}_{\mu} - (\nabla A)\mu + 3 A^{*}_{\nabla \mu} +
(\nabla_{\mu}B^{*})^{*} + 2 B_{\nabla_{\mu}} - B_{\nabla\mu} -2 A^{*}_{\nabla_{\mu}}) + 2 A^{*}_{\mu}\nu ]^{\mathcal{H}} \\
&= V(V(\ln\lambda))\mu + 3(V(\ln\lambda)^2)  \mu -3V(\ln\lambda) V(\lambda
e_{i}(\ln\beta)) \lambda e_{i}  \\
&+ \mu(g(\lambda e_{j},\mu)) \lambda e_{j} + |\mu|^{2} \mu .
\end{align*}

\begin{align*}
[\nabla_{\mu}\mu]^{\mathcal{H}} &=  \tfrac{\lambda^4 }{2} \operatorname{grad}_{h} ( | \operatorname{grad}_{h} \ln\beta |_{h}^{2}) ;\\
[\nabla_{\mu} \nu]^{\mathcal{H}} &= - (V(\ln\lambda))^2 \mu ; \\
  \Delta^{\mathcal{H}} (\ln\lambda) &= -2(V(\ln\lambda))^2 ;\\
[\nabla_{\mu} \operatorname{grad}\ln\lambda]^{\mathcal{H}} & = - (V(\ln\lambda))^2 \mu ;\\
 [\Delta \mu ]^{\mathcal{H}} &= \lambda^4 e_{i}(e_{i}(e_{j}\ln\beta))) e_{j} - (V(\ln\lambda))^2 \operatorname{grad}^{\mathcal{H}} \ln\beta\\
&- V(\ln\lambda) V(\lambda e_{j}(\ln\beta)) \lambda e_{j} +  V(V(\lambda e_{j}(\ln\beta))) \lambda e_{j}\\
& - \lambda^4 |\operatorname{grad}_{h} \ln\beta|_{h}^{2} \operatorname{grad}_{h} \ln\beta 
+ \tfrac{\lambda^4}{2} \operatorname{grad}_{h}(|\operatorname{grad}_{h} \ln\beta|_{h}^{2}) \\
&+ \lambda e_{k}(\ln\beta)\lambda^2 [\nabla_{\lambda e_i}(\nabla^{M^2}_{e_i}e_k)]^{\mathcal{H}} .
\end{align*}

\begin{align*}
0 &= -\lambda^4 e_{i}(e_{i}(e_{j}\ln\beta))) e_{j} - V(V(\lambda e_{j}(\ln\beta)))
\lambda e_{j} - \tfrac{\lambda^{4}}{2} \operatorname{grad}_{h} |\operatorname{grad}_{h} \ln\beta|_{h}^{2}\\
& - \lambda^4 G_{h} \operatorname{grad}_{h} \ln\beta  
- \lambda^2 V(V(\ln\lambda)\operatorname{grad}_h \ln\beta  - 2V(\ln\lambda)V(\lambda e_{i}(\ln\beta))
\lambda e_{i} \\
&- \lambda e_{k}(\ln\beta)\lambda^2 [\nabla_{\lambda
e_i}(\nabla^{M^2}_{e_i}e_k)]^{\mathcal{H}} .
\end{align*}

\begin{align*}
&V(V(\lambda e_{j}(\ln\beta))) \lambda e_{j}  = - \tfrac{3}{2} V(\lambda^2
|\operatorname{grad}_{h}\ln \beta|^2) V + \lambda^4|\operatorname{grad}_{h}\ln \beta|^2 \operatorname{grad}_{h}\ln \beta \\
& + \nabla_{V}\nabla_{V} [\lambda^2 \operatorname{grad}_{h}\ln \beta] ;\\
&V(\lambda e_{j}(\ln\beta)) \lambda e_{j} = \nabla_{V} (\lambda^2 \operatorname{grad}_{h}\ln \beta) - \lambda^2 |\operatorname{grad}_h \ln\beta |_{h}^2 V ;\\
&\operatorname{grad}_{h} (\Delta_{h} \ln\beta) = e_{i}e_{i}e_{j}(\ln\beta)e_{j} - G_h \operatorname{grad}_{h}\ln\beta\\
&- \langle \nabla_{e_{1}}\nabla_{e_{1}}e_{1}+ \nabla_{e_{2}}\nabla_{e_{2}}e_{1}
,e_{2}\rangle e_{2}(\ln\beta)e_{1}
 - \langle \nabla_{e_{1}}\nabla_{e_{1}}e_{2} + \nabla_{e_{2}}\nabla_{e_{2}}e_{2}
,e_{1}\rangle e_{1}(\ln\beta) e_{2} ;\\
& \lambda e_{k}(\ln\beta)\lambda^2 [\nabla_{\lambda e_i}(\nabla^{M^2}_{e_i}e_k)]^{\mathcal{H}}
= -\lambda^4 [ e_{1}(\ln\beta) h(\nabla^{M^2}_{e_1}\nabla^{M^2}_{e_1}e_2
+ \nabla^{M^2}_{e_2}\nabla^{M^2}_{e_2}e_2,e_1) e_2 \\
&+ e_{2}(\ln\beta) h(\nabla^{M^2}_{e_1}\nabla^{M^2}_{e_1}e_1 +
\nabla^{M^2}_{e_2}\nabla^{M^2}_{e_2}e_1,e_2) e_1 ],
\end{align*}

\begin{align*}
\phi : ({{\mathbb R}}^2 \times {{\mathbb R}} , dx^2 + dy^2 + \beta^2(x) dz^2) &\to ({{\mathbb R}}^2 , dx^2 + dy^2)\\
\phi(x,y,z) &= (x,y) ,
\end{align*}

$$ ff' + f'' =0 ,$$

\end{document}