\documentclass[a4paper,12pt]{article}


\usepackage{kv1}

\begin{document}


$$
\exists n \in \bbN \; \forall i,j \; (A^n)_{ij} > 0.
$$

\begin{equation}    \label{e:markov_metric}
d (\om^1, \om^2) = \begin{cases}
2^{-\min\{|n| \, : \, \om_n^1\neq \om_n^2 \}}, &  \om^1 \neq \om^2, \\
0, &   \om^1 = \om^2,
\end{cases}
\qquad \om^1,\om^2 \in \Sigma.
\end{equation}

$$
(\om, x) \mapsto (\sigma \om, f_{\om} (x)),
$$

$$
\dist_\sP (F,G) := \sup_\om (\dist_{C^1} (f_\om^{\pm 1}, g_\om^{\pm 1})).
$$

\begin{equation}    \label{e:vector_p}
\forall i \; p_i \ge 0, \text{ and } \sum_i \pi_{ij} p_i = p_j.
\end{equation}

$$
C_w := \{ \om' \in \Sigma \mid \om_k' = \om_k, \ldots, \om_m' = \om_m \}.
$$

\begin{equation}    \label{e:markov_measure}
\nu(C_w) := p_{\omega_{k}} \cdot \prod\limits_{i=k}^{m-1} \pi_{\omega_{i} \omega_{i+1}}.
\end{equation}

$$
\forall \om \, \forall \eps > 0 \quad \exists \delta > 0 \quad \text{ such that } \quad \dist(\om, \om') < \delta \Rightarrow B_{\om'} \subset U_\eps (B_\om).
$$

$$
\quad \varphi_1(\om) < \varphi_2 (\om).
$$

$$
S_{\varphi_1, \varphi_2} := \{ (\om,x) \mid \varphi_1(\om) \le x \le \varphi_2(\om) \}
$$

\begin{equation}    \label{e:Amax}
A_{\textup{max}}(S_{\varphi_1, \varphi_2}) := \bigcap_{n=0}^{+\infty} F^n (S_{\varphi_1, \varphi_2}).
\end{equation}

$$
\lim\limits_{n\to\infty} \frac{1}{n}\sum_{i=0}^{n-1} \varphi (F^i(p)) = \int\limits_{\Sigma\times I} \varphi \, d\mathbf{m}.
$$

\begin{equation}\label{e:factor}
\begin{CD}
\Sigma @>{\sigma}>> \Sigma \\
@V{\pi}VV            @VV{\pi}V \\
\Sigma_+ @>{\sigma_+}>> \Sigma_+
\end{CD}
\end{equation}

$$
\nu_+ (F_+^{-1} (A)) = \nu_+ (A).
$$

\begin{equation}\label{e:skew-factor}
\begin{CD}
\Sigma \times I @>{F}>> \Sigma \times I \\
@V{\pi\times\Id}VV            @VV{\pi\times\Id}V \\
\Sigma_+ \times I @>{F_+}>> \Sigma_+ \times I,
\end{CD}
\end{equation}

$$
\mathbf{m}_+(A) := \mathbf{m}(\pi^{-1} (A)),
$$

\begin{equation}\label{e:stoch_img}
  (f_* \mu)_j := \sum_i \pi_{ij} \cdot (f_j)_* \mu_i,
\end{equation}

\begin{equation}\label{e:inv_measure}
\mathbf{m}_+ (\mu) := \sum_k \nu_k^+ \times \mu_k,
\end{equation}

$$
\nu_k^+=\frac{\nu_+|_{C_{+,k}}}{\nu_+(C_{+,k})}.
$$

$$
\forall k,m: \, \pi_{km} > 0, \, f_k(D_k) \subset \inter D_m \quad ( \, f_k(D_k) \subset D_m \, ).
$$

$$
\tilde{D}_+=\bigsqcup_k C_{+,k} \times D_k \subset \Sigma_+ \times I
$$

\begin{equation}\label{eq:Ds}
\tilde{D}=\bigsqcup_k C_k \times D_k \subset \Sigma \times I
\end{equation}

$$
f_{w_1 \dots w_n} := f_{w_n}\circ \dots \circ f_{w_1}\colon I_{w_1}\to I_{w_{n+1}},
$$

$$
A_{\mu,k}:= \min\supp \mu_k, \quad B_{\mu,k}:= \max\supp \mu_k.
$$

$$
f_{i} (\supp \mu_i) \subset \supp\mu_j.
$$

\begin{equation}    \label{e:I_k_forw_inv}
f_{i} (I_{\mu,i}) \subset I_{\mu,j}.
\end{equation}

$$
(w_0,x_0),\dots,(w_n,x_n)
$$

$$
(w_0,x_0)=(w'_0,x'_0),\dots,(w'_{n'},x'_{n'}),
$$

$$
w^j=asbsc,
$$

$$
\Phi(D)= \bigsqcup_{m} \left(\bigcup_{k: \, (k,m) \, \text{admissible}} f_k(D\cap I_{k})\right),
$$

\begin{equation}\label{eq:N+1}
\Phi^{N+1}(D) \subset \inter \bigcup_{j=0}^N \Phi^j(D).
\end{equation}

$$
f_{w_1\dots w_{i-1}}(A_{\mu,w_1}-\eps)< G\circ f_{w_1\dots w_{i-1}}(A_{\mu,w_1}-\eps)  = f_{w_1\dots w_{j-1}}(A_{\mu,w_1}-\eps),
$$

$$
f_{w_1\dots w_{i-1}w_j\dots w_N}(A_{\mu,w_1}-\eps)<f_{w_1\dots w_{N}}(A_{\mu,w_1}-\eps).
$$

$$
\Phi_\delta (D) := \overline{U_\delta (\Phi(D))}.
$$

\begin{equation}\label{eq:delta}
\Phi_{\delta}^{N+1}(D) \subset 
\inter \bigcup_{j=0}^N \Phi_{\delta}^j(D).
\end{equation}

$$
\Phi(\Phi_{\delta}^{j}(D))\subset \inter \Phi_{\delta}^{j+1}(D), \quad j=0,\dots N.
$$

$$
\Phi(\tilde{D}_{\delta}) \subset \inter \tilde{D}_\delta,
$$

$$
G_A (I_{\mu,k}) \subset U_\eps (A_{\mu,k'}), \quad G_B (I_{\mu,k}) \subset U_\eps (B_{\mu,k'}).
$$

\begin{equation}    \label{e:n_image}
F^n(\om,x) = (\sigma^n \om, f_{n,\om} (x)).
\end{equation}

$$
f_{n,\om} = f_{\sigma^{n-1}\om} \circ f_{\sigma^{n-2}\om} \circ \ldots \circ f_{\om},\;\text{ and }\;
f_{-n,\om} = f_{\sigma^{-n}\om}^{-1} \circ f_{\sigma^{-n+1}\om}^{-1} \circ \ldots \circ f_{\sigma^{-1}\om}^{-1} = f^{-1}_{n,\sigma^{-n}\om}.
$$

$$
f_{n,\om} = f_{\om_{n-1}} \circ f_{\om_{n-2}} \circ \ldots \circ f_{\om_0},\;\text{ and }\;
f_{-n,\om} = f_{\om_{-n}}^{-1} \circ f_{\om_{-n+1}}^{-1} \circ \ldots \circ f_{\om_{-1}}^{-1}.
$$

$$
\tilde D := \bigsqcup_k C_k \times U_k,
$$

$$
A_\om = \bigcap_{n \ge 0} A_\om^{(n)},
$$

$$
A_\om^{(n)} = f_{-1} \circ \dots \circ f_{\om_{-n}} (\tilde D_{\sigma^{-n} \om}).
$$

$$
\om_{-n}' = \om_{-n}, \dots, \om_{-1}' = \om_{-1},
$$

$$
\Om_{k,x} \subset \bigsqcup_{s \ne w} \left\{ \om_{[-L,-1]} = s \right\}.
$$

$$
\left\{ \om_{[-L,-1]} = s \right\} = \bigsqcup_{s'} \left\{ \om_{[-2L,-1]} = s's \right\}.
$$

\begin{equation}\label{e:next_cyl}
\Om_{k,x} \cap \left\{ \om_{[-L,-1]} = s \right\} \subset \bigsqcup_{s' \ne w'} \left\{ \om_{[-2L,-1]} = s's \right\}.
\end{equation}

$$
wC := \left\{ \om_{[n_1 - L, n_2]} = wu \right\},
$$

$$
  \frac{\nu(wC)}{\nu(C)} > \lambda.
  $$

$$
\theta_n:=\frac{1}{n} \sum_{j=0}^{n-1} \delta_{F^j(\om,x)}.
$$

\begin{equation}\label{e:stoch_img_2}
  \sum_i \pi_{ij}  \cdot \bbE (\xi_{ij})_* \mu_i = \mu_j,
\end{equation}

\begin{equation}\label{e:lognorm}
\bbE \log \norm{D\xi_{ij}} < +\infty.
\end{equation}

\begin{equation}\label{e:lyap-vol}
    \lambda_{vol} = \sum_{i,j} \pi_{ij} \cdot \bbE \int_M \log \Jac \xi_{ij}|_x d\mu_i(x).
\end{equation}

$$
    \forall i,j \quad (\xi_{ij})_* \nu_i = \nu_j \quad \text{with the probability~}.
  $$

\begin{equation}\label{e:rel-entropy}
h(m_1|m_2) := \sup_{\psi \in C(X)} \left[ \log \int e^\psi \,dm_1 - \int \psi \,dm_2 \right] =
\left\{
  \begin{array}{ll}
    \int \left( \log \frac{dm_1}{dm_2} \right) \,dm_1, & \hbox{if ;}   \\
    +\infty, & \hbox{otherwise.}
  \end{array}
\right.
\end{equation}

\begin{equation}\label{e:lyap-vol-entropy}
    \lambda_{vol}(\mu) = -\sum \pi_{ij} \cdot \bbE h ((\xi_{ij})_* \mu_i | \mu_j).
\end{equation}

\begin{multline}\label{e:lyap-rel}
h ((\xi_{ij})_* \mu_i | \mu_j) = \int_{M_j} \log \left. \frac{d (\xi_{ij})_* \mu_i}{d\mu_j}\right|_{y}  \, d (\xi_{ij})_* \mu_i(y)= \int_{M_i} \log \left(\frac {\rho_{\mu_j}(\xi_{ij}(x))}{(\Jac \xi_{ij})(x) \cdot \rho_{\mu_i}(x)}\right) \, d \mu_i(x)=
\\
= -  \int_{M_i} \log \Jac \xi_{ij}|_{x}  \, d \mu_i(x) + \left(
\int_{M_i} \log \left({\rho_{\mu_j}(\xi_{ij}(x))}\right) \, d \mu_i(x) -
\int_{M_i} \log \left({\rho_{\mu_i}(x)}\right) \, d \mu_i(x)\right).
\end{multline}

\begin{multline}\label{e:lyap-corr}
\sum_{i,j} \pi_{ij} \bbE \int_{M_i} \log \rho_{\mu_j}(\xi_{ij}(x))\, d\mu_i(x)  -  \sum_{i,j} \pi_{ij} \bbE \int_{M_i} \log \rho_{\mu_i}(x) \,d\mu_i(x) = \\
=\sum_{j} \int_{M_j} \log \rho_{\mu_j}(y)\, d\left(\sum_i \pi_{ij} \bbE (\xi_{ij})_{*} \mu_i\right)(y)   -  \sum_{i} \int_{M_i} \log \rho_{\mu_i}(x) \,d\mu_i(x) = 0.
\end{multline}

$$
\lambda_{vol}(\mu^{\eps}; \Pi^{\eps})=-\sum_{i,j} \pi_{ij} \cdot \bbE h ((\xi_{ij}^{\eps})_* \mu^{\eps}_i | \mu^{\eps}_j) \le 0,
$$

$$
\sum_{i,j} \pi_{ij} \int \log \Jac \xi_{ij}|_x \, d\mu_i(x) = \lim_{n \to \infty} \sum_{i,j} \pi_{ij} \int \log \Jac \xi_{ij}^\eps|_x \, d\mu_i^\eps(x) = -\alpha < 0,
$$

$$
\lambda_{vol} (\tilde{\mu})= \sum_{i,j} \pi_{ij} \int \log \Jac \xi_{ij}|_x \, d\mu_i(x) \le -\alpha < 0.
$$

$$
\forall i \in \bbZ, \ \forall \om = \om_{[-\infty, -1]} \om_{[0, +\infty]}, \om' = \om_{[-\infty, -1]} \om_{[0, +\infty]}', \quad \varphi_{+\infty} (\om) = \varphi_{+\infty} (\om');
$$

$$
\varphi_{+\infty} (\sigma \om) = f_{\om} (\varphi_{+\infty} (\om)).
$$

$$
\varphi_n(\om) = f_{n, \sigma^{-n}\om} (\varphi (\sigma^{-n} \om)).
$$

\end{document}