\documentclass[a4paper,12pt]{article}


\usepackage{amssymb,color}

\begin{document}


\begin{align*}\Lambda^m &:= \{\lambda \in \Lambda : d(\lambda) = m\} \quad\text{and}\quad \Lambda^{\neq 0}:= \Lambda \setminus \Lambda^0,\\
 v \Lambda &:= \{\lambda \in \Lambda : r(\lambda) = v\} \quad\text{(this is denoted   in \cite{RSY03})},\\
v \Lambda^m &:= \Lambda^m \cap v\Lambda.
\end{align*}

\[\Omega_{k,m}:= \{(p,q) \in {\mathbb{N}}^k \times {\mathbb{N}}^k :  p \leq q \leq m \}.
 \]

\[\Omega_{k,m}^0 =\{p \in {\mathbb{N}}^k \mid p \leq m\},\]

\begin{equation*}
\Lambda^{\leq n}:=\{\lambda\in\Lambda: d(\lambda)\leq n, \text{\ and\ }d(\lambda)_i<n_i \text{\ implies\ }s(\lambda)\Lambda^{e_i}=\emptyset\},
\end{equation*}

\[
v\Lambda^{\leq e_i} = \begin{cases} v\Lambda^{e_i} & \text{ if }v\Lambda^{e_i} \neq \emptyset;\\
 \{v\} & \text{ otherwise.}\end{cases}
\]

\begin{equation}
 \label{eq:boundarypath}
v \in  \Omega_{k,m}^0 \text{ and }  v\Omega_{k,m}^{\leq e_i} = \{v\} \text{ imply }
x(v)\Lambda^{\leq e_i} = \{x(v)\}.
\end{equation}

\[
 d(\lambda^*) = -d(\lambda),\quad r(\lambda^*) = s(\lambda) \quad\text{ and }\quad s(\lambda^*)=r(\lambda).
\]

\[
S_{\lambda}S_{\mu} = S_{\lambda\mu}, \; S_{\mu^*}S_{\lambda^*} = S_{(\lambda\mu)^*}, \;
 P_{r(\lambda)}S_{\lambda} = S_{\lambda} = S_{\lambda}P_{s(\lambda)}, \;
  P_{s(\lambda)}S_{\lambda^*} = S_{\lambda^*} = S_{\lambda^*}P_{r(\lambda)},
\]

\[
S_{\lambda^*}S_{\mu} = \delta_{\lambda,\mu}P_{s(\lambda)},
\]

\[
P_v = \sum_{\lambda\in v\Lambda^n} S_{\lambda}S_{\lambda^*}.
\]

\begin{equation}\label{eq-span}
S_{\lambda^*}S_{\mu} = \sum_{d(\lambda\alpha)=n,\;\lambda\alpha = \mu\beta}S_{\alpha}S_{\beta^*}.
\end{equation}

\[S_{\lambda^{*}}S_\mu=\delta_{\lambda,\mu}P_{s(\lambda)};\]

\begin{equation*}
P_v=\sum_{\lambda \in v\Lambda^{\leq n}}S_\lambda S_{\lambda^{*}}.
\end{equation*}

\[
S_{\lambda^{*}}S_\mu=\sum_{\lambda\alpha=\mu\beta, 
\lambda\alpha \in \Lambda^{\leq n}} S_\alpha S_{\beta^{*}}.
\]

\begin{align*}
S_{\lambda^{*}}S_\mu &= (P_{s(\lambda)}S_{\lambda^{*}})(S_\mu P_{s(\mu)})
 \quad  \text{ by (KP2)}\\
&=\Big( \sum_{\alpha \in s(\lambda)\Lambda^{\leq n-d(\lambda)}}
 S_\alpha S_{\alpha^{*}}\Big)S_{\lambda^{*}}S_\mu \Big( \sum_{\beta 
\in s(\mu)\Lambda^{\leq n-d(\mu)}} S_\beta S_{\beta^{*}}\Big) \quad \text{ by (KP4)}\\
&= \sum_{\alpha \in s(\lambda)\Lambda^{\leq n-d(\lambda)}} \sum_{\beta \in s(\mu)\Lambda^{\leq n-d(\mu)}} 
S_\alpha S_{(\lambda\alpha)^{*}}
S_{\mu\beta} S_{\beta^{*}} \quad \text{ by (KP2)}
\\
&= \sum_{\alpha \in s(\lambda)\Lambda^{\leq n-d(\lambda)}} 
\sum_{\beta \in s(\mu)\Lambda^{\leq n-d(\mu)},\lambda\alpha=\mu\beta}S_\alpha P_{s(\mu\beta)} S_{\beta^{*}}
\intertext{by applying  (KP3) to each summand. By unique factorisation, for each  there is just one  of the given degree such that , and the sums collapse to}
&= \sum_{\alpha \in s(\lambda)\Lambda^{\leq n-d(\lambda)}, \lambda\alpha=\mu\beta} 
S_\alpha  S_{\beta^{*}}
\end{align*}

\[
\Lambda^{\min}(\lambda,\mu):=\{ (\alpha,\beta): \lambda\alpha=\mu\beta, d(\lambda\alpha)=d(\lambda)\vee d(\mu)\}.
\]

\begin{equation}\label{KP3'alt}
S_{\lambda^{*}}S_\mu=\sum_{(\alpha,\beta)\in\Lambda^{\min}(\lambda,\mu)}
S_\alpha S_{\beta^{*}}.
\end{equation}

\[
\Lambda^{\min}(\lambda,\mu)=\begin{cases} 
\{(s(\lambda), s(\lambda))\}&\text{if ;}
\\
\emptyset&\text{else,} \end{cases}
\]

\begin{align*}
\Lambda^{\min}(\lambda,\mu)&=\{(s(\lambda),\beta):\lambda=\mu\beta, d(\lambda)=d(\lambda)\vee d(\mu)\}\\
&=\{(s(\lambda),\beta):\lambda=\mu\beta, d(\mu)< d(\lambda)\}
\end{align*}

\begin{align*} f_v(x)&=
     \begin{cases}
      x & \text{if ;}\\
      0 & \text{otherwise,}
     \end{cases}\\
f_\lambda(x)&=
     \begin{cases}
      \lambda x & \text{if ;}\\
      0 & \text{ otherwise,}
     \end{cases}\\
f_{\mu^{*}}(x)&=
     \begin{cases}
      y & \text{if  for some ;}\\
      0 & \text{ otherwise.}
     \end{cases}
\end{align*}

\begin{equation*}
 S_{\lambda^*}S_{\mu}(x) 
= \begin{cases}
     S_{\lambda^*}(\mu x) & \text{if } x(0)=s(\mu) \text{ and  for some }
;\\
0&\text{otherwise}.
   \end{cases}
\end{equation*}

\begin{align*}
 S_{\lambda^*}S_{\mu}(x) 
&= \begin{cases}
     x & \text{if } x(0)=s(\mu) \text{ and }
 \lambda = \mu;\\
0&\text{otherwise},
   \end{cases}
\\
&= \delta_{\lambda,\mu}P_{s(\lambda)}(x)
\end{align*}

\begin{align*}
 \sum_{\lambda \in v\Lambda^{e_i}}S_{\lambda} S_{\lambda^{*}} (x)
= \sum_{\lambda \in v\Lambda^{e_i}} \delta_{\lambda,x(0,e_i)}x
&= \begin{cases}
    x& \text{if } r(x) =v;\\
0&\text{otherwise},
   \end{cases}\\
&= P_v(x).\qedhere
\end{align*}

\[\operatorname{KP}_R(\Lambda)_n := {\operatorname{\mathrm{span}}}\{s_\alpha s_{\beta^{*}}: d(\alpha)-d(\beta)=n\}\]

\[{\mathbb{F}}_R(w(X))_n:=\Big\{ \sum_{w \in w(X)} r_w w: r_w \neq 0 \implies d(w)=n \Big\}.\]

\[
({\mathbb{F}}_R(w(X))/I)_n:={\operatorname{\mathrm{span}}} \{ q(w):w\in w(X),  d(w)=n \}.
\]

\[
\operatorname{KP}_R(\Lambda)_n :=  {\operatorname{\mathrm{span}}}\{s_\alpha s_{\beta^{*}}: d(\alpha)-d(\beta)=n\}=({\mathbb{F}}_R(w(X))/I)_n.
\]

\begin{align*}
& q(\lambda\mu^*)=s_\lambda s_{\mu^*}\text{\ and \ } d(\lambda)-d(\mu)=d(\lambda\mu^*),\\
& q(\lambda\mu)=s_{\lambda\mu} s_{s(\mu)^*}\text{\ and \ } d(\lambda\mu)-d(s(\mu))=d(\lambda\mu),\\
& q(\mu^*\lambda^*)=s_{s(\mu)}s_{(\lambda\mu)^*}\text{\ and \ } d(s(\mu))-d((\lambda\mu)^*)=d(\mu^*\lambda^*).
 \end{align*}

\[
 q(\lambda^*\mu)=s_{\lambda^{*}}s_\mu=\sum_{\lambda\alpha=\mu\beta, 
\lambda\alpha \in \Lambda^{\leq m}} s_\alpha s_{\beta^{*}}.
 \]

\[
q(w)=s_{w_1}\cdots s_{w_{i-1}}s_{\lambda}s_{\mu}s_{w_{i+2}}\cdots s_{w_{n+1}}
=s_{w_1}\cdots s_{w_{i-1}}s_{\lambda\mu}s_{w_{i+2}}\cdots s_{w_{n+1}}=q(w').
\]

\begin{equation}\label{eq:aperiodic}
\text{for every , there exists 
such that   implies .}
\end{equation}

\[ a = \sum_{(\alpha, \beta) \in F} r_{\alpha, \beta}s_\alpha s_{\beta^{*}}\]

\[a=\sum_{(\mu,\nu) \in G} r_{\mu,\nu}s_\mu s_{\nu^{*}},\]

\[
s_\mu s_{\nu^{*}} = s_\mu p_{s(\mu)} s_{\nu^{*}}=s_\mu\Big(\sum_{\lambda \in s(\mu)\Lambda^{\leq n-d(\nu)}} s_\lambda s_{\lambda^{*}}\Big) s_{\nu{*}}=\sum_{\lambda \in s(\mu)\Lambda^{\leq n-d(\nu)}}s_{\mu\lambda} s_{(\nu\lambda)^{*}}.
\]

\begin{equation}\label{eq:4.2}
0 \neq s_{\mu^*}as_\nu = r_{\mu,\nu}p_{s(\mu)}+\sum_{(\alpha,\nu)\in F, d(\alpha)\neq d(\mu)} 
r_{\alpha,\nu}s_{\mu^*}s_\alpha,\end{equation}

\begin{align*}
s_{\mu^*}as_\nu 
&=\sum_{(\alpha,\beta) \in F} r_{\alpha,\beta}s_{\mu^*}s_\alpha s_{\beta^*} s_\nu 
=\sum_{(\alpha,\nu) \in F} r_{\alpha,\nu}s_{\mu^*}s_\alpha p_{s(\nu)}\\
&= r_{\mu,\nu}p_{s(\mu)}+\sum_{(\alpha,\nu) \in F, \alpha\neq\mu } r_{\alpha,\nu}s_{\mu^*}s_\alpha
\end{align*}

\[
s_{\mu^*}as_\nu = r_{\mu,\nu}p_{s(\mu)}+\sum_{(\alpha,\nu)\in F, d(\alpha)\neq d(\mu)} r_{\alpha,\nu}s_{\mu^*}s_\alpha.
\]

\[
0 \neq s_{\mu^*}as_\nu = r_{\mu,\nu}p_{s(\mu)}+\sum_{(\alpha,\nu)\in F, d(\alpha)\neq d(\mu)} 
r_{\alpha,\nu}s_{\mu^*}s_\alpha
\]

\[A:={\operatorname{\mathrm{span}}} \{t_{\lambda}t_{\mu}^*:\lambda, \mu \in \Lambda\}\]

\[
 A_n:= {\operatorname{\mathrm{span}}}\{t_{\lambda}t_{\mu}^*:d(\lambda)- d(\mu)=n\}\quad(n\in{\mathbb{Z}}^k)\]

\begin{equation}
\label{eq:Lem4.4}
0 \neq s_{\mu^*}as_\nu = r_{\mu,\nu}p_{s(\mu)}+\sum_{(\alpha,\nu)\in F, d(\alpha)\neq d(\mu)} 
r_{\alpha,\nu}s_{\mu^*}s_\alpha.
\end{equation}

\[m_\alpha=m \wedge m_{\alpha} \leq m \wedge (d(y) + d(\alpha)) \leq m \wedge d(y) + d(\alpha);
\]

\begin{align*}
s_{y(0,m\wedge d(y))^*}&(s_{\mu^*}as_\nu)s_{y(0,m\wedge d(y))}\\
&=r_{\mu,\nu}s_{y(0,m\wedge d(y))^*}p_{s(\mu)}s_{y(0,m\wedge d(y))} + 
\sum_{\alpha \in G}r_{\alpha,\nu}s_{y(0,m\wedge d(y))^*}s_{\mu^*}s_\alpha s_{y(0,m\wedge d(y))}\\
&=r_{\mu,\nu}p_{s(\mu)}+ \sum_{\{\alpha \in G: \alpha \neq \mu\}} 
r_{\alpha,\nu}s_{(\mu y(0,m\wedge d(y)))^*}s_{\alpha y(0,m\wedge d(y))} \\
\intertext{because  and (KP2), and then (KP3), all on the first summand. After composing paths this}
&=r_{\mu,\nu}p_{s(\mu)}+ \sum_{\alpha \in G}
 r_{\alpha,\nu}s_{(\mu y)(0,m\wedge d(y)+d(\mu))^*}s_{(\alpha y)(0,m\wedge d(y)+d(\alpha))}.
\end{align*}

\[s_{(\mu y)(0,m\wedge d(y)+d(\mu))^*}s_{(\alpha y)(0,m\wedge d(y)+d(\alpha))} \neq 0.\]

\[s_{y(0,m\wedge d(y))^*}(s_{\mu^*}as_\nu)s_{y(0,m\wedge d(y))}=r_{\mu,\nu}p_{s(\mu)}.\]

\[
 r(\lambda)\Lambda^n \setminus \{\lambda(0,n)\} \text{ and }  s(\lambda)\Lambda^n \setminus \{\lambda(d(\lambda)-n,d(\lambda))\}
\]

\begin{equation}\label{3.1}
\ \hfill
\parbox{0.9\textwidth}{
 contains no cycles and each vertex 
is the range of an isolated cycle in .
}\end{equation}

\begin{equation}\label{mu}
s_\alpha s_{\beta^*}=s_\alpha p_{s(\alpha)}s_{\beta^*}=s_\alpha\sum_{\lambda\in s(\alpha)\Lambda^{\leq(0,n_2)}}s_\lambda s_{\lambda^*}s_{\beta^*}=s_{\alpha\nu}s_{(\beta\nu)^*}.
\end{equation}

\begin{align*}
p_{\dagger}\operatorname{KP}_R(\Lambda)p_{\dagger}&={\operatorname{\mathrm{span}}}\{s_\alpha s_{\beta^*}: \alpha,\beta\in\Lambda^{{\operatorname{\mathrm{red}}}}, s(\alpha)=s(\beta), r(\alpha)=r(\beta)=\dagger\}\\
&={\operatorname{\mathrm{span}}}\{s_{\mu^i} s_{(\mu^j)^*}:i,j\in{\mathbb{N}}\} \quad\text{(using \eqref{mu})}\\
&={\operatorname{\mathrm{span}}}\{s_{\mu^i}, s_{(\mu^i)^*}:i\in{\mathbb{N}}\}\quad\text{(since )}.
\end{align*}

\[\pi\circ\rho^{-1}(1)=p_\dagger, \pi\circ\rho^{-1}(x)=s_\mu \text{ and } \pi\circ\rho^{-1}(x^{-1})=s_{\mu^*}.\]

\begin{equation}\label{matrixunits}
 \theta(\alpha,\beta):=\begin{cases}s_\alpha s_{\nu(\alpha,\beta)}s_{\beta^*}  
 &\text{if };\\
 s_\alpha s_{\nu(\alpha,\beta)^*}s_{\beta^*}  &\text{if }
 \end{cases}
 \end{equation}

\begin{align*}\sum_{\alpha\in Y} \theta(\alpha,\alpha)&=\sum_{\alpha\in Y} s_\alpha s_{\alpha^*}=\sum_{v\in\Lambda^0}\sum_{\alpha\in vY}s_\alpha s_{\alpha^*}
=\sum_{v\in\Lambda^0}\sum_{\alpha\in v\Lambda^{\leq (n_1,0)}}s_\alpha s_{\alpha^*}=\sum_{v\in\Lambda^0}p_v=1.
\end{align*}

\[
T_{\lambda^*}T_\mu=T_{\lambda^*}Q_{r(\lambda)}Q_{r(\mu)}T_\mu=\delta_{r(\lambda), r(\mu)}T_{\lambda^*}T_\mu,\]

\[Q_v=p_v=\sum_{\lambda\in v\Lambda^{e_i}}s_\lambda s_{\lambda^*}= \sum_{\lambda\in v\Lambda_N^{e_i}}s_\lambda s_{\lambda^*}.\]

\[C_{n,i}:={\operatorname{\mathrm{span}}}\{t_\mu t_{\nu^*}:\mu,\nu\in\Lambda_N, s(\mu)=s(\nu)\in V_{N,i}\}\]

\[Q_v=P_iq_v P_i, T_\mu=P_i t_\mu P_i \text {and } T_{\mu^*}=P_i t_{\mu^*} P_i.\]

\begin{align*}
P_i^2&=\sum_{v,w \in V}\sum_{\alpha\in v\Lambda^{{\operatorname{\mathrm{blue}}}} V_{N,i}}\sum_{\beta\in w\Lambda^{{\operatorname{\mathrm{blue}}}} V_{N,i}}t_\alpha t_{\alpha^*}q_v q_w t_\beta t_{\beta^*}
=\sum_{v \in V}\sum_{\alpha,\beta\in v\Lambda^{{\operatorname{\mathrm{blue}}}} V_{N,i}}t_\alpha t_{\alpha^*}t_\beta t_{\beta^*}\\
&=\sum_{v \in V}\sum_{\alpha\in v\Lambda^{{\operatorname{\mathrm{blue}}}} V_{N,i}}t_\alpha t_{\alpha^*}t_\alpha t_{\alpha^*}=P_i.
\end{align*}

\begin{align*}
P_it_\mu P_i&=\sum_{\alpha,\beta\in\Lambda^\blueV_{N,i}} t_\alpha t_{\alpha^*}t_\mu t_\beta t_{\beta^*}
=\sum_{\alpha\in r(\mu)\Lambda^\blueV_{N,i}}\sum_{\beta\in s(\mu)\Lambda^\blueV_{N,i}} t_\alpha t_{\alpha^*}t_{\mu \beta} t_{\beta^*}\\
&=\sum_{\beta\in s(\mu)\Lambda^\blueV_{N,i}} t_{\mu \beta} t_{\beta^*}
\quad\text{(by KP3 because such  must have )}\\
&=t_\mu P_i.
\end{align*}

\[
Q_vQ_w=P_iq_vP_i^2q_wP_i=P_i^3q_vq_wP_i=\delta_{v,w}P_iq_vP_i=\delta_{v,w}Q_v.
\]

\[
T_\lambda T_\mu=P_it_\lambda P_i^2 t_\mu P_i=P_it_\lambda t_\mu P_i=P_i t_{\lambda\mu}P_i=T_{\lambda\mu},
\]

\begin{align*}
T_{\lambda^*}T_\mu&=P_i t_{\lambda^*}P_it_\mu P_i=P_i t_{\lambda^*}t_\mu P_i\\
&=\delta_{\lambda,\mu}P_i q_{s(\mu)} P_i \quad\text{(because )}\\
&=\delta_{\lambda,\mu}Q_{s(\mu)}.
\end{align*}

\begin{align*}
\sum_{\lambda\in v\Lambda_{N,i}^{\leq n}} T_\lambda T_{\lambda^*}
&=\sum_{\lambda\in v\Lambda_{N,i}^{\leq n}} P_it_\lambda P_i^2 t_{\lambda^*}P_i=\sum_{\lambda\in v\Lambda_{N,i}^{\leq n}} P_it_\lambda  t_{\lambda^*}P_i\\
&=P_i\Big( \sum_{\lambda\in v\Lambda_{N,i}^{\leq n}} t_\lambda  t_{\lambda^*} \Big)P_i
=P_i\Big( \sum_{\beta\in v\Lambda_{N,i}^{\leq (n_1+N, n_2)}} t_\beta\ t_{\beta^*} \Big)P_i\\
&=P_iq_vP_i=Q_v.
\end{align*}

\begin{align*}{\operatorname{\mathrm{span}}}\{P_i t_\mu P_i t_{\nu^*}P_i:\lambda,\mu\in \Lambda_N\}&={\operatorname{\mathrm{span}}}\{P_i t_\mu P_i t_{\nu^*}P_i: s(\mu)=s(\nu)\in V_{N,i}, r(\mu), r(\nu)\in V\}, \end{align*}

\[w\mapsto \big( \theta(\dagger, \alpha)w\theta(\beta,\dagger )\big)_{\alpha,\beta\in Y}\]

\[\theta(\dagger,\alpha)PwP\theta(\beta,\dagger)=\begin{cases} \theta(\dagger,\alpha)w\theta(\beta,\dagger)&\text{if ;}\\0&\text{else}. \end{cases}\]

\[\theta(\dagger,\alpha)P\operatorname{KP}_R(\Lambda_N)P\theta(\beta,\dagger)=\theta(\dagger,\alpha)\operatorname{KP}_R(\Lambda_N)\theta(\beta,\dagger)=p_\dagger\operatorname{KP}_R(\Lambda_N)p_\dagger.\]

\[p=p_1+p_2,  \ x \in pRp_1,\   y \in p_1Rp,\ p=xy \text{ and } \ p_1=yx.\]

\begin{equation}\label{infinrels}
p=p_1+p_2,\quad p_1p_2=p_2p_1=0,\quad xy=p\quad \text{and}\quad yx=p_1.
\end{equation}

\[\operatorname{KP}_K(\Lambda_N)={\operatorname{\mathrm{span}}}\{t_\lambda t_{\mu^*}:s(\lambda)=s(\mu)\in V_N\}.\]

\[
C_{N,i}:={\operatorname{\mathrm{span}}}\{t_\lambda t_{\mu^*}:s(\lambda)=s(\mu)\in V_{N,i}\},
\]

\[Q_0\operatorname{KP}_K(\Lambda_N)Q_0=\bigoplus_i Q_0C_{N,i}Q_0.\]

\[
q=q_1+q_2,\quad q_1q_2=q_2q_1=0,\quad fg=q\quad \text{and}\quad gf=q_1.
\]

\[V_\Lambda:=\{(x;m):x \in \Lambda^{\leq \infty}, m \in {\mathbb{N}}^k\}\text{\ and\ }P_\Lambda:=\{(x;(m,n)):
x \in \Lambda^{\leq \infty}, m \leq n \in {\mathbb{N}}^k\};\]

\begin{align*}
&{\tilde{\Lambda}}^0 := V_\Lambda/\!\!\approx \text{\ and\ }{\tilde{\Lambda}} := P_{\Lambda}/\!\!\sim, \\
&r,s:{\tilde{\Lambda}} \to {\tilde{\Lambda}}^0  \text{ by } 
r([x;(m,n)]) = [x;m] \text{ and }
 s([x;(m,n)]) = [x;n],\\
&\operatorname{id}([x;m])=[x;(m,m)],\\
&[x;(m,n)] \circ [y;(p,q)] = [x(0,n \wedge d(x))\sigma^{p \wedge d(y)}(y);(m,n+p-q)],
\text{ and}\\
&d:{\tilde{\Lambda}} \to {\mathbb{N}}^k \text{ by } 
d(v) = 0 \text{ for all } v \in {\tilde{\Lambda}}^0 \text{ and }
d([x;(m,n)]) = n-m. 
\end{align*}

\begin{align*}
 z(m \wedge d(z),n \wedge d(z)) &= z(m,n \wedge d(z))= \sigma^m(z)(0, n \wedge d(z)-m)\\
&= x(0, n \wedge d(z)-m)= x(0, (n-m) \wedge d(x))
\end{align*}

\[
 \lambda = [y;(0,n)],
\mu = [x;(0,n)] \text{ and }
[x,0]=[y,0] = v.\]

\[ \pi(\lambda) = [y; (0, n \wedge d(y))] \text{ and }\\
\pi(\mu) = [x;(0, n \wedge d(x))].
\]

\[\iota(\Lambda)^{\min}(\iota(\lambda),\iota(\mu))
 \subseteq \tilde\Lambda^{\min}(\iota(\lambda),\iota(\mu)).\]

\[\iota(\lambda)\alpha = \iota(\mu)\beta = [z;(0,d(\lambda) \vee d(\mu))]\]

\[
    (\iota(\lambda)\alpha)(0,d(\lambda)) = \iota(\lambda) = [z;(0,d(\lambda))]
   \]

\[\tilde\Lambda^{\min}(\iota(\lambda),\iota(\mu)) \subseteq \iota(\Lambda)^{\min}(\iota(\lambda),\iota(\mu))\]

\begin{equation*}\label{eq-kp4alt}q_{\iota(v)} = \sum_{\lambda \in v\Lambda^{e_i}} t_{\iota(\lambda)}t_{\iota(\lambda)^*}.
\end{equation*}

\begin{align*}
q_{\iota(v)}&= \sum_{\mu \in \iota(v) {\tilde{\Lambda}}^{e_i}} t_\mu t_{\mu^*} 
\quad \text{by (KP4) for ,}\\
&= \sum_{\lambda \in v\Lambda^{e_i}} t_{\iota(\lambda)}t_{\iota(\lambda)^*}.
\end{align*}

\begin{align*}
t_{\iota(\lambda)^{*}}t_{\iota(\mu)}=
\sum_{(\sigma,\tau)\in\tilde\Lambda^{\min}(\iota(\lambda),\iota(\mu))}
t_{\sigma} t_{\tau^*} \text{\quad by \eqref{eq-span}}\\
=\sum_{(\alpha,\beta)\in\Lambda^{\min}(\lambda,\mu)}
t_{\iota(\alpha)} t_{\iota(\beta)^*} \text{\quad by Lemma~\ref{lem-minextensions}.}
\end{align*}

\[B(\tilde\Lambda) = {\operatorname{\mathrm{span}}}\{t_{\alpha}t_{\beta^*} : \alpha, \beta \in \tilde{\Lambda},
 r(\alpha),r(\beta) \in \iota(\Lambda^0)\}.\]

\[
 \alpha = [x;(0,d(\alpha))] \text{ and }
\beta = [y;(0,d(\beta))]
\]

\begin{equation}
 \label{eq:alpha_beta_v1}
x(d(\alpha) \wedge d(x)) = y(d(\beta) \wedge d(y))
\end{equation}

\begin{equation}
 \label{eq:alphabeta_v2}
d(\alpha)-d(\alpha) \wedge d(x) = d(\beta) -d(\beta) \wedge d(y).
\end{equation}

\begin{equation}\label{eq:talphatbeta*}
t_{\alpha}t_{\beta^*} = t_{\pi(\alpha)}t_{\gamma}t_{\gamma^*}t_{\pi(\beta)^*}.
\end{equation}

\[q_{r(\gamma) } = \sum_{\delta \in r(\gamma)  {\tilde{\Lambda}}^{d(\gamma)}} t_{\delta}t_{\delta^*}.\]

\[M := {\operatorname{\mathrm{span}}}\{t_{\lambda}t_{\mu^*} : \lambda, \mu \in \tilde{\Lambda}, r(\mu)\in \iota(\Lambda^0)\}\]

\[N := {\operatorname{\mathrm{span}}}\{t_{\lambda}t_{\mu^*} : \lambda, \mu \in \tilde{\Lambda}, r(\lambda)\in \iota(\Lambda^0)\}\]

\begin{gather*}
MN:={\operatorname{\mathrm{span}}}\{mn:m\in M, n\in N\}=\operatorname{KP}_R(\tilde\Lambda)\text{\ and\ } \\NM:={\operatorname{\mathrm{span}}}\{nm:m\in M, n\in N\}=B(\tilde\Lambda).
\end{gather*}

\[
t_\alpha t_{\beta^*}t_{\lambda}t_{\mu^*}=\sum_{d(\beta\sigma)=a,\beta\sigma=\lambda\tau} t_{\alpha\sigma}t_{(\mu\tau)^*}\in M
\]

\[
t_{\lambda}t_{\mu^*}t_\eta t_{\xi^*}=\sum_{d(\mu\sigma)=b,\mu\sigma=\eta\tau}t_{\lambda\sigma}t_{(\xi\tau)^*}\in M
\]

\[
t_\alpha t_{\beta^*} = t_\alpha q_{s(\alpha)} t_{\beta^*}=t_\alpha t_{\lambda^*} t_\lambda t_{\beta^*} \in MN.
\]

\[
nm=\sum_{d(\delta\sigma)=c,\delta\sigma=\lambda\tau} t_{\gamma\sigma}t_{(\mu\tau)^*}.
\]

\[
     \psi:M \otimes_B N \to A \text{ and }\phi:N \otimes_A M \to B
\]

\begin{equation}\label{eq-ops}n'\cdot \psi(m \otimes n) = \phi(n' \otimes m)\cdot n \text { and } m'\cdot \phi(n \otimes m) = \psi(
m' \otimes n)\cdot m\end{equation}

\[s(v\Lambda^{\leq e_i}) \subseteq H \text{ for some } i \in \{1, ..., k\} \implies
 v \in H.
\]

\[s(v{\tilde{\Lambda}}^{n}) \subseteq H \text{ for some } n \in {\mathbb{N}}^k \implies
 v \in H.
\]

\[\pi(v){\tilde{\Lambda}}^{m-m\wedge d(z)} = \{\lambda\}\]

\[
                  s\big(\pi(v){\tilde{\Lambda}}^{m-m\wedge d(z)}\big) = \{s(\lambda)\} = \{v\} \subseteq H,
                 \]

\[
 p_v=p_vp_vp_v \in NIM = L(I).
\]

\[H_{I,r} := \{v \in {\tilde{\Lambda}}^0 : rp_v \in I\},\]

\[rp_{\pi(v)} = p_{\pi(v)}rp_{\pi(v)}p_{\pi(v)} \in NIM = L(I).
\]

\[p_{\pi(v)} = p_{\pi(v)}p_{\pi(v)}p_{\pi(v)}  \in ML(I)N = I.\]

\[
s(\pi(v)\iota(\Lambda^{\leq e_i}))=s(\pi(v)\pi(\tilde\Lambda^{e_i}))=\pi(s(v\tilde\Lambda^{e_i}))\subseteq G.
\]

\begin{equation}J_G={\operatorname{\mathrm{span}}}\{s_\alpha s_{\beta^*}:\alpha,\beta\in\Lambda, s(\alpha)=s(\beta)\in G\}.\label{eq-is-ideal}\end{equation}

\begin{gather*}\operatorname{KP}_R(\tilde\Lambda)_j:= {\operatorname{\mathrm{span}}}\{t_\alpha t_{\beta^{*}}: \alpha,\beta\in{\tilde{\Lambda}}, d(\alpha)-d(\beta)=j\}\text{\ and }\\
B({\tilde{\Lambda}})_j:= {\operatorname{\mathrm{span}}}\{t_\alpha t_{\beta^{*}}: \alpha,\beta\in\iota(\Lambda), d(\alpha)-d(\beta)=j\}=B({\tilde{\Lambda}})\cap \operatorname{KP}_R(\tilde\Lambda)_j,
\end{gather*}

\begin{align}
L(I_H)&=NI_HM\notag\\
&={\operatorname{\mathrm{span}}}\{t_\lambda t_{\mu^*}t_\alpha t_{\beta^{*}}t_\sigma t_{\tau^{*}}: \lambda, \mu, \alpha,\beta, \sigma,\tau\in{\tilde{\Lambda}},s(\alpha)=s(\beta)\in H, r(\lambda),r(\tau)\in\iota(\Lambda^0)\}.\label{eq-mess}
\end{align}

\begin{align*}
t_\lambda (t_{\mu^*}t_\alpha)( t_{\beta^{*}}t_\sigma) t_{\tau^{*}}&=\sum_{(\gamma,\delta)\in\Lambda^{\min}(\mu,\alpha)}
\ \sum_{(\xi,\eta)\in\Lambda^{\min}(\beta,\sigma)} t_\lambda t_\gamma (t_{\delta^*}t_\xi) t_{\eta^*}t_{\tau^{*}}\\
&=\sum_{(\gamma,\delta)\in\Lambda^{\min}(\mu,\alpha)}
\ \sum_{(\xi,\eta)\in\Lambda^{\min}(\beta,\sigma)} \ \sum_{(\rho,\epsilon)\in\Lambda^{\min}(\delta,\xi)}t_\lambda t_\gamma t_{\rho}t_{\epsilon^*} t_{\eta^*}t_{\tau^{*}}
\end{align*}

\[
L(I_H)={\operatorname{\mathrm{span}}}\{t_\lambda t_{\tau^*}:\lambda,\tau\in{\tilde{\Lambda}}, r(\lambda),r(\tau)\in\iota(\Lambda^0), s(\lambda)=s(\tau)\in H\}
\]

\[
L(I_H)={\operatorname{\mathrm{span}}}\{t_\lambda t_{\tau^*}:\lambda,\tau\in\iota(\Lambda), s(\lambda)=s(\tau)\in H\cap \iota(\Lambda^0)\}.
\]

\[
 G\mapsto \pi^{-1}(G)\mapsto I_{\pi^{-1}(G)}\mapsto J_{\iota(G)}\mapsto J_G.\qedhere
 \]

\end{document}