\documentclass[a4paper]{article}


\usepackage{xspace}

\usepackage{graphicx}

\begin{document}


\begin{equation}
\label{model_subspace}
 {S}
 {:=}
 \Big\{ v:{\overline{\Omega}}\to{\mathbb{R}} \mid 
  \forall{K}\in{\mathcal{M}}\ v_{|{K}}\in{\mathcal{P}_{{\ell}}({{K}})}, \,
  v\in C^0({\overline{\Omega}}), \, v_{|\partial\Omega}=0
 \Big\},
\end{equation}

\begin{equation*}
\label{best-global-error}
 E(u)
 {:=}
 E(u,{S})
 {:=}
 \inf \big\{
  {\left\|{{\nabla}(u-v)}\right\|_{{\Omega}}} \mid v\in{S}
 \big\},
\end{equation*}

\begin{equation*}
\label{local-best-errors}
 e_{K}(u)
 {:=}
 \inf \big\{
  {\left\|{{\nabla}(u-p)}\right\|_{{K}}} \mid p\in{\mathcal{P}_{{\ell}}({{K}})}
 \big\},
\qquad
 \forall{K}\in{\mathcal{M}}.
\end{equation*}

\begin{equation}
\label{equivalence}
 \left(
  \sum_{{K}\in{\mathcal{M}}} e_{K}(u)^2
 \right)^{\frac12}
 \leq
 E(u)
 \leq
 C\left(
  \sum_{{K}\in{\mathcal{M}}} e_{K}(u)^2
 \right)^{\frac12},
\end{equation}

\begin{equation}
\label{apriori-ub}
 E(u)
 \leq
 C \left(
  \sum_{{K}\in{\mathcal{M}}} h_{K}^{2\ell}
   {\left\|{D^{\ell+1} u}\right\|_{{K}}}^2
 \right)^{\frac12},
\end{equation}

\begin{equation}
\label{TraceOp}
 (\cdot)_{|\partial{K}}:{H^{{1}}}({K})\to{L^{{2}}}(\partial{K})
\end{equation}

\begin{gather}
\label{A:conforming_mesh}
 \overline\Omega = \bigcup_{{K}\in{\mathcal{M}}} {K}
\qquad\text{and}\qquad
 \forall {K},{K}'\in{\mathcal{M}}
\quad
 \operatorname{Vert} ({K}\cap{K}') \subset \operatorname{Vert}{K} \cap \operatorname{Vert}{K}'.
\end{gather}

\[
 {\left|{\Omega}\right|}
 =
 \sum_{{K}\in{\mathcal{M}}} {\left|{K}\right|}
\]

\[
 v_{|\partial\Omega}=g
\quad\text{:}\quad
 \forall{K}\in{\mathcal{M}}\ v_{|\partial\Omega\cap\partial{K}} = 
   g_{|\partial\Omega\cap\partial{K}}.
\]

\[
 {S}^{{\ell},0}_0({\mathcal{M}})
 {:=}
 \{ V:\overline\Omega\to{\mathbb{R}} \mid
   \forall{K}\in{\mathcal{M}}\ V_{|{K}}\in{\mathcal{P}_{{\ell}}({{K}})},\ 
    V\in C^0(\overline\Omega),\ 
   V_{|\partial\Omega}=0 \}
\]

\begin{equation}
\label{D:H10}
 H^1_0(\Omega)
 {:=}
 \{v\in{L^{{2}}}(\Omega) \mid
  {\nabla} v\in{L^{{2}}}(\Omega),\ 
  v_{|\partial\Omega} = 0 \}.
\end{equation}

\[
 {S}^{{\ell},{-1}}({\mathcal{M}})
 {:=}
 \{ V:\overline\Omega\to{\mathbb{R}} \mid
   \forall{K}\in{\mathcal{M}}\ V_{|{K}}\in{\mathcal{P}_{{\ell}}({{K}})} \}
\]

\[
 {S}^{{\ell},0}({\mathcal{M}})
 {:=}
 \{ V\in{S}^{{\ell},{-1}} \mid
   V\in C^0(\overline\Omega) \}
\]

\[
 {L_{{\ell}}}({K})
 {:=}
 \left\{
  \frac1{\ell} \sum_{i=1}^k \alpha_i a_i \mid
   \alpha=(\alpha_0,\dots,\alpha_k)\in{\mathbb{N}}_0^{k+1}, \
   {|{{\alpha}}|}={\ell}
  \right\}.
\]

\[
 P_{|{L_{{\ell}}}({K})}=Q_{|{L_{{\ell}}}({K})}
\implies
 P=Q \text{ on }{K}
\]

\begin{equation}
\label{LagrangeCompatability}
 {L_{{\ell}}}({K})\cap{F}={L_{{\ell}}}({F}).
\end{equation}

\[
 {L_{{\ell}}}({\mathcal{M}})
 {:=}
 \bigcup_{{K}\in{\mathcal{M}}} {L_{{\ell}}}({K});
\]

\begin{equation}
\label{LgrBasis}
 {\Phi}_z\in{S}^{{\ell},0}({\mathcal{M}})
\quad\text{and}\quad
 \forall y\in{L_{{\ell}}}({\mathcal{M}})\ 
 {\Phi}_z(y) = \delta_{yz}
\end{equation}

\begin{equation*}
  V = \sum_{z\in{L_{{\ell}}}({\mathcal{M}})} V(z) {\Phi}_z
\end{equation*}

\[
 \operatorname{supp}{\Phi}_z
 =
 \omega_z\
 {:=}
 \bigcup_{{K}\in{\mathcal{M}}:{K}\ni z} {K}.
\]

\begin{equation}
\label{RefNode}
 \Hat{z}{:=}\sum_{i=1}^d \lambda_i^* e_i
 \in
 {L_{{\ell}}}({{{K}_d}}).
\end{equation}

\begin{equation}
\label{LebnormBFct2}
 {{\left\|{{{\Phi}_z}}\right\|_{{0,2;{K}}}}}
 =
 \sqrt{d!}{\left|{K}\right|}^{\frac12} {{\left\|{{\Hat{\Phi}_{\Hat z}}}\right\|_{{0,2;{{{K}_d}}}}}}
\end{equation}

\begin{equation}
\label{PointEVal}
 \delta_z : 
 {S}^{{\ell},0}({\mathcal{M}}) \ni V
 \mapsto
 V(z) \in {\mathbb{R}}
\end{equation}

\begin{equation}
\label{DBFct}
 {\Psi}_z^{F}\in{\mathcal{P}_{{\ell}}({{F}})}
\quad\text{and}\quad
 \forall y\in{L_{{\ell}}}({F}) \ 
  \int_F {\Phi}_y {\Psi}_z^{F} = \delta_{yz}.
\end{equation}

\begin{equation}
\label{LebnormDBFct2} 
 {{\left\|{{{\Psi}_z}}\right\|_{{0,2;{F}}}}}
 =
 \frac{1}{\sqrt{(d-1)!}}{\left|{F}\right|}^{-\frac12}
 {{\left\|{{\Hat{\Psi}_{\Hat z}}}\right\|_{{0,2;{{K}_{d-1}}}}}},
\end{equation}

\[
 \forall y\in{L_{{\ell}}}({\mathcal{M}})
\quad 
 \int_F {\Phi}_y {\Psi}_z^{F} = \delta_{yz}.
\]

\[
 \forall V\in{S}^{{\ell},0}({\mathcal{M}})
\quad 
 V(z) = {N}_{z;{F}}(V)
\]

\begin{equation}
\label{ScottZhangFct}
 {N}_{z;{F}}(v)
 {:=}
 \int_F v {\Psi}_z^{F}.
\end{equation}

\[
 v\in{H^{{1}}}_0(\Omega)
 \implies
 N_{z;F}(v) = 0
\]

\begin{equation}
\label{H1seminorm}
 {\left|{w}\right|_{{\Omega}}}
 {:=}
 {{\left\|{{|{\nabla} w|}}\right\|_{{0,2;\Omega}}}}
 =
 \left( \int_\Omega |{\nabla} w|^2 \right)^{\frac12}.
\end{equation}

\[
 E(v,{\mathcal{M}})
 {:=}
 E\big( v,{S}({\mathcal{M}}) \big)
 {:=}
 \inf_{V\in{S}({\mathcal{M}})} {\left|{v-V}\right|_{{\Omega}}}
\]

\[
 {\left|{v-V_{\mathcal{M}}}\right|_{{\Omega}}}
 =
 E(v,{\mathcal{M}}).
\]

\[
 \forall W\in{S}({\mathcal{M}})
\quad
 \int_\Omega {\nabla} V_{\mathcal{M}} \cdot {\nabla} W
 =
  \int_\Omega {\nabla} v \cdot {\nabla} W.
\]

\[
 e(v,{K})
 {:=}
 e\big( v,{\mathcal{P}_{{\ell}}({{K}})} \big)
 {:=}
 \inf_{P\in{\mathcal{P}_{{\ell}}({{K}})}} {\left|{v-P}\right|_{K}},
\]

\begin{equation}
\label{Pelm}
 P_{K}\in{\mathcal{P}_{{\ell}}({{K}})},
\quad
 \int_{K} P_{K} = \int_{K} v
\quad\text{and}\quad
 {\left|{v-P_{K}}\right|_{K}}=e(v,{K}),
\end{equation}

\begin{equation}
\label{Pelm:ort}
 \forall Q\in{\mathcal{P}_{{\ell}}({{K}})}
\quad
 \int_{K} {\nabla} P_{K} \cdot {\nabla} Q
 =
 \int_{K} {\nabla} v \cdot {\nabla} Q.
\end{equation}

\begin{align}
\label{local<=global}
 \left[
  \sum_{{K}\in{\mathcal{M}}} e(v,{K})^2
 \right]^{\frac12}
 \leq
  E(v,{S}'),
\end{align}

\begin{equation}
\label{global<=Clocal}
 \forall v\in X
\quad
 E\big( v,{S}({\mathcal{M}}) \big)
 \leq
 C  \left[
  \sum_{{K}\in{\mathcal{M}}} e(v,{K})^2
 \right]^{\frac12}
\end{equation}

\[
 {{\left\|{{w}}\right\|_{{0,2;{F}}}}}
 \leq
 {{C_\text{Tr}}} \left(
   \frac{h_{K} {\left|{F}\right|}}{{\left|{K}\right|}}
  \right)^{\frac12}
  h_{K}^{\frac12} {{\left\|{{{\nabla} w}}\right\|_{{0,2;{K}}}}},
\]

\begin{equation*}
 \frac1{{\left|{F}\right|}} {{\left\|{{w}}\right\|_{{0,2;{F}}}}}^2
 \leq
 \frac1{{\left|{K}\right|}} {{\left\|{{w}}\right\|_{{0,2;{K}}}}}^2
 +
 \frac{2h_{K}}{d{\left|{K}\right|}} {{\left\|{{w}}\right\|_{{0,2;{K}}}}}
  {{\left\|{{{\nabla} w}}\right\|_{{0,2;{K}}}}}.
\end{equation*}

\begin{equation*}
 {{\left\|{{w}}\right\|_{{0,2;{K}}}}}
 \leq
 C_P h_{K} {{\left\|{{{\nabla} w}}\right\|_{{0,2;{K}}}}},
\end{equation*}

\[
 \frac{h_{K} {\left|{F}\right|}}{{\left|{K}\right|}}
 =
 d\frac{h_{K}}{h^\perp_F}
 \leq
 d\frac{h_{K}}{\rho_{K}}
\]

\begin{align*}
 h_{F}^{-\frac12} {{\left\|{{P_{{K}_1}-P_{{K}_2}}}\right\|_{{0,2;{F}}}}}
 &\leq
 h_{F}^{-\frac12} {{\left\|{{P_{{K}_1}-v}}\right\|_{{0,2;{F}}}}}
  + 
  h_{F}^{-\frac12} {{\left\|{{v-P_{{K}_2}}}\right\|_{{0,2;{F}}}}}
\\
 &\leq
 C \big[ e(v,{K}_1) + e(v,{K}_2) \big],
\end{align*}

\[
 {\Pi}:{H^{{1}}}(\Omega)\to{S}^{{\ell},0}({\mathcal{M}})
\]

\begin{equation}
\label{Ip;BdryVals}
 v\in X
 \implies
 {\Pi} v\in{S}({\mathcal{M}})
\end{equation}

\begin{equation}
\label{GDcplng}
 {\left|{v-{\Pi} v}\right|_{{\Omega}}}
 \leq
 C \left[
  \sum_{{K}\in{\mathcal{M}}} e(v,{K})^2
 \right]^{\frac12}
\end{equation}

\[
 \Pi v
 =
 \sum_{z\in{L_{{\ell}}}({\mathcal{M}})} {\Pi}_z v \, {\Phi}_z
\]

\begin{equation}
\label{DefIp:unconstrained}
 {\Pi}_z v {:=} P_{K}(z),
\end{equation}

\begin{equation}
\label{DefIp:constrained}
 {\Pi}_z v
 {:=}
 {N}_{z;F_z}(v).
\end{equation}

\[
 {\mathcal{C}} = {L_{{\ell}}}({\mathcal{M}}) \cap {\Sigma}
\quad\text{with}\quad
 {\Sigma}
 {:=}
 \bigcup_{{F}\in{\mathcal{F}_{d-1}}({\mathcal{M}})} {F}
\]

\[
 \omega_z = \bigcup\{{K}\in{\mathcal{M}} : {K}\ni z\},
\qquad
 z\in{L_{{\ell}}}({\mathcal{M}}),
\]

\[
 {\left|{w}\right|_{{\Omega}}}^2
 =
 \sum_{{K}\in{\mathcal{M}}}{\left|{w}\right|_{K}}^2,
\]

\[
 \omega_{K}
 {:=}
 \bigcup \{{K}'\in{\mathcal{M}}:{K}'\cap{K}\neq\emptyset\}
\]

\begin{equation}
\label{LDcplng}
 {\left|{v - {\Pi} v}\right|_{K}}^2
 \leq
 e(v,{K})^2 
 +
 {\delta}_{K}^2
 \sum_{z\in{L_{{\ell}}}({K})} \sum_{{K}'\ni z} e(v,{K}')^2,
\end{equation}

\[
 {\left|{v - {\Pi} v}\right|_{K}}^2
 =
 e(v,{K})^2 
 +
 {\left|{P_{K} - {\Pi} v}\right|_{K}}^2,
\]

\[
 (P_{K} - {\Pi} v)_{|{K}}
 =
 \sum_{z\in{L_{{\ell}}}({K})}
  \big[ P_{K}(z) - {\Pi}_z v \big] {\Phi}_z{}_{|{K}}
 =
 \sum_{z\in{L_{{\ell}}}({K})\cap{\mathcal{C}}}
  \big[ P_{K}(z) - {N}_{z,{F}_z}(v) \big] {\Phi}_z{}_{|{K}},
\]

\begin{equation}
\label{CplngErr}
 {\left|{P_{K} - {\Pi} v}\right|_{K}}
 \leq
  \sum_{z\in{L_{{\ell}}}({K})\cap{\mathcal{C}}}
  \big| P_{K}(z) - {N}_{z,{F}_z}(v) \big|
   {{\left\|{{{\nabla}{\Phi}_z}}\right\|_{{0,2;{K}}}}}.
\end{equation}

\[
 P_{K}(z)-{N}_{z,{F}_z}(v)
 =
 {N}_{z,n}(P_n)-{N}_{z,0}(v)
\]

\[
 \forall i=0,\dots,n-1
\quad
 {N}_{z,i}(P_i)
 =
 P_i(z)
 =
 {N}_{z,i+1}(P_i),
\]

\begin{equation}
\label{Telescopic}
 P_{K}(z)-{N}_{z,{F}_z}(v)
 =
 {N}_{z,0}(P_0-v)
 +
 \sum_{i=1}^n {N}_{z,i}(P_i-P_{i-1}).
\end{equation}

\begin{align*}
 |{N}_{z,0}(v-P_0)|
 &=
 \left|
  \int_{{F}_0} (v-P_0) {\Psi}^i_z
 \right|
 \leq
 {{\left\|{{v-P_0}}\right\|_{{0,2;{{F}_0}}}}} {{\left\|{{{\Psi}^0_z}}\right\|_{{0,2;{{F}_0}}}}}
\\
 &\leq
 \frac{{C_\text{Tr}}}{\sqrt{(d-1)!}}
 {{\left\|{{\Hat{\Psi}_{\Hat z}}}\right\|_{{0,2;{{K}_{d-1}}}}}}
 \frac{h_{0}}{{\left|{{K}_0}\right|}^{\frac12}}
  e(v,{K}_0),
\end{align*}

\begin{equation*}\begin{aligned}
 {N}_{z,i}(P_i &- P_{i-1})
 \leq
 |{N}_{z,i}(P_i - v)| + |{N}_{z,i}(v - P_{i-1})|
\\
 &\leq
 \frac{{C_\text{Tr}}}{\sqrt{(d-1)!}}
 {{\left\|{{\Hat{\Psi}_{\Hat z}}}\right\|_{{0,2;{{K}_{d-1}}}}}}
 \left[
  \frac{h_{i}}{{\left|{{K}_i}\right|}^{\frac12}} e(v,{K}_i)
  +
  \frac{h_{i-1}}{{\left|{{K}_{i-1}}\right|}^{\frac12}} e(v,{K}_{i-1})
 \right].
\end{aligned}\end{equation*}

\[
 |P_{K}(z)-{N}_{z,{F}_z}(v)|
 \leq
 \frac{2{{C_\text{Tr}}}}{\sqrt{(d-1)!}}
 {{\left\|{{\Hat{\Psi}_{\Hat z}}}\right\|_{{0,2;{{K}_{d-1}}}}}}
 \sum_{i=0}^n 
  \frac{h_{i}}{{\left|{{K}_i}\right|}^{\frac12}} e(v,{K}_i).
\]

\begin{equation}\label{nbnval}
 |P_{K}(z)-{N}_{z,{F}_z}(v)|
 \leq
 \frac{2{{C_\text{Tr}}}}{\sqrt{(d-1)!}}
 {{\left\|{{\Hat{\Psi}_{\Hat z}}}\right\|_{{0,2;{{K}_{d-1}}}}}}
  \sum_{{K}'\subset\omega_z}
   \frac{h_{{K}'}}{{\left|{{K}'}\right|}^{\frac12}}
   e(v,{K}'),
\end{equation}

\begin{equation*}
 {\left|{P_{K} - {\Pi} v}\right|_{K}}
 \leq
 2 \sqrt{d} {{C_\text{Tr}}}
 \sum_{z\in{L_{{\ell}}}({K})\cap{\mathcal{C}}}
 \sum_{{K}'\subset\omega_z}
  d_{\Hat z}
   \frac{h_{{K}'} {{\left\|{{{\nabla}{\Phi}_z}}\right\|_{{0,2;{K}}}}} {\left|{K}\right|}^{\frac12}}
   {{{\left\|{{{\Phi}_z}}\right\|_{{0,2;{K}}}}} {\left|{{K}'}\right|}^{\frac12}}
   e(v,{K}')
\end{equation*}

\[
 d_{\Hat z}
 {:=}
 {{\left\|{{\Hat{\Psi}_{\Hat z}}}\right\|_{{0,2;{{K}_{d-1}}}}}}
 {{\left\|{{\Hat{\Phi}_{\Hat z}}}\right\|_{{0,2;{{{K}_d}}}}}}.
\]

\begin{equation}
\label{locDcplngConst}
 {\delta}_{K}^2
 =
 4 d {{C_\text{Tr}}}
 \sum_{z\in{L_{{\ell}}}({K})\cap{\mathcal{C}}}
  d_{\Hat z}^2 \mu_z
  \frac{h_{K}^2 {{\left\|{{{\nabla}{\Phi}_z}}\right\|_{{0,{K};2}}}}^2}
   {{{\left\|{{{\Phi}_z}}\right\|_{{0,{K};2}}}}^2}
\end{equation}

\[
 \mu_z
 {:=}
 \frac{{\left|{K}\right|}}{h_{K}^2}
 \sum_{{K}'\subset\omega_z}
  \frac{h_{{K}'}^2}{{\left|{{K}'}\right|}}.
\]

\[
 \frac{h_{{K}'}^2{\left|{K}\right|}}{h_{K}^2{\left|{{K}'}\right|}}.
\]

\begin{equation}
\label{LocShapeReg}
 \forall {K}'\subset\omega_{K}
\quad
 \frac{h_{{K}'}}{\rho_{{K}'}}
 \leq
 \sigma_{K}.
\end{equation}

\[
 \frac{h_{K} {{\left\|{{{\nabla}{\Phi}_z}}\right\|_{{0,{K};2}}}}}
  {{{\left\|{{{\Phi}_z}}\right\|_{{0,{K};2}}}}}
 \leq
 \sigma_{K}
 \frac{{{\left\|{{{\nabla}\Hat{\Phi}_{\Hat z}}}\right\|_{{0,{{{K}_d}};2}}}}}
  {{{\left\|{{\Hat{\Phi}_{\Hat z}}}\right\|_{{0,{{{K}_d}};2}}}}}.
\]

\[
 {\delta}_{K}^2
 \leq
 4 d {{C_\text{Tr}}}
 C(\sigma_{K})
 \sum_{z\in{L_{{\ell}}}({K})\cap{\mathcal{C}}}
  {{\left\|{{\Hat{\Psi}_{\Hat z}}}\right\|_{{0,{{K}_{d-1}};2}}}}^2
  {{\left\|{{{\nabla}\Hat{\Phi}_{\Hat z}}}\right\|_{{0,{{{K}_d}};2}}}}^2.
\]

\begin{equation*}
 {\left|{v-{\Pi} v}\right|_{{\Omega}}}
 \leq
 C \left[
  \sum_{{K}\in{\mathcal{M}}} e(v,{K})^2
 \right]^{\frac12}
\end{equation*}

\[
 N_{\mathcal{M}}
 {:=}
 \max_{z\in{L_{{\ell}}}({\mathcal{M}})} \#\{{K}'\in{\mathcal{M}} \mid {K}'\ni z\}
\]

\[
 X_g {:=} \{ v \in {H^{1}}(\Omega) \mid v_{|\partial\Omega} = g \}
\]

\[
 {S}_g({\mathcal{M}})
 {:=}
 \{ V\in{S}^{{\ell},-1}({\mathcal{M}}) \mid
    V\in C^0(\overline\Omega),
    V_{|\partial\Omega} = {\Pi^{\text{SZ}}} g \}
 
 
\]

\[
  E\big( v,{S}_g({\mathcal{M}}) \big)
 \leq
 C  \left[
  \sum_{{K}\in{\mathcal{M}}} e(v,{K})^2
 \right]^{\frac12},
\]

\[
 {\mathcal{C}} = {L_{{\ell}}}({\mathcal{M}}) \cap {\Sigma}
\quad\text{with}\quad
 {\Sigma}
 =
 \bigcup_{{F}\in{\mathcal{F}_{d-1}}({\mathcal{M}})} {F}
\]

\[
 {\Pi} v_{|\partial\Omega}
  =
 {\Pi^{\text{SZ}}} v_{|\partial\Omega}
\]

\[
 \Tilde X {:=} {H^{1}}(\Omega)/{\mathbb{R}},
\]

\[
 \Tilde{S}({\mathcal{M}})
 {:=}
 {S}^{{\ell},0}({\mathcal{M}})/{\mathbb{R}}.
\]

\[
  E\big( v, \Tilde{S}({\mathcal{M}}) \big)
 \leq
 C  \left[
  \sum_{{K}\in{\mathcal{M}}} e(v,{K})^2
 \right]^{\frac12},
\]

\begin{align*}
 {\underline{e}}(v,{K})
 &{:=}
 \inf_{Q\in{\mathcal{P}_{{{\ell}-1}}({{K}})}^d} {\left\|{{\nabla} v-Q}\right\|_{K}}
 =
 \left( \sum_{i=1}^d
  \inf_{R\in{\mathcal{P}_{{{\ell}-1}}({{K}})}} {\left\|{\partial_i v - R}\right\|_{K}}^2
 \right)^{\frac12},
\end{align*}

\[
 {\left\|{f}\right\|_{{\Omega}}}
 {:=}
 \| |f| \|_{0,2;\Omega}
 =
 \left(
  \int_\Omega |f|^2
 \right)^{\frac12}
\]

\[
 {\underline{e}}(v,{K}) \leq e(v,{K})
\]

\[
  e(v,{K})
  \leq
  C {\underline{e}}(v,{K}).
\]

\begin{equation}\label{Diff-avgTaylor}
 \partial_i \Big( \big[ I_{\ell} (v\circ A) \big] \circ A^{-1} \Big)
 =
 \Big( I_{{\ell}-1} \big[ (\partial_i v) \circ A \big] \Big) \circ A^{-1},
\end{equation}

\begin{gather*}
 w\in{\mathcal{P}_{{\ell}}({{{{K}_d}}})} \implies I_{\ell} w = w,
\\
 {\left\|{I_{\ell} w}\right\|_{{{K}_d}}} \leq C_{d,{\ell}} {\left\|{w}\right\|_{{{K}_d}}}.
\end{gather*}

\begin{equation}\label{Ipdeg:nbest}
 {\left\|{w-I_{\ell} w}\right\|_{{{K}_d}}}
 \leq
 C_{d,{\ell}} \inf_{S\in{\mathcal{P}_{{\ell}}({{{{K}_d}}})}} {\left\|{w-S}\right\|_{{{K}_d}}}.
\end{equation}

\begin{align*}
 e(v,{K})^2
 &\leq
 {\left\|{{\nabla} (v - P)}\right\|_{K}}^2
 =
 \sum_{i=1}^d {\left\|{\partial_i v - \partial_i P}\right\|_{K}}^2
\\
 &=
 \sum_{i=1}^d 
  {\left\|{\partial_i v - \Big(
    I_{{\ell}-1} \big[ (\partial_i v) \circ A \big] 
    \Big) \circ A^{-1}}\right\|_{K}}^2.
\\
 &=
 \frac{{\left|{K}\right|}}{{\left|{{{K}_d}}\right|}} \sum_{i=1}^d 
  {\left\|{ (\partial_i v)\circ A - I_{{\ell}-1} \big[ (\partial_i v) \circ A 
   \big] }\right\|_{{{K}_d}}}^2
\\
 &\leq
 C_{d,{\ell}-1}^2 \frac{{\left|{K}\right|}}{{\left|{{{K}_d}}\right|}} \sum_{i=1}^d
  \inf_{S\in{\mathcal{P}_{{{\ell}-1}}({{{{K}_d}}})}}
   {\left\|{\partial_i v\circ A - S}\right\|_{{{K}_d}}}^2
\\
 &\leq
 C_{d,{\ell}-1}^2  \sum_{i=1}^d
  \inf_{R\in{\mathcal{P}_{{{\ell}-1}}({{K}})}}
   {\left\|{\partial_i v - R}\right\|_{K}}^2
 =
 C_{d,{\ell}-1}^2 {\underline{e}}(v,{K})^2
\end{align*}

\[
 E\big( v,{S}({\mathcal{M}}) \big)
 \leq
 C \left[
  \sum_{{K}\in{\mathcal{M}}} {\underline{e}}(v,{K})^2
 \right]^{\frac12},
\]

\[
  E(v,{\mathcal{M}}) \to 0
  \quad\text{as}\quad
  h {:=} \max_{{K}\in{\mathcal{M}}} h_{K} \to 0
 \]

\[
 \forall{K}\in{\mathcal{M}}
 \quad
 \overline f_{|{K}} = \frac1{{\left|{K}\right|}} \int_{K} f.
\]

\begin{equation}\label{mv-bd}\begin{aligned}
 E(v,{\mathcal{M}}) 
 &\leq
 C \left( \sum_{{K}\in{\mathcal{M}}} e(v,{K})^2 \right)^{\frac12}
 \leq
 C \left(
  \sum_{{K}\in{\mathcal{M}}} \inf_{P\in{\mathcal{P}_{1}({{K}})}} {\left|{v-P}\right|_{K}}^2
 \right)^{\frac12}
\\
 &=
 C \left(
  \sum_{{K}\in{\mathcal{M}}} \inf_{c\in{\mathbb{R}}} {\left\|{{\nabla} v - c}\right\|_{K}}^2
 \right)^{\frac12}
 =
 C {\left\|{{\nabla} v - \overline{{\nabla} v}}\right\|_{{\Omega}}},
\end{aligned}\end{equation}

\begin{multline*}
 {\left\|{{\nabla} v - \overline{{\nabla} v}}\right\|_{{\Omega}}}
 \leq
 {\left\|{{\nabla} v - g}\right\|_{{\Omega}}}
  + {\left\|{g - \overline g}\right\|_{{\Omega}}}
  + {\left\|{\overline{g-{\nabla} v}}\right\|_{{\Omega}}}
 \leq
 (2{\epsilon})/3 + {\left\|{g - \overline g}\right\|_{{\Omega}}}
\end{multline*}

\begin{equation*}
 {{\left|{{v}}\right|_{{{s},{2};{K}}}}}
 {:=}
 \begin{cases}
  \left(
   \sum_{|\alpha|=s} {{\left\|{{\partial^\alpha v}}\right\|_{{0,{2};{K}}}}}^2
  \right)^{\frac12}
  & \text{if }s\in{\mathbb{N}}
\\
  (1-\theta)\left(
    \sum_{|\alpha|=\lfloor s\rfloor} \displaystyle
     \int_{K}\int_{K}
     \frac{|\partial^\alpha v(x) - \partial^\alpha v(y)|^2}{|x-y|^{2\theta+d}}
    \right)^{\frac12}
  & \text{otherwise,}
 \end{cases} 
\end{equation*}

\[
 E(v,{\mathcal{M}})
 \leq
 C \left(
   \sum_{{K}\in{\mathcal{M}}} h_{K}^{2(s-1)} {{\left|{{v}}\right|_{{{s},{2};{K}}}}}^2
 \right)^{\frac12},
\]

\[
 C \leq \frac{s!}{(\lceil\frac{s}{d}\rceil!)^d} C_P^{s-1}\delta({\mathcal{M}})
\]

\begin{equation}\label{BrambleHilbert}
 e(v,{K})
 \leq
 C h_{K}^{s-1} {{\left|{{v}}\right|_{{{s},{2};{K}}}}}
\end{equation}

\[
  \texttt{error reduction} \to \texttt{sparsity adjustment}.
 \]

\begin{equation}\label{complete}
 \#\texttt{complete}({\mathcal{M}}') - \#{\mathcal{M}}_0
 \leq
 {{C_\text{cmpl}}} (\#{\mathcal{M}}' - \#{\mathcal{M}}_0)
\end{equation}

\begin{equation*}
 \sigma(v,N)
 {:=}
 \min \big\{ E \big( v,{S}({\mathcal{M}}) \big)
  \mid {\mathcal{M}}\in{\mathbb{M}},\ \#{\mathcal{M}}\leq 
N \big\}
\end{equation*}

\begin{equation}
\label{nlberr}
 \sigma'(v,N)
 {:=}
 \min \{ E\big( v,{S}^{{\ell},-1}({\mathcal{M}}') \big)
   \mid {\mathcal{M}}'\in{\mathbb{M}}',\ \#{\mathcal{M}}'\leq N \}
\end{equation}

\[
 \sigma(v,N)
 \leq
 C_1 \sigma'\left(
  v, \left\lfloor \frac{N-N_0}{C_2} \right\rfloor + N_0
  \right).
\]

\begin{align*}
 \sigma(v,N)
 &\leq
 E\big( v, {S}({\mathcal{M}}) \big)
 \leq
 {\delta}({\mathcal{M}}) E\big( v, {S}^{{\ell},-1}({\mathcal{M}}) \big)
 \leq
 {\delta}({\mathcal{M}}) E\big( v, {S}^{{\ell},-1}({\mathcal{M}}') \big)
\\
 &=
 {\delta}({\mathcal{M}}) \sigma'(v,N')
\end{align*}

\[
 {\epsilon}({K}){:=} e(v,{K})^2,
\]

\[
 E\big( v,{S}({\mathcal{M}}) \big)
 \leq
 C_1 \sigma' \left( v, \left\lceil \frac{\#{\mathcal{M}}}{C_2} \right\rceil \right)
\]

\[
 {\epsilon}({K}_1) + {\epsilon}({K}_2) \leq {\epsilon}({K}).
\]

\[
 N_0{:=}\#{\mathcal{M}}_0,
\quad
 N'{:=}\#{\mathcal{M}}_t',
\quad
 L'{:=} N'-N_0
\]

\[
 E\big( v,{S}^{{\ell},-1}({\mathcal{M}}_t') \big)
 \leq
 \min_{0 \leq l \leq L'} \left( 1 +
   \frac{l + \min\{l,N_0\}}{L' + 1 - l}
   \right) \sigma'(v,N_0+l).
\]

\[
 E\big( v,{S}^{{\ell},-1}({\mathcal{M}}_t') \big)
 \leq
 \min_{2N_0 \leq n \leq N'} \frac{N'+1}{N'+1-n} \sigma'(v,n).
\]

\[
 N - N_0
 \leq
 {{C_\text{cmpl}}} (N' - N_0)
\]

\[
 E\big( v,{S}^{{\ell},-1}({\mathcal{M}}_t) \big)
 \leq
 \min_{2N_0 \leq n \leq N/\Tilde C_2}
   \frac{N}{N - \Tilde C_2 n} \sigma'(v,n)
\]

\[
 E\big( v,{S}({\mathcal{M}}_t) \big)
 \leq
 \delta \min_{2N_0 \leq n \leq N/\Tilde C_2}
   \frac{N}{N - \Tilde C_2 n} \sigma'(v,n)
\]

\[
 \Tilde{\epsilon}({K})
 {:=}
 \inf\big\{
  {\left|{v-V}\right|_{{\omega_{K}}}} \mid V\in{S}({\mathcal{M}}_{K})
  \big\}
\]

\[
 R^-({K})
 {:=}
 \bigcap_{{\mathcal{M}}\in{\mathbb{M}}:{\mathcal{M}}\ni{K}} R({K},{\mathcal{M}})
\quad\text{with}\quad
 R({K},{\mathcal{M}})
 {:=}
 \bigcup_{{K}'\in{\mathcal{M}}:{K}'\cap{K}\neq\emptyset} {K}'.
\]

\end{document}