\documentclass{article}


\usepackage{xypic}

\usepackage{thmtools}

\begin{document}


\begin{equation}\label{eq:0.1}
q(ax)=a^2q(x)
\end{equation}

\begin{equation}\label{eq:0.2}
q(x+y)= q(x)+q(y)+b(x,y)
\end{equation}

\begin{align}
\text{If}\ ex\ne ey, & \ \text{ then} \ x+y\in\{x,y\}, \label{eq:0.3} \\
\text{If}\ ex= ey,& \ \text{ then} \ x+y=ey. \label{eq:0.4}
\end{align}

\begin{equation}\label{eq:0.5}
u\le v {\ {\Leftrightarrow} \ } u+v=v.
\end{equation}

\begin{equation}\label{eq:0.6}
x+y=\begin{cases} y&\ \text{if}\ ex<ey,\\
x&\ \text{if}\ ex>ey,\\
ey&\ \text{if}\ ex=ey.
\end{cases}
\end{equation}

\begin{equation}\label{eq:0.7}
ex=0 {\ {\Rightarrow} \ } x=0.
\end{equation}

$$R':={\mathcal T}(R)\cup e{\mathcal T}(R)\cup\{0\}$$

\begin{equation}\label{eq:0.8}
q\bigg(\sum_ix_i{\varepsilon}_i\bigg)=\sum_i q({\varepsilon}_i)x_i^2,
\end{equation}

\begin{equation}\label{eq:0.9}
q=q_{QL}+\rho,
\end{equation}

\begin{equation}\label{eq:0.10}
{\operatorname{CS}}(x,y):=\frac{eb(x,y)^2}{eq(x)q(y)}\in eR,
\end{equation}

$$x\le y {\ {\Leftrightarrow} \ } \exists z\in V: x+z=y.$$

\begin{equation}\label{eq:II.5.1}
eb_1(x,y)=eb_2(x,y)\end{equation}

\begin{equation}\label{eq:II.5.2}
\chi:=\chi_{x,y}:R{\varepsilon}_1+R{\varepsilon}_2\to V\end{equation}

\begin{equation}\label{eq:II.5.3} {\tilde q} :=q\circ\chi:R{\varepsilon}_1+R{\varepsilon}_2\to R.\end{equation}

\begin{equation}\label{eq:II.5.4}
{\tilde b}(v_1,v_2):=b(\chi(v_1),\chi(v_2)) \qquad (v_1,v_2\in V) \end{equation}

$${\tilde q} ({\lambda} {\varepsilon}_1+ \mu {\varepsilon}_2)={\tilde q} ({\lambda} {\varepsilon}_1)+{\tilde q} (\mu {\varepsilon}_2)$$

\begin{equation}\label{eq:II.5.5}
b(x,y)^2\le_\nu q(x)q(y).\end{equation}

\begin{equation}\label{eq:II.5.6}
b(x,y)^2<_\nu \pi^{-1}q(x)q(y)\end{equation}

\begin{equation}\label{eq:II.5.7}
b(x,y)^2\cong_\nu \pi^{-1}q(x)q(y).\end{equation}

\begin{equation}\label{eq:II.5.8}
 b(x,y)^2>_\nu \pi^{-1}q(x)q(y)\end{equation}

$$b(x,y)^2>_\nu q(x)q(y).$$

$$b(x,y)^2>_\nu \pi^{-1}q(x)q(y),$$

$$b(x,y)^2\cong_\nu \pi^{-1}q(x)q(y)$$

\begin{equation}\label{eq:II.5.9}
b(x,y)^2 {<_\nu} q(x)q(y).\end{equation}

\begin{equation}\label{eq:II.5.10}
b(x,y)^2 {\leq_\nu} q(x)q(y)\end{equation}

\begin{equation}\label{eq:II.5.11}
b(x,y)^2 {\leq_\nu} c q(x)q(y)\end{equation}

\begin{equation}\addtocounter{equation}{-1}\label{eq:str.1}
q(x+y) = q(x) + q(y).
\end{equation}

\begin{equation}\addtocounter{equation}{-1}\label{eq:str.1}
q(x+y) = q(x) + q(y) + b(x,y).
\end{equation}

\begin{equation}\label{eq:II.6.1}
V_{\operatorname{an}}:=\{x\in V {\ {|} \ }q(x)\ne0\} \cup \{ 0 \},\end{equation}

\begin{equation}\label{eq:II.6.2}
V+V_{\operatorname{an}} =V_{\operatorname{an}}.\end{equation}

\begin{equation}\label{eq:II.6.3}
\bigg[\frac{\lambda}{\mu}\bigg]_\nu\cong_\nu\gamma
{\quad {\Leftrightarrow} \quad }\gamma\mu\cong_\nu{\lambda}.
\end{equation}

\begin{equation}\label{eq:II.6.4} \forall {\gamma} \in {\mathcal T}: \qquad
\bigg[\frac{\lambda}{\mu}\bigg]_\nu\cong_\nu\gamma {\quad {\Leftrightarrow} \quad }{\lambda}\cong_\nu\gamma\mu.
\end{equation}

$${\operatorname{CS}}(x,y):=\bigg[\frac{b(x,y)^2}{q(x)q(y)}\bigg]_\nu$$

\begin{equation}\label{eq:II.6.6}
{\operatorname{CS}}({\lambda} x,\mu y)={\operatorname{CS}}(x,y)\end{equation}

\begin{equation}\label{eq:II.6.8}
ac+bd=(a+b)(c+d).\end{equation}

\begin{equation}\label{eq:II.6.9}
ac+bd\cong_\nu (a+b)(c+d).\end{equation}

\begin{equation}\label{eq:II.6.10}
{\operatorname{CS}}(x+y,w){\ {\le} \ }{\operatorname{CS}}(x,w)+{\operatorname{CS}}(y,w).\end{equation}

\begin{equation}\label{eq:II.6.11}
{\operatorname{CS}}(x+y,w){\ {<} \ }{\operatorname{CS}}(x,w)+{\operatorname{CS}}(y,w).\end{equation}

\begin{equation}\label{eq:II.6.12}
{\operatorname{CS}}(x+y,w){\ {=} \ }{\operatorname{CS}}(x,w)+{\operatorname{CS}}(y,w).\end{equation}

$$b(x,w)^2\cong_\nu cq(x)q(w),$$

$$b(y,w)^2\cong_\nu dq(y)q(w).$$

\begin{equation}\label{eq:II.6.13}
b(x+y,w)^2\cong_\nu[cq(x)+dq(y)]q(w).\end{equation}

$$ac+bd\le_\nu(a+b)(c+d),$$

$$a+b\le_\nu q(x)+q(y)+b(x,y)=q(x+y).$$

$$b(x+y,w)^2\le_\nu (a+b)(c+d)q(w)\le_\nu(c+d)q(x+y)q(w).$$

$$b(x+y,w)^2<_\nu (c+d)q(x+y)q(w),$$

$$ac+bd\cong_\nu (a+b)(c+d).$$

\begin{equation}\label{eq:II.7.1}
{\alpha}_1 := q(x), \qquad {\alpha}_2 := q(y), \qquad {\alpha} := b(x,y).
\end{equation}

$$\chi : R {\varepsilon}_1 + R {\varepsilon}_2 {\ {\to} \ } V$$

$$ q = \begin{bmatrix} {\alpha}_1& {\alpha}\\   &   {\alpha}_2\end{bmatrix}, $$

\begin{equation}\label{eq:II.7.2}
  {\alpha} \cong_\nu {\zeta} {\alpha}_1, \qquad {\alpha}_2 \cong_\nu \eta {\alpha},
  \end{equation}

\begin{equation}\label{eq:II.7.3}
  \eta {\zeta}  \cong_\nu {\xi}^2.
  \end{equation}

\begin{equation}
  {\alpha} = {\zeta} {\alpha}_1, \qquad {\alpha}_2 = \eta {\alpha},
\tag{\ref{eq:II.7.2}}\end{equation}

\begin{equation}
  \eta {\zeta} =  {\xi}^2.
\tag{\ref{eq:II.7.3}}\end{equation}

\begin{equation}\label{eq:II.7.4}
{\alpha}_1 {\alpha}_2 {<_\nu} {\alpha}^2 {\quad {\iff} \quad } \eta {<_\nu} {\zeta},
\end{equation}

\begin{equation}\label{eq:II.7.5}
\eta {\leq_\nu} \tau {<_\nu} {\xi} {<_\nu} {\sigma} {\leq_\nu} {\zeta},
\end{equation}

\begin{equation}\label{eq:II.7.6}
\eta {<_\nu} \tau {<_\nu} {\xi} {<_\nu} {\sigma} {<_\nu} {\zeta}.
\end{equation}

\begin{equation}
  \label{eq:II.7.7}
  q({\lambda} x + \mu y ) = \left\{
    \begin{array}{lll}
      {\lambda}^2 {\alpha}_1 & &  {\lambda} {>_\nu} {\zeta} \mu, \\[1mm]
      e {\lambda}^2 {\alpha}_1 = e {\lambda} \mu {\alpha}  &  & {\lambda} {\cong_\nu} {\zeta} \mu, \\[1mm]
      {\lambda} \mu {\alpha}  &  & \eta \mu {<_\nu} {\lambda} {<_\nu} {\zeta} \mu, \\[1mm]
       e \mu^2 {\alpha}_2 = e {\lambda} \mu {\alpha}  &  &  {\lambda} {\cong_\nu} \eta \mu, \\[1mm]
      \mu^2 {\alpha}_2 &  & {\lambda} {<_\nu} \eta \mu. \\
    \end{array}
  \right.
    \end{equation}

\begin{equation}\label{eq:II.7.8}
   q({\lambda} x + \mu y ) = \left\{
    \begin{array}{lll}
      {\lambda}^2 {\alpha}_1 & &  {\lambda} {>_\nu} {\sigma} \mu, \\[1mm]
      e {\lambda}^2 {\alpha}_1 = e {\lambda} \mu {\alpha}  &  & {\lambda} {\cong_\nu} {\sigma} \mu, \\[1mm]
       e \mu^2 {\alpha}_2 = e {\lambda} \mu {\alpha}  &  &  {\lambda} {\cong_\nu} \tau \mu, \\[1mm]
      \mu^2 {\alpha}_2 &  & {\lambda} {<_\nu} \tau \mu. \\
    \end{array}
  \right.
  \end{equation}

\begin{equation}\label{eq:II.7.9}
   q({\lambda} x + \mu y ) = \left\{
    \begin{array}{lll}
      {\lambda}^2 {\alpha}_1 & &  {\lambda} {>_\nu} {\xi} \mu , \\[1mm]
       e {\lambda}^2 {\alpha}_1 = e \mu^2 {\alpha}_2  &  &  {\lambda} {\cong_\nu} {\xi} \mu, \\[1mm]
      \mu^2 {\alpha}_2 &  & {\lambda} {<_\nu} {\xi} \mu. \\
    \end{array}
  \right.
  \end{equation}

\begin{equation}\label{eq:II.7.10}
   q({\lambda} x + \mu y ) = \left\{
    \begin{array}{lll}
      {\lambda}^2 {\alpha}_1 & &  {\lambda} {>_\nu} {\xi} \mu, \\[1mm]
       \mu^2 {\alpha}_2 &  & {\lambda} {<_\nu} {\xi} \mu. \\
    \end{array}
  \right.
  \end{equation}

$$ q({\lambda} x + \mu y) = {\lambda}^2 {\alpha}_1 + \mu^2 {\alpha}_2,$$

$$ q({\lambda} x + \mu y ) = {\lambda}^2 {\alpha}_1 + {\lambda} \mu {\alpha} + \mu^2 {\alpha}_2.$$

\begin{equation}\label{eq:II.7.11}
   q({\lambda} x + \mu y ) = \left\{
    \begin{array}{lll}
      {\lambda}^2 {\alpha}_1 & \text{if} &  {\lambda} {>_\nu} {\zeta} \mu,  \\[1mm]
      e {\lambda}^2 {\alpha}_1  = e {\lambda} \mu  {\alpha} & \text{if}  &  {\lambda} {\cong_\nu} {\zeta} \mu , \\[1mm]
       {\lambda} \mu {\alpha}  & \text{if}  & {\lambda} {<_\nu} {\zeta} \mu . \\
    \end{array}
  \right.
  \end{equation}

\begin{equation} \label{eq:II.7.12} q( {\lambda} x + \mu y )  = {\lambda} \mu {\alpha}.
  \end{equation}

$$ eq({\lambda} x + \mu y) = q ((e{\lambda})x + (e\mu)y).$$

\begin{equation}\label{eq:II.7.13}
x' = {\lambda}_1 x + \mu_1 y, \qquad y' = {\lambda}_2 x + \mu_2 y,
\end{equation}

\begin{equation}\label{eq:II.7.14}
{\lambda}_1 \mu_2  {\ {{>_\nu}} \ } {\lambda}_2 \mu_1,
\end{equation}

\begin{equation}\label{eq:II.7.15}
b(x,x) = b(y,y) = 0, \qquad b(x,y) = {\alpha},
\end{equation}

\begin{equation}\label{eq:II.7.16}
b(x', y') = {\lambda}_1 \mu_2 {\alpha}.
\end{equation}

\begin{equation}\label{eq:II.7.17}
{\operatorname{CS}}(x,y) = \bigg[ \frac{{\alpha}^2}{ {\alpha}_1 {\alpha}_2} \bigg]  = \bigg[ \frac{{\zeta}^ 2 {\alpha}_1^2 }{ {\zeta} \eta {\alpha}_1^2} \bigg] = \bigg[ \frac{\zeta}{ \eta} \bigg].
\end{equation}

\begin{equation}\label{eq:II.7.18}
z := {\zeta} x + y, \qquad w := \eta x + y
\end{equation}

$$q(z) = e {\zeta}^2 {\alpha}_1, \quad q(w) = e {\alpha}_2, \quad b(z,w) = {\zeta} {\alpha} = {\zeta}^2 {\alpha}_1;$$

\begin{equation}\label{eq:II.7.19}
{\operatorname{CS}}(z,w) = \bigg[ \frac{{\zeta}^4 {\alpha}_1^2}{ {\zeta}^2 {\alpha}_1 {\alpha}_2} \bigg]  = \bigg[ \frac{{\zeta}^ 2 {\alpha}_1^2 }{ {\zeta} \eta {\alpha}_1^2} \bigg] = \bigg[ \frac{\zeta}{ \eta} \bigg] {>_\nu} 1.
\end{equation}

\begin{equation}\label{eq:II.7.20}
{\operatorname{CS}}(x,z) = \bigg[ \frac{{\alpha}^2}{ {\alpha}_1 \cdot {\zeta}^2 {\alpha}_1} \bigg]  {\cong_\nu} 1,
\end{equation}

\begin{equation}\label{eq:II.7.21}
{\operatorname{CS}}(w,y) = \bigg[ \frac{\eta ^2 {\alpha}^2}{ {\alpha}_1 \cdot {\alpha}_2} \bigg]  {\cong_\nu} 1.
\end{equation}

\begin{equation}\label{eq:II.7.22}
{\operatorname{CS}}(x',y') \leq \bigg[ \frac{\zeta}{\eta} \bigg] = {\operatorname{CS}}(x,y)
\end{equation}

\begin{equation}\label{eq:II.7.23}
{\operatorname{CS}}(x',y') = \bigg[ \frac{{\lambda}_1 ^2  \mu_2 ^2 {\alpha}^2}{ {\lambda}_1^2 {\alpha}_1 {\lambda}_2^2 {\alpha} } \bigg]  =
\bigg[ \frac{ \mu_2 ^2 {\zeta} ^2}{{\lambda}_2^2 } \bigg] {\leq_\nu} 1.
\end{equation}

\begin{equation}\label{eq:II.7.24}
{\operatorname{CS}}(x',y') = \bigg[ \frac{{\lambda}_1 ^2  \mu_2 ^2 {\alpha}^2}{ \mu_1^2 {\alpha}_1 \mu_2^2 {\alpha}_2 } \bigg]  =
\bigg[ \frac{ {\lambda}_1 ^2 {\alpha} ^2}{\mu_1^2 {\alpha}_2^2 } \bigg] =
\bigg[ \frac{ {\lambda}_1 ^2 }{\mu_1^2 \eta^2 } \bigg] {\leq_\nu} 1.
\end{equation}

\begin{equation}\label{eq:II.7.25}
{\operatorname{CS}}(x',y') = \bigg[ \frac{{\lambda}_1 ^2  \mu_2 ^2 {\alpha}^2}{{\lambda}_1 {\lambda}_2  \mu_1  \mu_2 {\alpha}^2 } \bigg]  =
\bigg[ \frac{ {\lambda}_1 \mu_2 }{\mu_1 {\lambda}_2 } \bigg] {>_\nu} 1.
\end{equation}

\begin{equation}\label{eq:II.7.26}
{\operatorname{CS}}(x',y') = \bigg[ \frac{{\zeta}  \mu_2 }{ {\lambda}_2} \bigg]  = {\operatorname{CS}}(z,y').
\end{equation}

\begin{equation}\label{eq:II.7.27}
{\operatorname{CS}}(x',y') = \bigg[ \frac{{\lambda}_1 }{ \mu_1 \eta} \bigg]  = {\operatorname{CS}}(x',w).
\end{equation}

\begin{equation}\label{eq:II.7.28}
{\operatorname{CS}}(x',y') =
\left\{
  \begin{array}{ll}
    \big[ \frac{  \mu_2 ^2 {\zeta}^2}{ {\lambda}_2^2} \big]  {\leq_\nu} 1  & \text{if } {\lambda}_2 {\geq_\nu} {\zeta} \mu_2; \\[2mm ]
        \big[ \frac{  \mu_2  {\zeta}}{ {\lambda}_2} \big]  {>_\nu} 1  & \text{if } {\lambda}_1 {\geq_\nu} {\zeta} \mu_1 \text{ and } {\lambda}_2 {<_\nu} {\zeta} \mu_2 ; \\[2mm]
        \big[ \frac{  {\lambda}_1 \mu_2}{ {\lambda}_2  \mu_1 } \big]  {>_\nu} 1  & \text{if } {\lambda}_1 {\leq_\nu} {\zeta} \mu_1.  \\
  \end{array}
\right.
\end{equation}

\begin{equation}\label{eq:II.7.29}
{\operatorname{CS}}(x',y') = \bigg[ \frac{{\lambda}_1 ^2  \mu_2 ^2 {\alpha}^2}{{\lambda}_1 \mu_1 {\alpha}  \cdot {\lambda}_2    \mu_2 {\alpha}  } \bigg]  =
\bigg[ \frac{ {\lambda}_1 \mu_2 }{\mu_1 {\lambda}_2 } \bigg] {>_\nu} 1.
\end{equation}

\begin{equation}\label{eq:II.8.1}
v(a)< v(b){\ {\Rightarrow} \ }{\varphi}(a+b)={\varphi}(b).\end{equation}

$$q=(q,v_1,v_2)=\begin{bmatrix} {\alpha}_1 & {\alpha}\\  &{\alpha}_2\end{bmatrix}$$

\begin{equation}\label{eq:II.8.2}
q^{\varphi}:=(q,v_1,v_2)^{\varphi}=\begin{bmatrix}{\varphi}({\alpha}_1) & {\varphi}({\alpha})\\  & {\varphi}({\alpha}_2)\end{bmatrix} \end{equation}

\begin{equation}\label{eq:II.8.3}
 b^{\varphi}=(b,v_1,v_2)^{\varphi}=\begin{pmatrix} {\varphi}(2){\varphi}({\alpha}_1) & {\varphi}({\alpha})\\ {\varphi}({\alpha}) &{\varphi}(2){\varphi}({\alpha}_2)\end{pmatrix}\end{equation}

$$v_1'=a_{11}v_1+a_{12}v_2,\qquad v_2'=a_{21}v_1+a_{22}v_2,$$

$$(q,v_1',v_2')=\begin{bmatrix} a_{11}a_{12} & a_{11}a_{22}+a_{12}a_{21}\\
 & a_{21}a_{22}\end{bmatrix}.$$

$${\tilde q}:=(q,v_1',v_2')^{\varphi},\qquad {\tilde b}:=(b,v_1',v_2')^{\varphi}.$$

\begin{equation}\label{eq:II.8.4}
{\tilde q}=\begin{bmatrix} {\varphi}(a_{11}a_{12})& {\varphi}(a_{11}a_{22}+a_{12}a_{21})\\  & {\varphi}(a_{21}a_{22})\end{bmatrix}.
\end{equation}

$${\tilde q}=\begin{bmatrix} {\varphi}(a_{11}a_{12}) & {\varphi}(a_{11}a_{22})\\  & {\varphi}(a_{21}a_{22})\end{bmatrix}.$$

$${\tilde b}=\begin{pmatrix} {\varphi}(2a_{11}a_{12}) & {\varphi}(a_{11}a_{22})\\
{\varphi}(a_{11}a_{22})& {\varphi}(2a_{21}a_{22})\end{pmatrix}.$$

$${\tilde q}=c\begin{bmatrix} b_1 &1\\  & b_2\end{bmatrix},\qquad {\tilde b}=c\begin{pmatrix}{\varphi}(2)b_1 & 1\\ 1 & {\varphi}(2)b_2\end{pmatrix},$$

\begin{align*}c&: = {\varphi}(a_{11}a_{22})\in{\mathcal T},\\
 b_1&:=\frac{{\varphi}(a_{12})}{{\varphi}(a_{22})}\in{\mathcal T}\cup\{0\},\\
 b_2&:=\frac{{\varphi}(a_{21})}{{\varphi}(a_{11})}\in{\mathcal T}\cup\{0\},\end{align*}

$${\operatorname{CS}}({\varepsilon}_1,{\varepsilon}_2)\cong_\nu\frac{1}{b_1b_2}$$

$${\tilde q}=\begin{bmatrix} {\varphi}(a_{11}a_{12}) & {\varphi}(a_{12}a_{21})\\
  & {\varphi}(a_{21}a_{22})\end{bmatrix},$$

$${\tilde q}=c\begin{bmatrix} b_1 & 1\\  & b_2\end{bmatrix},\qquad{\tilde b}=c\begin{pmatrix} {\varphi}(2)b_1 & 1\\ 1 & {\varphi}(2)b_2,\end{pmatrix}$$

$${\operatorname{CS}}({\varepsilon}_1,{\varepsilon}_2)\cong_\nu \frac{1}{b_1b_2}.$$

$$ v(x+y) {\ {\leq} \ } v(x) + v(y) \quad [= \max\{ v(x), v(y)\}]$$

$${\tilde q}=\begin{bmatrix} {\varphi}(a_{11}a_{12}) & \gamma\\  & {\varphi}(a_{21}a_{22})\end{bmatrix}$$

$${\tilde q}=c\begin{bmatrix} b_1 &\delta\\  & b_2\end{bmatrix},\qquad {\tilde b}=c\begin{pmatrix} {\varphi}(2)b_1 & \delta\\
\delta & {\varphi}(2)b_2\end{pmatrix}$$

$$c={\varphi}(a_{11}a_{22})\in{\mathcal T},\qquad \delta\le_\nu1,$$

$$b_1=\frac{{\varphi}(a_{12})}{{\varphi}(a_{22})}\in{\mathcal T},\qquad b_2=\frac{{\varphi}(a_{21})}{{\varphi}(a_{11})}\in{\mathcal T}.$$

$${\tilde q}=[b_1,b_2]:=\begin{bmatrix} b_1 &0\\  & b_2\end{bmatrix}.$$

$$v_1'=a_{11}v_1+a_{12} v_2,\qquad v_2'=a_{21}v_1+a_{22}v_2$$

\begin{equation}\label{eq:II.8.5}
(q,v_1',v_2')=\begin{bmatrix} a_{11}^2 {\alpha} +a_{12}^2{\beta}& a_{11}a_{21}{\alpha}+a_{12}a_{22}{\beta}\\
 & a_{21}^2{\alpha}+a_{22}^2{\beta}\end{bmatrix}.
\end{equation}

$${\tilde q}:=(q,v_1',v_2')^{\varphi},\qquad{\tilde b}:=(b,v_1',v_2')^{\varphi}.$$

$$v(a_{11}a_{21}{\alpha})>v(a_{12}a_{22}{\beta}).$$

$${\tilde q}=\begin{bmatrix}{\varphi}(a_{11}^2{\alpha})& {\varphi}(a_{11}a_{21}{\alpha})\\  & {\varphi}(a_{21}^2{\alpha})
\end{bmatrix}.$$

\begin{equation}\label{eq:II.8.6}
{\tilde q}=[{\varphi}(a_{11}^2{\alpha}),{\varphi}(a_{21}^2{\alpha})]=[{\varphi}({\alpha}),{\varphi}({\alpha})].
\end{equation}

$$v(a_{11}a_{21}{\alpha})>v(a_{12}a_{22}{\beta}),$$

$${\tilde q}=\begin{bmatrix}{\varphi}(a_{11}^2{\alpha} + a_{12}^2{\beta}) & {\varphi}(a_{11}a_{12}{\alpha})\\  & {\varphi}(a_{21}^2{\alpha})\end{bmatrix}.$$

$$ v(a_{11}^2{\alpha} + a_{12}^2 {\beta}) = \max \{   v(a_{11}^2{\alpha}) , v( a_{12}^2 {\beta})\} $$

$${\tilde q}=\begin{bmatrix} {\varphi}(a_{11}^2{\alpha}) & {\varphi}(a_{11}a_{21}{\alpha}+a_{12}a_{22}{\beta})\\
 & {\varphi}(a_{22}^2{\beta})\end{bmatrix}.$$

\begin{align*}
{\operatorname{CS}}({\varepsilon}_1,{\varepsilon}_2)&=\frac{v(a_{11}a_{21}{\alpha}+a_{12}a_{22}{\beta})^2}{v(a_{11}^2a_{22}^2{\alpha}{\beta})}\\[1mm]
& \leq \frac{v(a_{11}^2a_{21}^2{\alpha}^2)}{v(a_{11}^2a_{22}^2{\alpha}{\beta})}+\frac{v(a_{12}^2a_{22}^2{\beta}^2)}{v(a_{11}^2a_{22}^2{\alpha}{\beta})}\\[1mm]
&=\frac{v(a_{21}^2{\alpha})}{v(a_{22}^2{\beta})}+\frac{v(a_{12}^2{\beta})}{v(a_{11}^2{\alpha})} {\ {<} \ }e.\end{align*}

$${\tilde q}=[{\varphi}(a_{11}^2{\alpha}),{\varphi}(a_{22}^2{\beta})]=[{\varphi}({\alpha}),{\varphi}({\beta})].$$

$$v(a_{11}^2{\alpha})\le v(a_{12}^2{\beta}),\qquad v(a_{21}^2{\alpha})>v(a_{22}^2{\beta}),$$

$$v(a_{11}^2{\alpha})<v(a_{12}^2{\beta}),\qquad v({\alpha}_{21}^2{\alpha})\le v(a_{22}^2{\beta}),$$

$$v(a_{11}^2{\alpha})<v(a_{12}^2{\beta}),\qquad v(a_{21}^2{\alpha})>v(a_{22}^2{\beta}),$$

\begin{equation}\label{eq:I.6.1}
x\le_Vy {\quad {\rightleftharpoons} \quad }\exists z\in V: x+z=y.
\end{equation}

$$x+e(z+w)=x,\quad y+e(z+w)=y.$$

$$y=x+e(z+w)=x,$$

\begin{gather}
 0\le z,\label{eq:I.6.2}\\
 x\le y {\quad {\Rightarrow} \quad } x+z\le y+z.\label{eq:I.6.3}
 \end{gather}

\begin{equation}\label{eq:I.6.4}
{\lambda} \le\mu,\ x\le y{\quad {\Rightarrow} \quad } {\lambda}  x\le \mu y
\end{equation}

\begin{equation}\label{eq:I.6.5}
\qquad x\le _V z {\quad {\Rightarrow} \quad } q(x)\le_R q(z),\end{equation}

\begin{equation}\label{eq:I.6.6}
x\le _V z,\ y\le_V w{\quad {\Rightarrow} \quad } b(x,y)\le_R b(z,w),\end{equation}

\begin{equation}\label{eq:I.6.7}
b(x,y) {\ {{\le_R}} \ }  q(x+y).\end{equation}

\begin{equation}\label{eq:I.6.8}
x<y {\quad {\Leftrightarrow} \quad } x<_\nu y,\end{equation}

\begin{equation}\label{eq:I.6.9}
y<x {\quad {\Leftrightarrow} \quad } \text{either}\ y<_\nu x\ ,  \text{or}\ y\in{\mathcal T}\ \text{and}\ y\cong_\nu x.\end{equation}

\begin{equation}\label{eq:I.6.10}
x<y{\quad {\Leftrightarrow} \quad } \text{either}\ x <_\nu y\ , \text{or}\ x\cong_\nu y\ \text{and}\ y\in eR,\end{equation}

\begin{equation}\label{eq:I.6.11}
y<x {\quad {\Leftrightarrow} \quad }   y<_\nu x.\end{equation}

\begin{equation}\label{eq:I.6.13}
x \vee y{\quad {=} \quad } \left\{
                  \begin{array}{ll}
                    x & \hbox{if \ } ex < ey; \\
                    y & \hbox{if \ } ex > ey;\\
                    ex & \hbox{if \ } ex =  ey.
                  \end{array}
                \right.
\end{equation}

\begin{equation}\label{eq:I.6.13}
e(x \vee y) = (ex)\vee (ey) = ex + ey,
\end{equation}

$$x=\sum_{i\in I}x_i{\varepsilon}_i\quad y=\sum_{i\in I}y_i{\varepsilon}_i,$$

\begin{equation}\label{eq:I.6.14}
x\le_Vy {\quad {\Leftrightarrow} \quad } \forall i\in I\quad x_i\le_Ry_i.\end{equation}

\begin{equation}\label{eq:I.6.15}
x\vee y {\quad {=} \quad }  \sum _{i \in I} (x_i \vee y_i){\varepsilon}_i.\end{equation}

\begin{equation}\label{eq:I.6.16}
{\operatorname{supp}}(x) := \{  i \in I {\ {|} \ } x_i \neq 0\}.    \end{equation}

\begin{equation}\label{eq:I.6.17}
{\operatorname{supp}}(x \vee y) ={\operatorname{supp}}(x) \cup {\operatorname{supp}}(y).    \end{equation}

$$y\le x {\quad {\Rightarrow} \quad } {\phi}  (y)\le{\phi}  (x).$$

$$(x_1,\dots, x_n) {\ {\mapsto} \ } cx_1^{{\alpha} _1}\cdots x_n^{{\alpha} _n}, \qquad ({\alpha} _i\in{\mathbb N}_0),$$

\begin{equation}
q(x)=\sum_{i\in J }x _i^2q({\varepsilon}_i)+\sum_{\substack{i<j\\i,j\in J }}x _ix _j
b({\varepsilon}_i,{\varepsilon}_j).\tag{}
\end{equation}

$$ q(x) = x_k x_\ell b({\varepsilon}_k, {\varepsilon}_\ell) \leq q(x_k {\varepsilon}_k +  x_\ell {\varepsilon}_\ell) \leq q(x).$$

$$q(x')={\lambda} '{}^2{\alpha} _1<_\nu{\lambda} ^2{\alpha} _1=q(x),$$

$$q(x')\leq q({\lambda} '{\varepsilon}_1+\mu{\varepsilon}_2)=\mu^2{\alpha} _2<e\mu^2{\alpha} _2=q(x).$$

\begin{equation}\label{eq:sstr}
q(x) = {\alpha}_1 x_1^2 + {\beta} x_1 x_2 + {\alpha}_2 x_2^2.
\tag{}
\end{equation}

$$x( J ):=\sum_{i\in  J } x_i{\varepsilon}_i.$$

$$x=\sum_{i=1}^n x_i{\varepsilon}_i,\quad\text{all}\quad x_i\ne0.$$

\begin{equation}\label{eq:7.1}
q(x)=\sum_{i=1}^n{\alpha}_ix_i^2+\sum_{i<j}{\beta}_{ij}x_ix_j.
\end{equation}

$$x=x(i)\vee x(j,k),$$

$$q(x(j,k))={\alpha}_jx_j^2+{\beta}_{ik}x_jx_k+{\alpha}_kx_k^2\in {\mathcal T}.$$

$${\alpha}_jx_j^2+{\alpha}_kx_k^2<_\nu {\beta}_{jk}x_jx_k,$$

$$b(x(i),x(j,k))<_\nu q(x(i)) \cong_\nu q(x).$$

\begin{equation}\label{eq:7.2}
q(x)\cong_\nu{\beta}_{ij}x_ix_j\cong_\nu{\beta}_{ik}x_ix_k>_\nu{\beta}_{jk}x_jx_k,
\end{equation}

\begin{equation}\label{eq:7.3}
q(x)\cong_\nu{\beta}_{12}x_1x_2\cong_\nu{\beta}_{13}x_1x_3 \cong_\nu{\beta}_{23}x_2x_j.
\end{equation}

\begin{align*}
b(x(j),x(k))<_\nu q(x(i,j))\cong_\nu q(x(i,k))
&\cong_\nu q(x), \end{align*}

$$b (x(r),x(s))\cong_\nu q(x(r,s))\cong_\nu q(x).$$

$$q(x(J))\cong_\nu q(x(K))\cong_\nu q(x),$$

$$b(x(S),x(T))<_\nu q(x).$$

$$q(x(J))\cong_\nu q(x(K))\cong_\nu q(x).$$

\begin{equation}\label{eq:7.4}
b(x(J),x(K))<_\nu q(x). \end{equation}

\begin{equation}\label{eq:7.5}
b(x(J),x(K))= q(x), \end{equation}

\begin{equation}\label{eq:7.6}
b(x(J{\setminus} K),x(K{\setminus} J))\cong_\nu q(x). \end{equation}

\begin{equation}\label{eq:7.7}
b(x(J{\setminus} K),x(K{\setminus} J))\cong_\nu q(x),\quad
b(x(J{\setminus} K),x(K{\setminus} J)\in {\mathcal T}.
\end{equation}

\begin{equation}\label{eq:7.6.b}
b(y,z)\le_\nu q(y)\cong_\nu q(z).
\end{equation}

\begin{equation}\label{eq:7.7.b}
b(y,z)<_\nu q(y)\cong_\nu q(z).
\end{equation}

$$y=y_1{\varepsilon}_1,\qquad z=z_2{\varepsilon}_2+z_3{\varepsilon}_3,$$

$$x_1=y_1,\qquad x_2=z_2,\qquad x_3=z_3.$$

\begin{equation}\label{eq:7.8}
{\alpha}_2x_2^2+{\alpha}_3x_3^2<_\nu{\beta}_{23}x_2x_3=q(z)\in{\mathcal T}.\end{equation}

\begin{equation}\label{eq:7.9}
{\beta}_{11}x_1^2+{\beta}_{12}x_1x_2+{\beta}_{13}x_1x_3<_\nu{\alpha}_1x_1^2\cong_\nu{\beta}_{23}x_2x_3.
\end{equation}

$$q(x)={\alpha}_1x_1^2+{\beta}_{23}x_2x_3=eq(y)=eq(z).$$

$$\sum_1^3{\alpha}_ix_i'{}^{2}+\sum_{i<j}{\beta}_{ij}x_i'x_j'=q(x')$$

$$q(x')={\beta}_{23}x_2x_3\in {\mathcal T},\quad\text{and}\quad
q(x')\cong_\nu q(x).$$

$$y=y_1{\varepsilon}_1+y_2{\varepsilon}_2,\qquad
z=z_3{\varepsilon}_3+z_4{\varepsilon}_4,$$

$$x_1=y_1,\qquad x_2=y_1,\qquad x_3=z_3,\qquad x_4=z_4.$$

\begin{gather}
{\alpha}_1x_1^2+{\alpha}_2x_2^2<_\nu{\beta}_{12}x_1x_2=q(y)\in {\mathcal T},\\
{\alpha}_3x_3^2+{\alpha}_4x_4^2<_\nu{\beta}_{34}x_3x_4=q(z)\in {\mathcal T},
\end{gather}

$${\beta}_{13}x_1x_3+{\beta}_{14}x_1x_4+{\beta}_{23}x_2x_3+{\beta}_{24}x_2x_4<_\nu
q(y)\cong_\nu q(z).$$

\begin{align*}
q(x')&={\beta}_{12}x_1'x_2+{\beta}_{34}x_3x_4 = {\beta}_{34}x_3x_4.
\end{align*}

$$x:=y\vee z=x_1{\varepsilon}_1+x_2{\varepsilon}_2+x_3{\varepsilon}_3$$

$$x_1=ey_1,\qquad x_2=y_2,\qquad x_3=z_3.$$

$$q(y)={\beta}_{12}y_1y_2\cong_\nu{\beta}_{13}z_1z_3=q(z).$$

$$b(y_1{\varepsilon}_1,z_1{\varepsilon}_1)\le_\nu
{\alpha}_1y_1^2\cong_\nu{\alpha}_1z_1^2$$

$$b(y,z)={\beta}_{11}y_1z_1+{\beta}_{12}z_1y_2+{\beta}_{13}y_1z_3=eq(y)=eq(z).$$

$$q(x)=q(y)+q(z)+b(y,z)=eq(y).$$

$$q(x')\ge {\beta}_{12}y_1y_2+{\beta}_{13}y_1z_3=eq(y).$$

\begin{equation}\label{eq:7.10}
b(y(J\setminus K),z(K\setminus J))<_\nu q(y)\cong_\nu q(z);
\end{equation}

\begin{equation}\label{eq:7.11}
b(y(J\setminus K),z(K\setminus J))\in {\mathcal T},\quad
b(y(J\setminus K),z(K\setminus J))\cong_\nu q(y)\cong_\nu q(z).
\end{equation}

$$y=y_1{\varepsilon}_1+y_2{\varepsilon}_2,\qquad
z=z_1{\varepsilon}_1+z_3{\varepsilon}_3$$

$$x_1=y_1 = z_1,\qquad x_2=y_2,\qquad x_3=z_3.$$

\begin{align*}
&x_1'<x_1,\quad x_2'=x_2,\quad x_3'=x_3\quad\text{or}\\
&x_1'=x_1,\quad x_2'<x_2,\quad x_3'=x_3.
\end{align*}

$$b(y(J\setminus K),z(K\setminus
J))=b(y_2{\varepsilon}_2,z_3{\varepsilon}_3)={\beta}_{23}x_2x_3,$$

$${\beta}_{12}x_1'x_2<_\nu {\beta}_{12}x_1x_2,\quad
{\beta}_{13}x_1'x_3<_\nu{\beta}_{13}x_1x_3.$$

$${\beta}_{12}x_1x_2<_\nu {\beta}_{12}x_1x_2,\qquad
{\beta}_{23}x_2'x_3<_\nu{\beta}_{23}x_2x_3.$$

$$q(x')={\beta}_{13}x_1x_3\cong_\nu q(x).$$

$$q(x')={\beta}_{23}x_2x_3\cong_\nu q(x),$$

$$q(x')={\beta}_{13}x_1x_3\cong_\nu q(x).$$

\begin{equation}\label{eq:7.12}
\sum_1^n{\alpha}_ix_i^2+\sum_{i<j}{\beta}_{ij}x_ix_j=q(x)
\end{equation}

$${\alpha}_1y_1^2+{\alpha}_2y_2^2<{\beta}_{12}y_1y_2 = q(y)\in {\mathcal T}.$$

\end{document}