\documentclass[10pt, reqno]{article}


\usepackage{amssymb,latexsym}

\usepackage{eucal}

\usepackage{tikz}

\begin{document}


\begin{equation}\label{di}
\bar {\mathrm{r}}(H_1\cap H_2)  \le  2\tfrac{q^*}{q^*-2}
 \bar {\mathrm{r}}(H_1) \bar {\mathrm{r}}(H_2)  .
\end{equation}

\begin{equation}\label{conj}
 \bar {\mathrm{r}}(H_1\cap H_2)  \le  \tfrac{q^*}{q^*-2}
 \bar {\mathrm{r}}(H_1) \bar {\mathrm{r}}(H_2)  .
 \end{equation}

$$
\bar {\mathrm{r}}(H_1\cap H_2)  \le  \tfrac{q^*}{q^*-2}  \bar {\mathrm{r}}(H_1) \bar {\mathrm{r}}(H_2) = 3  \bar {\mathrm{r}}(H_1) \bar {\mathrm{r}}(H_2) .
$$

\begin{equation}\label{HNC}
\bar {\mathrm{r}}(H_1\cap H_2)  \le   \bar {\mathrm{r}}(H_1) \bar {\mathrm{r}}(H_2) .
 \end{equation}

\begin{equation}\label{imrn}
  \bar {\mathrm{r}}(H_1\cap H_2)  \le   \left(2 - \tfrac{(4+2\sqrt{3})p}{(2p-3+\sqrt{3})^2} \right) \cdot \tfrac{p}{p-2}  \bar {\mathrm{r}}(H_1) \bar {\mathrm{r}}(H_2)
 \end{equation}

\begin{equation}\label{conjs}
\bar {\mathrm{r}}(H_1, H_2) :=   \sum_{s \in S(H_1, H_2)} \bar {\mathrm{r}}(H_1\cap s H_2 s^{-1})
\le \tfrac{q^*}{q^*-2}   \bar {\mathrm{r}}(H_1) \bar {\mathrm{r}}(H_2)  ,
\end{equation}

\begin{equation}\label{dfy0}
{\bar {\mathrm{r}}} (H_1 , H_2) \le \sigma(H_1)  {\bar {\mathrm{r}}}(H_1) {\bar {\mathrm{r}}}(H_2)
\end{equation}

$$
\sigma(H_1)  = \sup \{ \tfrac{{\bar {\mathrm{r}}} (H_1,  H_2)}{{\bar {\mathrm{r}}} (H_1) {\bar {\mathrm{r}}} (H_2) } \}
$$

\begin{equation}\label{dfy0d}
\sigma_d(H_1)  := \sup \{ \tfrac{{\bar {\mathrm{r}}} (H_1 ,  H_2)}{{\bar {\mathrm{r}}} (H_1) {\bar {\mathrm{r}}} (H_2) } \}
\end{equation}

$$
\tfrac{p}{p-2} \le   \sigma_d(H_1)\le \sigma(H_1)  \le   \left(2 - \tfrac{(4+2\sqrt{3})p}{(2p-3+\sqrt{3})^2} \right) \cdot \tfrac{p}{p-2} .
$$

\begin{equation}\label{lpa}
{\mathcal{P}}(H_1, d) = \max\{ c(d)x(d) \mid A(d)x(d) \le b(d)  \}
\end{equation}

$$
{\mathcal{P}}^*(H_1, d) = \min \{ b(d)^{\top}  y(d)  \mid A(d)^{\top}y(d) = c(d)^{\top} , \, y(d) \ge 0  \}
$$

$$
| E  \Psi(H_2^*) | < 2^{  2^{4| E  \Psi(H_1) | + 1+ \log_2 \log_2 (2d)  } } .
$$

$$
{\mathcal{P}}^*(H_1)  = \inf \{ b^{\top} y \mid A^{\top} y = c^{\top} , \, y \ge 0  \}
$$

$$
d' := \max\{ |I_1 \cup I_2| , \max\{ |G_{\alpha} | \, : \,   {\alpha} \in I_1 \cup I_2 \} \} .
$$

\begin{equation*}
{\varphi} : E\Psi \to {\mathcal{A}} , \qquad {\theta} :  V_S \Psi \to I ,
\end{equation*}

$$
{\theta}(e_{i,j}) := {\alpha}(i,j),  \quad {\theta}(f_{i,j}) := {\alpha}(i,j) , \quad {\varphi}(e_{i,j}) := a_{i,j}b_{i,j}^{-1},  \  {\varphi}(f_{i,j}) := b_{i,j} ,
$$

$$
\tau_i : V_P \Psi_o'(H_1, H_2) \to V_P \Psi_{o_i}(H_i)
$$

$$
(e_i)_- = \tau_i(v) , \  (f_i)_- = \tau_i(w) ,  \ (e_i)_+ = (f_i)_+
$$

\begin{gather}\label{tau1}
\tau_i :  \Psi(H_1, H_2) \to  \Psi(H_i)  , \quad i=1,2 \, .
\end{gather}

$$
{\Omega}_T : T \to S_1(V_P Y_1) .
$$

\begin{gather}\label{cd1}
1 \le  | [(a, u)]_{ {\sim}_{{\Omega}_T} } | \le |T|   .
\end{gather}

$$
|[ (a, u)  ]_{{\sim}_{{\Omega}_T}} | \ge 2
$$

\begin{equation}\label{Nal}
N_{\alpha} ( {\Omega}_T ) := \sum ( |  [  (a, u) ]_{{\sim}_{{\Omega}_T}} | -2 )
\end{equation}

\begin{equation*}
N_{\alpha} ( {\Omega}_T ) = \sum ( |  [  (a, u) ]_{{\sim}_{{\Omega}_T}} | -2 )  \le
     |T|\cdot |V_P Y_1 | - 2r \le (|T| - 2) |V_P Y_1 | .
\end{equation*}

\begin{equation*}
N_{\alpha} ( {\Omega}_T ) = \sum ( |  [  (a, u) ]_{{\sim}_{{\Omega}_T}} | -2 )  \le
   (|T| -2 ) r   \le (|T| - 2) |V_P Y_1 |  .
\end{equation*}

\begin{equation}\label{cd2}
N_{\alpha} ( {\Omega}_T )\le (|T| - 2) |V_P Y_1 |  .
\end{equation}

\begin{equation}\label{inqa}
- x_{A_1} -\dots  - x_{A_{k}}  - (k-2)x_s \le   - N_1(\Omega_T)   .
\end{equation}

\begin{equation}\label{inqb}
 x_{A_1} +\dots  + x_{A_{k}}  - (k-2)x_s \le   - N_2(\Omega_T)   .
\end{equation}

\begin{equation}\label{slid}
\operatorname{\textsf{SLI}}_d[Y_1]
\end{equation}

$$
 {\Omega}_{T_u} : T_u \to S_1(V_P Y_1)
 $$

\begin{equation*}
\operatorname{\textsf{inq}}_S : V_S Y_2 \to \operatorname{\textsf{SLI}}[Y_1]
\end{equation*}

\begin{equation*}\label{inc2}
\sum_{u \in V_S Y_2}  \operatorname{\textsf{inq}}_S(u)^L = -2 {\bar {\mathrm{r}}} (Y_2) x_s  \, ,   \ \mbox{and}  \
\sum_{u \in  V_S Y_2}  \operatorname{\textsf{inq}}_S(u)^R = -2 {\bar {\mathrm{r}}} ( \operatorname{core}(Y_1 \times  Y_2) )   .
\end{equation*}

$$
\sum_{u \in V_S Y_2 } \operatorname{\textsf{inq}}_S(u)^L ,
$$

\begin{equation}\label{add1a}
\sum_{u \in V_S Y_2}  (\deg u -2) = 2 {\bar {\mathrm{r}}} (Y_2)  ,
\end{equation}

\begin{equation*}
\sum_{u \in V_S (\operatorname{core}(Y_1 \times  Y_2))}  (\deg u -2) = 2{\bar {\mathrm{r}}} (\operatorname{core}(Y_1 \times  Y_2)) ,
\end{equation*}

$$
\sum_{q \in  \operatorname{\textsf{inq}} (V_S  Y_2) }^{}q^L := \sum_{j=1}^{m}q_j^L = - 2 {\bar {\mathrm{r}}}(Y_2)  x_s  .
$$

\begin{equation}\label{l2i11}
\sum_{q \in  Q}^{}q^L = -C x_s  ,
\end{equation}

\begin{equation}\label{l2i2}
\sum_{q \in  \operatorname{\textsf{inq}}( V_S Y_Q)}^{}q^L = - 2{\bar {\mathrm{r}}}(Y_Q) x_s \quad  \mbox{and}   \quad
\sum_{q \in  \operatorname{\textsf{inq}}(V_S Y_Q)}^{}q^R = - 2 {\bar {\mathrm{r}}}(\operatorname{core}(Y_1  \times  Y_Q))   .
\end{equation}

$$
{\Omega}_j : T_j \to S_1( V_P Y_1) ,
$$

$$
(-1)^{{\alpha}_j}x_{ {\Omega}_j(b_{\ell,j})} \quad \mbox{and} \quad  (-1)^{{\alpha}_{j'}}x_{ {\Omega}_{j'}(b_{\ell',j'})}
$$

$$
\tau_Q : \operatorname{core}(  Y_1  \times  Y_Q ) \to Y_Q
$$

\begin{equation*}\label{l2i1}
\sum_{q \in Q}^{}q^L   =    -2{\bar {\mathrm{r}}}(Y_2) x_s \quad  \mbox{and}   \quad
\sum_{q \in  Q}^{  }q^R = - 2{\bar {\mathrm{r}}}(\operatorname{core}(Y_1  \times  Y_2))   .
\end{equation*}

$$
cx= c_1x_1+\dots +c_nx_n
$$

$$
\max\{ cx \mid Ax \le b  \} .
$$

$$
 \min\{ cx \mid Ax \le b    \} = -  \max\{ -cx \mid Ax \le b    \}
 $$

$$
 \min\{ b^{\top}y \mid A^{\top}y = c^{\top}, y\ge 0  \} ,
 $$

\begin{equation}\label{dt}
\max\{ cx \mid Ax \le b    \}  =  \min\{ b^{\top}y \mid A^{\top}y = c^{\top}, y\ge 0  \}
\end{equation}

$$
\inf \{ b^{\top}y \mid A^{\top}y = c^{\top}, y\ge 0  \} ,
$$

\begin{equation}\label{dtt}
\sup \{ cx \mid Ax \le b    \}  \le   \inf \{ b^{\top}y \mid A^{\top}y = c^{\top}, y\ge 0  \}
\end{equation}

$$cx :=  -x_s$$

\begin{equation}\label{dlpp}
\sum_{j=1}^{\infty } y_j q_j^R \to \inf  \quad  \mbox{subject to} \quad   y \ge 0 , \  \
\sum_{j=1}^{\infty } y_j q_j^L = - x_s ,
\end{equation}

\begin{equation}\label{dlp}
\inf \{ \sum_{j=1}^{\infty} y_j q_j^R \mid  \sum_{j=1}^{\infty} y_j q_j^L = - x_s , y \ge 0  \} .
\end{equation}

\begin{equation*}
\sum_{j=1}^{i_d } y_j q_j^R \to \min  \quad   \mbox{subject to} \quad  y \ge 0,  \
\sum_{j=1}^{i_d} y_j q_j^L = - x_s
\end{equation*}

\begin{equation}\label{dlpd}
\min  \{ \sum_{j=1}^{i_d} y_j q_j^R \mid  \sum_{j=1}^{i_d} y_j q_j^L = - x_s , y \ge 0  \} .
\end{equation}

$$
\operatorname{\textsf{inq}}  :   Y_2 \to  \operatorname{\textsf{inq}}(Y_2)
$$

\begin{equation}\label{st1}
\sum_{q \in Q} q^L = -C(Q) x_s     ,
\end{equation}

\begin{equation}\label{st2}
     \sum_{q \in Q} q^L =  \sum_{j=1 }^{i_d} \delta_j \ell_j(Q) x_s =  -C(Q) x_s    .
\end{equation}

\begin{equation}\label{dfyy}
\operatorname{\textsf{sol}}_d :  Q \to y_Q = ( y_{Q,1}, \dots,  y_{Q, i_{d}} )^{\top}   ,
\end{equation}

$$
\sum_{j=1}^{i_{d}} y_{{Q,j}} q_j^L  = - x_s    .
$$

$$
\{ y \mid y \ge 0, \sum_{j=1}^{i_{d}} y_{j} q_j^L   = - x_s \}
$$

$$
\sum_{q \in Q} q^L =   \sum_{j=1}^{i_{d}} \ell_j q_j^L = \sum_{j=1}^{i_{d}} C {\widehat} y_{j}  q_j^L  =  C \sum_{j=1}^{i_{d}} {\widehat} y_{j}  q_j^L  = - C x_s  .
$$

\begin{equation}\label{ps4}
\sum_{j=1 }^{i_d}    {\widehat} y_{j}  q_j^R    =   -\frac{{\bar {\mathrm{r}}} (\operatorname{core}(Y_1 \times  Y_2))}{{\bar {\mathrm{r}}} (Y_2) }     .
\end{equation}

\begin{equation}\label{eqq1}
\sum_{q \in Q} q^L = - 2{\bar {\mathrm{r}}} (Y_2) x_s  \quad \mbox{ and} \quad  \sum_{q \in Q} q^R = - 2{\bar {\mathrm{r}}} (\operatorname{core}(Y_1 \times  Y_2) ) .
\end{equation}

\begin{equation*}
\sum_{j=1}^{i_d}  {\widehat} y_j q_j^R = ( \sum_{q \in Q } q^R  )
C(Q)^{-1} = -\frac {{\bar {\mathrm{r}}}( \operatorname{core}(Y_1 \times  Y_2) ) }{ {\bar {\mathrm{r}}}(Y_2 ) }   ,
 \end{equation*}

\begin{equation*}
{\bar {\mathrm{r}}} ( \operatorname{core}(Y_1 \times  Y_2) )  \le  \sigma(Y_1)  {\bar {\mathrm{r}}}(Y_1) {\bar {\mathrm{r}}}(Y_2)
\end{equation*}

\begin{equation*}
{\bar {\mathrm{r}}} ( \operatorname{core}(Y_1 \times  Y_2) )  \le  \sigma_d(Y_1)  {\bar {\mathrm{r}}}(Y_1) {\bar {\mathrm{r}}}(Y_2)
\end{equation*}

\begin{multline}
\label{st3}
- 2 \tfrac{q^*}{q^*-2} {\bar {\mathrm{r}}}(Y_1) \le \sup \{ - x_s \mid \operatorname{\textsf{SLI}} [Y_1]\}    \le   \max \{ - x_s \mid \operatorname{\textsf{SLI}}_d[Y_1]\}  = \\  = \min \{ \sum_{j=1}^{i_d}
 y_j q_j^R   \mid y \ge 0 , \ \sum_{j=1}^{i_d}   y_j q_j^L  = - x_s \} =
 - \sigma_d(Y_1) {\bar {\mathrm{r}}}(Y_1)  .
\end{multline}

\begin{multline}
\label{st3a}
\inf   \{  \sum_{j=1}^{\infty}   y_j q_j^R   \mid y \ge 0 , \
\sum_{j=1}^{\infty}   y_j q_j^L  = - x_s \} =  - \sigma(Y_1) {\bar {\mathrm{r}}}(Y_1) \\ \le
\min   \{  \sum_{j=1}^{i_d}   y_j q_j^R   \mid y \ge 0 , \
\sum_{j=1}^{i_d}   y_j q_j^L  = - x_s \} = - \sigma_d(Y_1)  {\bar {\mathrm{r}}}(Y_1) .
\end{multline}

$$
\{  y   \mid y \ge 0 , \sum_{j=1}^{\infty}  y_j q_j^L  = - x_s \} ,   \quad \{  y   \mid y \ge 0 , \sum_{j=1}^{i_d}  y_j q_j^L  = - x_s \}
$$

\begin{align}\label{dd1}
 -(k-2)\cdot 2\tfrac{q^*}{q^*-2} {\bar {\mathrm{r}}}(Y_1) \le -   N_{\alpha}(\Omega_T)
\end{align}

\begin{align}\label{dd2}
\sum_{g \in G_{\alpha}} \max(|T \cap Bg | -2, 0)  \le \tfrac{q^*}{q^*-2}(|T|-2)(|B|-2) =
\tfrac{q^*}{q^*-2}(k-2)(\ell-2) .
\end{align}

\begin{align*}
N_{\alpha}(\Omega)   \le \tfrac{q^*}{q^*-2} (k-2) \cdot 2 {\bar {\mathrm{r}}}_{\alpha} (Y_1)  \le \tfrac{q^*}{q^*-2} (k-2) \cdot 2 {\bar {\mathrm{r}}} (Y_1)    ,
\end{align*}

\begin{align*}
-x_s \ge  -\tfrac{2q^*}{q^*-2}  {\bar {\mathrm{r}}} (Y_1)  .
\end{align*}

$$
 \operatorname{\textsf{sol}}_d \circ \operatorname{\textsf{inq}} : Y_2 \to    {\widehat} y
$$

\begin{equation*}
\sigma_d(Y_1 )  {\bar {\mathrm{r}}}(Y_1 ) :=  \sup_{Y_2} \tfrac {{\bar {\mathrm{r}}}(  \operatorname{core}(Y_1 \times Y_2) ) }{ {\bar {\mathrm{r}}}(Y_2 ) }  =
- \inf_{Y_2}  \left( - \tfrac {{\bar {\mathrm{r}}}(  \operatorname{core}(Y_1 \times Y_2)  ) }{ {\bar {\mathrm{r}}}(Y_2 ) }  \right)
\end{equation*}

\begin{align*}
  \sigma_d(Y_1 )  {\bar {\mathrm{r}}}(Y_1 ) &  =  -\inf \{  \sum_{j=1}^{i_d}   y_j q_j^R   \mid y \ge 0 , \ \sum_{j=1}^{i_d}
 y_j q_j^L = - x_s \}   \\
  & =  - \min \{  \sum_{j=1}^{i_d}   y_j q_j^R   \mid y \ge 0 , \ \sum_{j=1}^{i_d}
 y_j q_j^L = - x_s \} \\ &  = -   \sum_{j=1}^{i_d}  {\widehat} y_j(d) q_j^R
  =  - \max \{ - x_s \mid \operatorname{\textsf{SLI}}_d[Y_1]\}   ,
\end{align*}

$$
\inf \{  \sum_{j=1}^{\infty}   y_j q_j^R   \mid y \ge 0 , \
\sum_{j=1}^{\infty}   y_j q_j^L  = - x_s \} =\inf_d  \min   \{  \sum_{j=1}^{i_d}   y_j q_j^R   \mid y \ge 0 , \
\sum_{j=1}^{i_d}   y_j q_j^L  = - x_s \}
$$

\begin{equation}\label{bol}
    \frac{{\bar {\mathrm{r}}}(H_1, H_4) }{  {\bar {\mathrm{r}}}(H_4) }  >  \frac{{\bar {\mathrm{r}}}(H_1, H_2) }{  {\bar {\mathrm{r}}}(H_2) }  . \end{equation}

$$
\tau_2 : \operatorname{core} (\Psi(H_1) \times \Psi(H_2)) \to  \Psi(H_2)
$$

$$
{\bar {\mathrm{r}}}(  \operatorname{core} (\Psi(H_1) \times \Gamma )  ) = {\bar {\mathrm{r}}}(  \operatorname{core} (\Psi(H_1) \times \Psi(H_2))  ) >0,
$$

\begin{equation}\label{e52}
\frac{{\bar {\mathrm{r}}}( \operatorname{core} (  \Psi(H_1) \times \Gamma   ))  }{  {\bar {\mathrm{r}}}(\Gamma ) }  > \frac{{\bar {\mathrm{r}}}( \operatorname{core} (  \Psi(H_1) \times \Psi(H_2)   ))  }{  {\bar {\mathrm{r}}}(\Psi(H_2) ) } .
\end{equation}

$$
{\bar {\mathrm{r}}}( \operatorname{core} (  \Psi(H_1) \times \Gamma )) >0 ,
$$

$$
{\bar {\mathrm{r}}}(\Gamma) = \sum_{j=1}^k {\bar {\mathrm{r}}}(\Gamma_j) , \qquad   {\bar {\mathrm{r}}}( \operatorname{core} (  \Psi(H_1) \times \Gamma )) = \sum_{j=1}^k {\bar {\mathrm{r}}}( \operatorname{core} (  \Psi(H_1) \times \Gamma_j )) ,
$$

\begin{equation}\label{e53}
\frac{{\bar {\mathrm{r}}}( \operatorname{core} (  \Psi(H_1) \times \Gamma   ))  }{  {\bar {\mathrm{r}}}(\Gamma ) } =  \frac{ \sum_{j=1}^k {\bar {\mathrm{r}}}( \operatorname{core} (  \Psi(H_1) \times \Gamma_j )) }{     \sum_{j=1}^k {\bar {\mathrm{r}}}(  \Gamma_j )      } .
\end{equation}

$$
\frac{  {\bar {\mathrm{r}}}( \operatorname{core} ( \Psi(H_1) \times \Gamma_{j^*} )) } {  {\bar {\mathrm{r}}}( \Gamma_{j^*} )      }
$$

$$
 \frac{ \sum_{j=1}^k {\bar {\mathrm{r}}}( \operatorname{core} (  \Psi(H_1) \times \Gamma_j )) }{     \sum_{j=1}^k {\bar {\mathrm{r}}}(  \Gamma_j )      }
  \le     \frac{  {\bar {\mathrm{r}}}( \operatorname{core} ( \Psi(H_1) \times \Gamma_{j^*} )) } {  {\bar {\mathrm{r}}}( \Gamma_{j^*} )      } .
  $$

$$
 \frac{  {\bar {\mathrm{r}}}( \operatorname{core} ( \Psi(H_1) \times \Gamma_{j^*} )) } {  {\bar {\mathrm{r}}}( \Gamma_{j^*} )      }  \ge
  \frac{  {\bar {\mathrm{r}}}( \operatorname{core} ( \Psi(H_1) \times \Gamma)) } {  {\bar {\mathrm{r}}}( \Gamma ) } >
  \frac{  {\bar {\mathrm{r}}}( \operatorname{core} ( \Psi(H_1) \times \Psi(H_2))) } {  {\bar {\mathrm{r}}}( \Psi(H_2) ) } .
  $$

$$
\sigma_d(H_1){\bar {\mathrm{r}}}(H_1 )   = \sigma_d( \Psi(H_1)){\bar {\mathrm{r}}}(\Psi(H_1)) \quad \mbox{and}  \quad
\sigma(H_1){\bar {\mathrm{r}}}(H_1) =  \sigma( \Psi(H_1)) {\bar {\mathrm{r}}}(\Psi(H_1)).
$$

$$\sup \frac{ {\bar {\mathrm{r}}}(   H_1, H_3  )  }{  {\bar {\mathrm{r}}}(H_3 ) }$$

$$
{\mathcal{F}}_2(1) =   G_1 *  G(2, m)
$$

\begin{equation}\label{map2}
a_{\alpha} \to
  (g_{{\alpha}+1} \ldots  g_{m}  g_{1} \ldots  g_{\alpha})^{-1}  a_{\alpha}   g_{{\alpha} +1} \ldots  g_{m}  g_{1} \ldots   g_{\alpha}   ,
\end{equation}

$$
 \mu : {\mathcal{F}} \to {\mathcal{F}} , \qquad \mu_2 : {\mathcal{F}} \to  {\mathcal{F}}_2(1)
 $$

$$
 \mu : {\mathcal{F}} \to {\mathcal{F}} , \quad \mu_2 :  {\mathcal{F}} \to {\mathcal{F}}_2(1) .
 $$

$$
W' \mu(U_1') (W')^{-1} \overset 0 =  \mu(U_2)
$$

$$
W \mu(U_1) W^{-1} \overset 0 = \mu(U_2)
$$

\begin{equation}\label{e54}
    \mu(U) \overset 0 = WVW^{-1}
\end{equation}

$$
\mu(U) \overset 0 = W' V' (W')^{-1} ,
$$

$$
{\bar {\mathrm{r}}}(K_1, K_2)   := \sum_{S \in S(K_1, K_2)}  {\bar {\mathrm{r}}}( K_1 \cap S K_2 S^{-1}) =
{\bar {\mathrm{r}}}(  \mu_2(K_1) , \mu_2(K_2) )  ,
$$

\begin{equation*}\tag{1.8}
{\mathcal{P}}(H_1, d) = \max\{ c(d)x(d) \mid A(d)x(d) \le b(d)  \}
\end{equation*}

$$
{\mathcal{P}}^*(H_1, d) = \min \{ b(d)^{\top}  y(d)  \mid A(d)^{\top}y(d) = c(d)^{\top} , \, y(d) \ge 0  \}
$$

$$
| E  \Psi(H_2^*) | < 2^{  2^{4| E  \Psi(H_1) | + 1+ \log_2 \log_2 (2d)  } } .
$$

$$
{\mathcal{P}}^*(H_1)  = \inf \{ b^{\top} y \mid A^{\top} y = c^{\top} , \, y \ge 0  \}
$$

\begin{equation}\label{lppf}
    \max \{ - x_s \mid \operatorname{\textsf{SLI}}_d[Y_1] \}  .
\end{equation}

$$
\sigma_d(Y_1){\bar {\mathrm{r}}}(Y_1) = \sup \frac{  {\bar {\mathrm{r}}} ( \operatorname{core}(Y_1 \times Y_2) )}{ {\bar {\mathrm{r}}}(Y_2) }
$$

\begin{equation}\label{fplh}
 \{  y \mid y \ge 0 , \ \sum_{j=1}^{i_d}   y_j q_j^L  = - x_s \}
 \end{equation}

\begin{equation}\label{hy2}
 \operatorname{\textsf{sol}}_d ( \operatorname{\textsf{inq}}( {\widehat} Y_2)) = {\widehat} y(d) \quad
  \mbox{and} \quad
  {\bar {\mathrm{r}}} (\operatorname{core}(Y_1 \times {\widehat}  Y_2))    =   \sigma_d(Y_1)   {\bar {\mathrm{r}}} (Y_1)  {\bar {\mathrm{r}}} ({\widehat} Y_2) .
 \end{equation}

\begin{equation}\label{upp}
| E {\widehat} Y_2 | <   2^{ 2^{4| E Y_1 | +1+ \log_2 (\log_2 2d)  } }
\end{equation}

\begin{align}\label{dlp2}
- \sigma_d(Y_1) {\bar {\mathrm{r}}}(Y_1) & =  \min   \{  \sum_{j=1}^{i_d}   y_j q_j^R   \mid y \ge 0 ,
\sum_{j=1}^{i_d}   y_j q_j^L  = - x_s \}  \\ \label{lp0}
  & =   \min \{ b^{\top}y \mid A^{\top}y = c^{\top}, y\ge 0  \}  \\   \label{lp2}
  & =  \max\{ cx \mid Ax \le b  \} =  \max \{ - x_s \mid \operatorname{\textsf{SLI}}_d[Y_1]\}   .
\end{align}

$$
A_{r \times r}^{\top}  \bar y(d)  = (c_1, \dots,  c_r)^{\top} = \bar c^{\top} .
$$

\begin{equation}\label{cr1}
| \det A_{r \times r} | <    d^{2r} .
\end{equation}

\begin{equation}\label{cr2}
{\widehat} y_{i}(d) = \frac{\det A_{r \times r, i}^{\top}(\bar c^{\top})}{  \det A_{r \times r}}  ,
\end{equation}

\begin{equation}\label{cr3}
| \det A_{r \times r, i}(\bar c^{\top}) | <  d^{2r-2}
\end{equation}

\begin{equation}\label{eQ}
|{\widehat}  Q | < r d^{2r-2}  ,
\end{equation}

\begin{equation}\label{cr4}
|  E {\widehat} Y_2 | \le  2d | V_S {\widehat}  Y_2 | = 2d |{\widehat}  Q | <  2d  r d^{2r-2} < 2 r d^{2r} .
\end{equation}

\begin{equation}\label{cr5}
r \le n \le (2^{|V_P Y_1 |}   - 1) + 1  = 2^{  4| E Y_1 |}
\end{equation}

\begin{align*}
| E {\widehat}  Y_2 |  & < 2 r d^{2r}  =   2^{ 4| E Y_1 | +1}  d^{   2^{  4| E Y_1 | +1}  }  <   2^{ 4| E Y_1|  +1 +  \log_2 d  \cdot 2^{ 4 | E Y_1 | +1 }  } \\ & <  2^{ (\log_2 d +1 )  \cdot 2^{4| E Y_1 | +1}   } \le 2^{  \log_2 (2d) \cdot 2^{4| E Y_1 | +1 } } \\
 & \le  2^{  2^{4| E Y_1 | +1+ \log_2 \log_2 (2d)  } }   .
\end{align*}

$$
0 \le N({{\Omega}}_T)_{\alpha} \le (d-2) |   V_P Y_1| ,
$$

\begin{equation}\label{t3t3}
    b_1 b_2^{-1} = {\varphi}(e_1) {\varphi}(e_2)^{-1}
\end{equation}

\begin{equation}\label{fscz}
{{\Omega}}_{ C \cup Z} : C \cup Z \to S_1(V_P Y_1) .
\end{equation}

$$
 \zeta_i(a) \zeta_i(b)^{-1} = {\varphi}(e) {\varphi}(f)^{-1}
 $$

$$
 Z_{i+1} := Z_{i} ,  \quad C_{i+1} := C_{i}  ,  \quad   \zeta_{i+1} := \zeta_{i} .
 $$

$$
Z_{i+1} := Z_{i}\cup \{ a \}  ,  \quad   C_{i+1} := C_{i}\cup \{ \eta(a) \}
$$

$$
Z_{i+1} := Z_{i}   ,  \quad    C_{i+1} := C_{i}  ,  \quad   \zeta_{i+1} := \zeta_{i} .
$$

$$
\zeta = \zeta_{i} : C \cup Z \to  C_i \subseteq G_{\alpha} ,
$$

$$
{{\Omega}}_{C \cup Z} : C \cup Z \to S_1(V_PY_1) ,
$$

$$
C_i({\alpha}, d) :=   C({\alpha}, d) \cap  (E_1 h_1 \cup \dots \cup E_i h_i )
$$

$$
e_1 b^{-1} c_1 \in R_{c_1} \cap (E_1 h_1 \cup \dots \cup E_i h_i) \quad \mbox{and}   \quad e_2 b^{-1} c_2 \in R_{c_2}\cap (E_1 h_1 \cup \dots \cup E_i h_i) ,
$$

$$
|C({\alpha}, d)|- | C_i({\alpha}, d)| \ge (d^2 +d)-d = d^2
$$

$$
- \sigma_d( Y_1)  {\bar {\mathrm{r}}} (Y_1) = - \sigma_d( H_1)  {\bar {\mathrm{r}}} (H_1)
= - \sigma( Y_1)  {\bar {\mathrm{r}}} (Y_1) = - \sigma( H_1)  {\bar {\mathrm{r}}} (H_1) .
$$

\begin{align*}
| {\widehat} Q| < rd^{2r-2} < 2^{4| EY_1 |} d^{2^{ 4| EY_1 |+1 }} = 2^{2^{O(| EY_1 |)}} .
\end{align*}

$$
| E \Psi(H_2^*) | <  2^{  2^{4| E \Psi(H_1) | + 1+ \log_2 \log_2 (2d)  } },
$$

$$
d' := \max\{ |I_1 \cup I_2| , \max\{ |G_{\alpha} | \, : \,   {\alpha} \in I_1 \cup I_2 \} \} .
$$

\begin{equation}\label{eq11}
 \deg v \le d' := \max \{ | I(H_1)|, \, \max \{   | G_{\alpha} |   :   {\alpha} \in   I(H_1)  \} \, \} .
 \end{equation}

$$
 \sigma( H_1) =  \sigma_{d'}( H_1) = \sup \tfrac {{\bar {\mathrm{r}}}(H_1, H_2)}{{\bar {\mathrm{r}}}(H_1)  {\bar {\mathrm{r}}}(H_2)} ,
 $$

\end{document}